simplify file organizaiton

theory/Static_Semantics.thy
@@ -142,4 +142,2184 @@ inductive may_be_static_eval :: "abstract_value_env \<times> abstract_value_env 
     (\<V>, \<C>) \<Turnstile>\<^sub>e LET x = APP f x\<^sub>a in e
   "
 
+
+fun value_to_abstract_value :: "val \<Rightarrow> abstract_value" ("|_|" [0]61) where
+  "|VUnit| = ^\<lparr>\<rparr>" |
+  "|VChan (Ch \<pi> x)| = ^Chan x" |
+  "|VClosure p \<rho>| = ^p"
+
+
+inductive 
+  may_be_static_eval_value :: "abstract_value_env \<times> abstract_value_env \<Rightarrow> val \<Rightarrow> bool" (infix "\<Turnstile>\<^sub>\<omega>" 55) and  
+  may_be_static_eval_env :: "abstract_value_env \<times> abstract_value_env \<Rightarrow> val_env \<Rightarrow> bool" (infix "\<Turnstile>\<^sub>\<rho>" 55) 
+where
+  Unit: "
+    (\<V>, \<C>) \<Turnstile>\<^sub>\<omega> VUnit
+  " |
+
+  Chan: "
+    (\<V>, \<C>) \<Turnstile>\<^sub>\<omega> VChan c
+  " |
+
+  Send_Evt: "
+    (\<V>, \<C>) \<Turnstile>\<^sub>\<rho> \<rho> \<Longrightarrow>
+    (\<V>, \<C>) \<Turnstile>\<^sub>\<omega> (VClosure (Send_Evt _ _) \<rho>)
+  " |
+
+  Recv_Evt: "
+    (\<V>, \<C>) \<Turnstile>\<^sub>\<rho> \<rho> \<Longrightarrow>
+    (\<V>, \<C>) \<Turnstile>\<^sub>\<omega> (VClosure (Recv_Evt _) \<rho>)
+  " |
+
+  Left: "
+    (\<V>, \<C>) \<Turnstile>\<^sub>\<rho> \<rho> \<Longrightarrow>
+    (\<V>, \<C>) \<Turnstile>\<^sub>\<omega> (VClosure (Left _) \<rho>)
+  " |
+
+  Right: "
+    (\<V>, \<C>) \<Turnstile>\<^sub>\<rho> \<rho> \<Longrightarrow>
+    (\<V>, \<C>) \<Turnstile>\<^sub>\<omega> (VClosure (Right _) \<rho>)
+  " |
+
+  Abs: "
+    {^Abs f x e} \<subseteq> \<V> f \<Longrightarrow> 
+    (\<V>, \<C>) \<Turnstile>\<^sub>e e \<Longrightarrow> 
+    (\<V>, \<C>) \<Turnstile>\<^sub>\<rho> \<rho> \<Longrightarrow>
+    (\<V>, \<C>) \<Turnstile>\<^sub>\<omega> (VClosure (Abs f x e) \<rho>)
+  " |
+
+  Pair: "
+    (\<V>, \<C>) \<Turnstile>\<^sub>\<rho> \<rho> \<Longrightarrow>
+    (\<V>, \<C>) \<Turnstile>\<^sub>\<omega> (VClosure (Pair _ _) \<rho>)
+  " |
+
+  Intro: " 
+    \<forall> x \<omega> . \<rho> x = Some \<omega> \<longrightarrow> {|\<omega>|} \<subseteq> \<V> x \<and> (\<V>, \<C>) \<Turnstile>\<^sub>\<omega> \<omega> \<Longrightarrow>
+    (\<V>, \<C>) \<Turnstile>\<^sub>\<rho> \<rho>
+  "
+
+
+inductive may_be_static_eval_stack :: "abstract_value_env \<times> abstract_value_env \<Rightarrow> abstract_value set \<Rightarrow> cont list \<Rightarrow> bool" ("_ \<Turnstile>\<^sub>\<kappa> _ \<Rrightarrow> _" [56,0,56]55) where
+  Empty: "(\<V>, \<C>) \<Turnstile>\<^sub>\<kappa> \<W> \<Rrightarrow> []" |
+  Nonempty: "
+    \<lbrakk> 
+      \<W> \<subseteq> \<V> x;
+      (\<V>, \<C>) \<Turnstile>\<^sub>e e;
+      (\<V>, \<C>) \<Turnstile>\<^sub>\<rho> \<rho>;
+      (\<V>, \<C>) \<Turnstile>\<^sub>\<kappa> \<V> (\<lfloor>e\<rfloor>) \<Rrightarrow> \<kappa>
+    \<rbrakk> \<Longrightarrow> 
+    (\<V>, \<C>) \<Turnstile>\<^sub>\<kappa> \<W> \<Rrightarrow> (\<langle>x, e, \<rho>\<rangle> # \<kappa>)
+  "
+
+
+inductive may_be_static_eval_state :: "abstract_value_env \<times> abstract_value_env \<Rightarrow> state \<Rightarrow> bool" (infix "\<Turnstile>\<^sub>\<sigma>" 55)  where
+  Intro: "
+    \<lbrakk>
+      (\<V>, \<C>) \<Turnstile>\<^sub>e e;
+      (\<V>, \<C>) \<Turnstile>\<^sub>\<rho> \<rho>;
+      (\<V>, \<C>) \<Turnstile>\<^sub>\<kappa> \<V> (\<lfloor>e\<rfloor>) \<Rrightarrow> \<kappa>
+    \<rbrakk> \<Longrightarrow>
+    (\<V>, \<C>) \<Turnstile>\<^sub>\<sigma> \<langle>e; \<rho>; \<kappa>\<rangle>
+  "
+
+inductive may_be_static_eval_pool :: "abstract_value_env \<times> abstract_value_env \<Rightarrow> trace_pool \<Rightarrow> bool" (infix "\<Turnstile>\<^sub>\<E>" 55) where
+  Intro: "
+    (\<forall> \<pi> \<sigma> . \<E> \<pi> = Some \<sigma> \<longrightarrow> (\<V>, \<C>) \<Turnstile>\<^sub>\<sigma> \<sigma>) \<Longrightarrow> 
+    (\<V>, \<C>) \<Turnstile>\<^sub>\<E> \<E>
+  "
+
+lemma may_be_static_eval_state_to_exp_result: "
+  (\<V>, \<C>) \<Turnstile>\<^sub>\<sigma> \<langle>RESULT x;\<rho>;\<langle>x\<^sub>\<kappa>,e\<^sub>\<kappa>,\<rho>\<^sub>\<kappa>\<rangle> # \<kappa>\<rangle> \<Longrightarrow> (\<V>, \<C>) \<Turnstile>\<^sub>e e\<^sub>\<kappa>
+"
+proof -
+  assume 
+    "(\<V>, \<C>) \<Turnstile>\<^sub>\<sigma> \<langle>RESULT x;\<rho>;\<langle>x\<^sub>\<kappa>,e\<^sub>\<kappa>,\<rho>\<^sub>\<kappa>\<rangle> # \<kappa>\<rangle>" 
+  then have 
+    "(\<V>, \<C>) \<Turnstile>\<^sub>\<kappa> \<V> x \<Rrightarrow> \<langle>x\<^sub>\<kappa>,e\<^sub>\<kappa>,\<rho>\<^sub>\<kappa>\<rangle> # \<kappa>" by (simp add: may_be_static_eval_state.simps) then
+  show 
+    "(\<V>, \<C>) \<Turnstile>\<^sub>e e\<^sub>\<kappa>" by (rule may_be_static_eval_stack.cases; auto)
+qed
+
+
+lemma may_be_static_eval_state_to_exp_let_case_left: "
+  (\<V>, \<C>) \<Turnstile>\<^sub>\<sigma> \<langle>LET x = CASE x\<^sub>s LEFT x\<^sub>l |> e\<^sub>l RIGHT x\<^sub>r |> e\<^sub>r in e; \<rho>; \<kappa>\<rangle> \<Longrightarrow> 
+  \<rho> x\<^sub>s = Some (VClosure (Left x\<^sub>l') \<rho>\<^sub>l) \<Longrightarrow> 
+  (\<V>, \<C>) \<Turnstile>\<^sub>e e\<^sub>l
+"
+proof -
+  assume 
+    H1: "\<rho> x\<^sub>s = Some (VClosure (Left x\<^sub>l') \<rho>\<^sub>l)" and
+    H2: "(\<V>, \<C>) \<Turnstile>\<^sub>\<sigma> \<langle>LET x = CASE x\<^sub>s LEFT x\<^sub>l |> e\<^sub>l RIGHT x\<^sub>r |> e\<^sub>r in e; \<rho>; \<kappa>\<rangle>" 
+
+
+  from H2 have 
+    H3: "(\<V>, \<C>) \<Turnstile>\<^sub>e LET x = CASE x\<^sub>s LEFT x\<^sub>l |> e\<^sub>l RIGHT x\<^sub>r |> e\<^sub>r in e" and
+    H4: "(\<V>, \<C>) \<Turnstile>\<^sub>\<rho> \<rho>" using may_be_static_eval_state.cases by blast+
+
+  from H4 have H5: "\<forall>x \<omega>. \<rho> x = Some \<omega> \<longrightarrow> {|\<omega>|} \<subseteq> \<V> x" using may_be_static_eval_env.simps by auto
+
+  from H1 H5 have 
+    H6: "^prim.Left x\<^sub>l' \<in> \<V> x\<^sub>s" by fastforce
+
+  from H3 show 
+    "(\<V>, \<C>) \<Turnstile>\<^sub>e e\<^sub>l"
+  proof cases
+    case Let_Case 
+
+    from H6 local.Let_Case(1) show 
+      "(\<V>, \<C>) \<Turnstile>\<^sub>e e\<^sub>l" by auto
+  qed
+qed
+
+
+lemma may_be_static_eval_state_to_exp_let_case_right: "
+  (\<V>, \<C>) \<Turnstile>\<^sub>\<sigma> \<langle>LET x = CASE x\<^sub>s LEFT x\<^sub>l |> e\<^sub>l RIGHT x\<^sub>r |> e\<^sub>r in e; \<rho>; \<kappa>\<rangle> \<Longrightarrow> 
+  \<rho> x\<^sub>s = Some (VClosure (Right x\<^sub>r') \<rho>\<^sub>r) \<Longrightarrow> 
+  (\<V>, \<C>) \<Turnstile>\<^sub>e e\<^sub>r
+"
+proof -
+  assume "\<rho> x\<^sub>s = Some (VClosure (Right x\<^sub>r') \<rho>\<^sub>r)"
+  assume "(\<V>, \<C>) \<Turnstile>\<^sub>\<sigma> \<langle>LET x = CASE x\<^sub>s LEFT x\<^sub>l |> e\<^sub>l RIGHT x\<^sub>r |> e\<^sub>r in e; \<rho>; \<kappa>\<rangle>" then
+  have "(\<V>, \<C>) \<Turnstile>\<^sub>e LET x = CASE x\<^sub>s LEFT x\<^sub>l |> e\<^sub>l RIGHT x\<^sub>r |> e\<^sub>r in e"  
+  and "(\<V>, \<C>) \<Turnstile>\<^sub>\<rho> \<rho>" 
+    by (simp add: may_be_static_eval_state.simps)+ then
+  have "\<forall>x \<omega>. \<rho> x = Some \<omega> \<longrightarrow> {|\<omega>|} \<subseteq> \<V> x" by (simp add: may_be_static_eval_env.simps)
+  with `\<rho> x\<^sub>s = Some (VClosure (Right x\<^sub>r') \<rho>\<^sub>r)`
+  have "^prim.Right x\<^sub>r' \<in> \<V> x\<^sub>s" by fastforce
+  with `(\<V>, \<C>) \<Turnstile>\<^sub>e LET x = CASE x\<^sub>s LEFT x\<^sub>l |> e\<^sub>l RIGHT x\<^sub>r |> e\<^sub>r in e`
+  show "(\<V>, \<C>) \<Turnstile>\<^sub>e e\<^sub>r"
+  proof cases
+    case Let_Case 
+    with 
+      `\<forall>x\<^sub>r'. ^prim.Right x\<^sub>r' \<in> \<V> x\<^sub>s \<longrightarrow> \<V> x\<^sub>r' \<subseteq> \<V> x\<^sub>r \<and> \<V> (\<lfloor>e\<^sub>r\<rfloor>) \<subseteq> \<V> x \<and> (\<V>, \<C>) \<Turnstile>\<^sub>e e\<^sub>r`  
+      `^prim.Right x\<^sub>r' \<in> \<V> x\<^sub>s`
+    show "(\<V>, \<C>) \<Turnstile>\<^sub>e e\<^sub>r" by blast
+  qed
+qed
+
+
+lemma may_be_static_eval_state_to_exp_let: "
+  (\<V>, \<C>) \<Turnstile>\<^sub>\<sigma> \<langle>LET x = b in e; \<rho>; \<kappa>\<rangle> \<Longrightarrow> (\<V>, \<C>) \<Turnstile>\<^sub>e e
+"
+proof -
+ assume "(\<V>, \<C>) \<Turnstile>\<^sub>\<sigma> \<langle>LET x = b in e; \<rho>; \<kappa>\<rangle>" then
+ have "(\<V>, \<C>) \<Turnstile>\<^sub>e LET x = b in e" by (simp add: may_be_static_eval_state.simps) then
+ show "(\<V>, \<C>) \<Turnstile>\<^sub>e e" by (rule may_be_static_eval.cases; auto)
+qed
+
+
+lemma may_be_static_eval_state_to_exp_let_app: "
+ (\<V>, \<C>) \<Turnstile>\<^sub>\<sigma> \<langle>LET x = APP f x\<^sub>a in e; \<rho>; \<kappa>\<rangle> \<Longrightarrow> 
+ \<rho> f = Some (VClosure (Abs f' x\<^sub>p e\<^sub>b) \<rho>') \<Longrightarrow>
+ (\<V>, \<C>) \<Turnstile>\<^sub>e e\<^sub>b
+"
+
+proof -
+  assume "\<rho> f = Some (VClosure (Abs f' x\<^sub>p e\<^sub>b) \<rho>')"
+  assume "(\<V>, \<C>) \<Turnstile>\<^sub>\<sigma> \<langle>LET x = APP f x\<^sub>a in e; \<rho>; \<kappa>\<rangle>" then
+  have "(\<V>, \<C>) \<Turnstile>\<^sub>\<rho> \<rho>" by (simp add: may_be_static_eval_state.simps) then
+  have "\<forall>x \<omega>. \<rho> x = Some \<omega> \<longrightarrow> {|\<omega>|} \<subseteq> \<V> x \<and> (\<V>, \<C>) \<Turnstile>\<^sub>\<omega> \<omega>" by (simp add: may_be_static_eval_env.simps)
+  with `\<rho> f = Some (VClosure (Abs f' x\<^sub>p e\<^sub>b) \<rho>')`
+  have "(\<V>, \<C>) \<Turnstile>\<^sub>\<omega> (VClosure (Abs f' x\<^sub>p e\<^sub>b) \<rho>')" by simp then
+  show "(\<V>, \<C>) \<Turnstile>\<^sub>e e\<^sub>b" by (rule may_be_static_eval_value.cases; auto)
+qed
+
+lemma may_be_static_eval_state_to_env_result: "
+  (\<V>, \<C>) \<Turnstile>\<^sub>\<sigma> \<langle>RESULT x; \<rho>; \<langle>x\<^sub>\<kappa>,e\<^sub>\<kappa>,\<rho>\<^sub>\<kappa>\<rangle> # \<kappa>\<rangle> \<Longrightarrow> 
+  \<rho> x = Some \<omega> \<Longrightarrow> 
+  (\<V>, \<C>) \<Turnstile>\<^sub>\<rho> \<rho>\<^sub>\<kappa>(x\<^sub>\<kappa> \<mapsto> \<omega>)
+"
+proof
+ assume "\<rho> x = Some \<omega> "
+
+ assume "(\<V>, \<C>) \<Turnstile>\<^sub>\<sigma> \<langle>RESULT x; \<rho>; \<langle>x\<^sub>\<kappa>,e\<^sub>\<kappa>,\<rho>\<^sub>\<kappa>\<rangle> # \<kappa>\<rangle>" then
+ have "(\<V>, \<C>) \<Turnstile>\<^sub>\<kappa> \<V> x \<Rrightarrow> \<langle>x\<^sub>\<kappa>,e\<^sub>\<kappa>,\<rho>\<^sub>\<kappa>\<rangle> # \<kappa>" and "(\<V>, \<C>) \<Turnstile>\<^sub>\<rho> \<rho>" by (rule may_be_static_eval_state.cases; auto)+
+
+ from `(\<V>, \<C>) \<Turnstile>\<^sub>\<rho> \<rho>` and `\<rho> x = Some \<omega>`
+ have "{|\<omega>|} \<subseteq> \<V> x" "(\<V>, \<C>) \<Turnstile>\<^sub>\<omega> \<omega>" by (simp add: may_be_static_eval_env.simps)+
+
+ from `(\<V>, \<C>) \<Turnstile>\<^sub>\<kappa> \<V> x \<Rrightarrow> \<langle>x\<^sub>\<kappa>,e\<^sub>\<kappa>,\<rho>\<^sub>\<kappa>\<rangle> # \<kappa>`
+ show "\<forall>x \<omega>'. (\<rho>\<^sub>\<kappa>(x\<^sub>\<kappa> \<mapsto> \<omega>)) x = Some \<omega>' \<longrightarrow> {|\<omega>'|} \<subseteq> \<V> x \<and> (\<V>, \<C>) \<Turnstile>\<^sub>\<omega> \<omega>'"
+ proof cases
+   case Nonempty
+   assume "\<V> x \<subseteq> \<V> x\<^sub>\<kappa>" and "(\<V>, \<C>) \<Turnstile>\<^sub>\<rho> \<rho>\<^sub>\<kappa>"
+
+   from `{|\<omega>|} \<subseteq> \<V> x` `\<V> x \<subseteq> \<V> x\<^sub>\<kappa>`
+   have "{|\<omega>|} \<subseteq> \<V> x\<^sub>\<kappa>" by blast
+
+   {
+     fix x' \<omega>'
+     assume "(\<rho>\<^sub>\<kappa>(x\<^sub>\<kappa> \<mapsto> \<omega>)) x' = Some \<omega>'" 
+
+     have "{|\<omega>'|} \<subseteq> \<V> x' \<and> (\<V>, \<C>) \<Turnstile>\<^sub>\<omega> \<omega>'" 
+     proof cases
+       assume "x' = x\<^sub>\<kappa>" with `(\<rho>\<^sub>\<kappa>(x\<^sub>\<kappa> \<mapsto> \<omega>)) x' = Some \<omega>'`
+       and  `{|\<omega>|} \<subseteq> \<V> x\<^sub>\<kappa>` `(\<V>, \<C>) \<Turnstile>\<^sub>\<omega> \<omega>`
+     
+       show "{|\<omega>'|} \<subseteq> \<V> x' \<and> (\<V>, \<C>) \<Turnstile>\<^sub>\<omega> \<omega>'" by simp
+     next
+       assume "x' \<noteq> x\<^sub>\<kappa>" with `(\<rho>\<^sub>\<kappa>(x\<^sub>\<kappa> \<mapsto> \<omega>)) x' = Some \<omega>'`
+
+       have "\<rho>\<^sub>\<kappa> x' = Some \<omega>'" by simp 
+       with `(\<V>, \<C>) \<Turnstile>\<^sub>\<rho> \<rho>\<^sub>\<kappa>`
+       
+       show "{|\<omega>'|} \<subseteq> \<V> x' \<and> (\<V>, \<C>) \<Turnstile>\<^sub>\<omega> \<omega>'" by (simp add: may_be_static_eval_env.simps)+
+     qed
+   } then
+
+   show "\<forall>x \<omega>'. (\<rho>\<^sub>\<kappa>(x\<^sub>\<kappa> \<mapsto> \<omega>)) x = Some \<omega>' \<longrightarrow> {|\<omega>'|} \<subseteq> \<V> x \<and> (\<V>, \<C>) \<Turnstile>\<^sub>\<omega> \<omega>'" by auto
+ qed
+qed
+
+
+lemma may_be_static_eval_state_to_stack_result: "
+  (\<V>, \<C>) \<Turnstile>\<^sub>\<sigma> \<langle>RESULT x; \<rho>; \<langle>x\<^sub>\<kappa>,e\<^sub>\<kappa>,\<rho>\<^sub>\<kappa>\<rangle> # \<kappa>\<rangle> \<Longrightarrow> 
+  \<rho> x = Some \<omega> \<Longrightarrow> 
+  (\<V>, \<C>) \<Turnstile>\<^sub>\<kappa> \<V> (\<lfloor>e\<^sub>\<kappa>\<rfloor>) \<Rrightarrow> \<kappa>
+"
+proof -
+  assume "\<rho> x = Some \<omega>"
+  assume "(\<V>, \<C>) \<Turnstile>\<^sub>\<sigma> \<langle>RESULT x; \<rho>; \<langle>x\<^sub>\<kappa>,e\<^sub>\<kappa>,\<rho>\<^sub>\<kappa>\<rangle> # \<kappa>\<rangle>" then
+  have "(\<V>, \<C>) \<Turnstile>\<^sub>\<kappa> \<V> x \<Rrightarrow> \<langle>x\<^sub>\<kappa>,e\<^sub>\<kappa>,\<rho>\<^sub>\<kappa>\<rangle> # \<kappa>" by (simp add: may_be_static_eval_state.simps) then
+  show "(\<V>, \<C>) \<Turnstile>\<^sub>\<kappa> \<V> (\<lfloor>e\<^sub>\<kappa>\<rfloor>) \<Rrightarrow> \<kappa>" by (rule may_be_static_eval_stack.cases; auto)
+qed
+
+
+lemma may_be_static_eval_state_to_state_result: "
+  (\<V>, \<C>) \<Turnstile>\<^sub>\<sigma> \<langle>RESULT x; \<rho>; \<langle>x\<^sub>\<kappa>,e\<^sub>\<kappa>,\<rho>\<^sub>\<kappa>\<rangle> # \<kappa>\<rangle> \<Longrightarrow> 
+  \<rho> x = Some \<omega> \<Longrightarrow> 
+  (\<V>, \<C>) \<Turnstile>\<^sub>\<sigma> \<langle>e\<^sub>\<kappa>; \<rho>\<^sub>\<kappa>(x\<^sub>\<kappa> \<mapsto> \<omega>); \<kappa>\<rangle>
+"
+proof
+  assume "\<rho> x = Some \<omega>" "(\<V>, \<C>) \<Turnstile>\<^sub>\<sigma> \<langle>RESULT x; \<rho>; \<langle>x\<^sub>\<kappa>,e\<^sub>\<kappa>,\<rho>\<^sub>\<kappa>\<rangle> # \<kappa>\<rangle>" then
+  show "(\<V>, \<C>) \<Turnstile>\<^sub>\<rho> \<rho>\<^sub>\<kappa>(x\<^sub>\<kappa> \<mapsto> \<omega>)" by (blast intro: may_be_static_eval_state_to_env_result)
+
+  with `(\<V>, \<C>) \<Turnstile>\<^sub>\<sigma> \<langle>RESULT x; \<rho>; \<langle>x\<^sub>\<kappa>,e\<^sub>\<kappa>,\<rho>\<^sub>\<kappa>\<rangle> # \<kappa>\<rangle>`
+  show "(\<V>, \<C>) \<Turnstile>\<^sub>e e\<^sub>\<kappa>" by (blast intro: may_be_static_eval_state_to_exp_result)
+
+  with `\<rho> x = Some \<omega>` `(\<V>, \<C>) \<Turnstile>\<^sub>\<sigma> \<langle>RESULT x; \<rho>; \<langle>x\<^sub>\<kappa>,e\<^sub>\<kappa>,\<rho>\<^sub>\<kappa>\<rangle> # \<kappa>\<rangle>`
+  show "(\<V>, \<C>) \<Turnstile>\<^sub>\<kappa> \<V> (\<lfloor>e\<^sub>\<kappa>\<rfloor>) \<Rrightarrow> \<kappa>" by (blast intro: may_be_static_eval_state_to_stack_result)
+qed
+
+
+lemma may_be_static_eval_state_to_env_let_unit: "
+  (\<V>, \<C>) \<Turnstile>\<^sub>\<sigma> \<langle>LET x = \<lparr>\<rparr> in e; \<rho>; \<kappa>\<rangle> \<Longrightarrow> (\<V>, \<C>) \<Turnstile>\<^sub>\<rho> \<rho>(x \<mapsto> VUnit)
+"
+proof
+  assume "(\<V>, \<C>) \<Turnstile>\<^sub>\<sigma> \<langle>LET x = \<lparr>\<rparr> in e; \<rho>; \<kappa>\<rangle>" then 
+  have "(\<V>, \<C>) \<Turnstile>\<^sub>e LET x = \<lparr>\<rparr> in e" "(\<V>, \<C>) \<Turnstile>\<^sub>\<rho> \<rho>" by (simp add: may_be_static_eval_state.simps)+ 
+
+  from `(\<V>, \<C>) \<Turnstile>\<^sub>e LET x = \<lparr>\<rparr> in e`
+  have "{^\<lparr>\<rparr>} \<subseteq> \<V> x" by (rule may_be_static_eval.cases; auto)+
+  have "(\<V>, \<C>) \<Turnstile>\<^sub>\<omega> VUnit" by (simp add: Unit)
+
+  {
+    fix x' \<omega>'
+    assume "(\<rho>(x \<mapsto> VUnit)) x' = Some \<omega>'" 
+    have "{|\<omega>'|} \<subseteq> \<V> x' \<and> (\<V>, \<C>) \<Turnstile>\<^sub>\<omega> \<omega>'"
+    proof cases
+      assume "x' = x" 
+      with `(\<rho>(x \<mapsto> VUnit)) x' = Some \<omega>'` 
+      and `{^\<lparr>\<rparr>} \<subseteq> \<V> x` `(\<V>, \<C>) \<Turnstile>\<^sub>\<omega> VUnit`
+
+      show "{|\<omega>'|} \<subseteq> \<V> x' \<and> (\<V>, \<C>) \<Turnstile>\<^sub>\<omega> \<omega>'" by simp
+    next 
+      assume "x' \<noteq> x"  with `(\<rho>(x \<mapsto> VUnit)) x' = Some \<omega>'` 
+
+      have "\<rho> x' = Some \<omega>'" by simp
+
+      from `(\<V>, \<C>) \<Turnstile>\<^sub>\<rho> \<rho>` `\<rho> x' = Some \<omega>'`
+
+      show "{|\<omega>'|} \<subseteq> \<V> x' \<and> (\<V>, \<C>) \<Turnstile>\<^sub>\<omega> \<omega>'" by (simp add: may_be_static_eval_env.simps)
+    qed
+
+  }
+  with `{^\<lparr>\<rparr>} \<subseteq> \<V> x` `(\<V>, \<C>) \<Turnstile>\<^sub>\<omega> VUnit`
+  show "\<forall>x' \<omega>'. (\<rho>(x \<mapsto> VUnit)) x' = Some \<omega>' \<longrightarrow> {|\<omega>'|} \<subseteq> \<V> x' \<and> (\<V>, \<C>) \<Turnstile>\<^sub>\<omega> \<omega>'" by auto
+qed
+
+
+lemma may_be_static_eval_state_to_stack_let: "
+  (\<V>, \<C>) \<Turnstile>\<^sub>\<sigma> \<langle>LET x = b in e; \<rho>; \<kappa>\<rangle> \<Longrightarrow> (\<V>, \<C>) \<Turnstile>\<^sub>\<kappa> \<V> (\<lfloor>e\<rfloor>) \<Rrightarrow> \<kappa>
+"
+by (erule may_be_static_eval_state.cases; auto)
+
+lemma may_be_static_eval_state_to_state_let_unit: "
+  (\<V>, \<C>) \<Turnstile>\<^sub>\<sigma> \<langle>LET x = \<lparr>\<rparr> in e; \<rho>; \<kappa>\<rangle> \<Longrightarrow> (\<V>, \<C>) \<Turnstile>\<^sub>\<sigma> \<langle>e; \<rho>(x \<mapsto> VUnit); \<kappa>\<rangle>
+"
+proof
+  assume "(\<V>, \<C>) \<Turnstile>\<^sub>\<sigma> \<langle>LET x = \<lparr>\<rparr> in e; \<rho>; \<kappa>\<rangle>" then
+  show "(\<V>, \<C>) \<Turnstile>\<^sub>e e" by (auto simp: may_be_static_eval_state_to_exp_let)
+
+  from `(\<V>, \<C>) \<Turnstile>\<^sub>\<sigma> \<langle>LET x = \<lparr>\<rparr> in e; \<rho>; \<kappa>\<rangle>` 
+  show "(\<V>, \<C>) \<Turnstile>\<^sub>\<rho> \<rho>(x \<mapsto> VUnit)" by (auto simp: may_be_static_eval_state_to_env_let_unit)
+
+  from `(\<V>, \<C>) \<Turnstile>\<^sub>\<sigma> \<langle>LET x = \<lparr>\<rparr> in e; \<rho>; \<kappa>\<rangle>` 
+  show "(\<V>, \<C>) \<Turnstile>\<^sub>\<kappa> \<V> (\<lfloor>e\<rfloor>) \<Rrightarrow> \<kappa>" by (auto simp: may_be_static_eval_state_to_stack_let)
+
+qed
+
+lemma may_be_static_eval_to_value_let_prim: "
+  (\<V>, \<C>) \<Turnstile>\<^sub>e LET x = Prim p in e \<Longrightarrow> (\<V>, \<C>) \<Turnstile>\<^sub>\<rho> \<rho> \<Longrightarrow> (\<V>, \<C>) \<Turnstile>\<^sub>\<omega> (VClosure p \<rho>)
+"
+by (erule may_be_static_eval.cases; auto; rule; auto)
+
+lemma may_be_static_eval_state_to_env_let_prim: "
+  (\<V>, \<C>) \<Turnstile>\<^sub>\<sigma> \<langle>LET x = Prim p in e; \<rho>; \<kappa>\<rangle> \<Longrightarrow> (\<V>, \<C>) \<Turnstile>\<^sub>\<rho> \<rho>(x \<mapsto> (VClosure p \<rho>))
+"
+proof
+  assume "(\<V>, \<C>) \<Turnstile>\<^sub>\<sigma> \<langle>LET x = Prim p in e; \<rho>; \<kappa>\<rangle> " then 
+  have "(\<V>, \<C>) \<Turnstile>\<^sub>e LET x = Prim p in e" "(\<V>, \<C>) \<Turnstile>\<^sub>\<rho> \<rho>" by (simp add: may_be_static_eval_state.simps)+ then
+  have "(\<V>, \<C>) \<Turnstile>\<^sub>\<omega> (VClosure p \<rho>)" by (simp add: may_be_static_eval_to_value_let_prim)
+
+  from `(\<V>, \<C>) \<Turnstile>\<^sub>e LET x = Prim p in e`
+  have "{^p} \<subseteq> \<V> x" by (rule may_be_static_eval.cases; auto)+
+ 
+  {
+    fix x' \<omega>'
+    assume "(\<rho>(x \<mapsto> (VClosure p \<rho>))) x' = Some \<omega>'" 
+    have "{|\<omega>'|} \<subseteq> \<V> x' \<and> (\<V>, \<C>) \<Turnstile>\<^sub>\<omega> \<omega>'"
+    proof cases
+      assume "x' = x" with \<open>(\<rho>(x \<mapsto> (VClosure p \<rho>))) x' = Some \<omega>'\<close>
+      and `{^p} \<subseteq> \<V> x` `(\<V>, \<C>) \<Turnstile>\<^sub>\<omega> (VClosure p \<rho>)`
+
+      show "{|\<omega>'|} \<subseteq> \<V> x' \<and> (\<V>, \<C>) \<Turnstile>\<^sub>\<omega> \<omega>'" by auto
+    next
+      assume  "x' \<noteq> x"  with \<open>(\<rho>(x \<mapsto> (VClosure p \<rho>))) x' = Some \<omega>'\<close>
+
+      have "\<rho> x' = Some \<omega>'" by simp
+      with `(\<V>, \<C>) \<Turnstile>\<^sub>\<rho> \<rho>` 
+  
+      show "{|\<omega>'|} \<subseteq> \<V> x' \<and> (\<V>, \<C>) \<Turnstile>\<^sub>\<omega> \<omega>'" by (simp add: may_be_static_eval_env.simps)
+    qed
+
+  } then
+
+  show "\<forall>x' \<omega>'. (\<rho>(x \<mapsto> (VClosure p \<rho>))) x' = Some \<omega>' \<longrightarrow> {|\<omega>'|} \<subseteq> \<V> x' \<and> (\<V>, \<C>) \<Turnstile>\<^sub>\<omega> \<omega>'" by auto
+qed
+
+lemma may_be_static_eval_state_to_state_let_prim: "
+  (\<V>, \<C>) \<Turnstile>\<^sub>\<sigma> \<langle>LET x = Prim p in e; \<rho>; \<kappa>\<rangle> \<Longrightarrow> (\<V>, \<C>) \<Turnstile>\<^sub>\<sigma> \<langle>e; \<rho>(x \<mapsto> (VClosure p \<rho>)); \<kappa>\<rangle>
+"
+proof
+  assume "(\<V>, \<C>) \<Turnstile>\<^sub>\<sigma> \<langle>LET x = Prim p in e; \<rho>; \<kappa>\<rangle>" then
+  show "(\<V>, \<C>) \<Turnstile>\<^sub>e e" by (auto simp: may_be_static_eval_state_to_exp_let)
+
+  from `(\<V>, \<C>) \<Turnstile>\<^sub>\<sigma> \<langle>LET x = Prim p in e; \<rho>; \<kappa>\<rangle>` 
+  show "(\<V>, \<C>) \<Turnstile>\<^sub>\<kappa> \<V> (\<lfloor>e\<rfloor>) \<Rrightarrow> \<kappa>" by (auto simp: may_be_static_eval_state_to_stack_let)
+
+  from `(\<V>, \<C>) \<Turnstile>\<^sub>\<sigma> \<langle>LET x = Prim p in e; \<rho>; \<kappa>\<rangle>` 
+  show "(\<V>, \<C>) \<Turnstile>\<^sub>\<rho> \<rho>(x \<mapsto> (VClosure p \<rho>))" by (auto simp: may_be_static_eval_state_to_env_let_prim)
+
+qed
+
+
+lemma may_be_static_eval_state_to_env_let_case_left: "
+  (\<V>, \<C>) \<Turnstile>\<^sub>\<sigma> \<langle>LET x = CASE x\<^sub>s LEFT x\<^sub>l |> e\<^sub>l RIGHT x\<^sub>r |> e\<^sub>r in e; \<rho>; \<kappa>\<rangle> \<Longrightarrow> 
+  \<rho> x\<^sub>s = Some (VClosure (Left x\<^sub>l') \<rho>\<^sub>l) \<Longrightarrow> \<rho>\<^sub>l x\<^sub>l' = Some \<omega>\<^sub>l \<Longrightarrow> 
+  (\<V>, \<C>) \<Turnstile>\<^sub>\<rho> \<rho>(x\<^sub>l \<mapsto> \<omega>\<^sub>l)
+"
+
+proof
+  assume "\<rho> x\<^sub>s = Some (VClosure (Left x\<^sub>l') \<rho>\<^sub>l)" "\<rho>\<^sub>l x\<^sub>l' = Some \<omega>\<^sub>l"
+  assume "(\<V>, \<C>) \<Turnstile>\<^sub>\<sigma> \<langle>LET x = CASE x\<^sub>s LEFT x\<^sub>l |> e\<^sub>l RIGHT x\<^sub>r |> e\<^sub>r in e; \<rho>; \<kappa>\<rangle>" then 
+  have "(\<V>, \<C>) \<Turnstile>\<^sub>e LET x = CASE x\<^sub>s LEFT x\<^sub>l |> e\<^sub>l RIGHT x\<^sub>r |> e\<^sub>r in e" "(\<V>, \<C>) \<Turnstile>\<^sub>\<rho> \<rho>" by (simp add: may_be_static_eval_state.simps)+
+
+  from `(\<V>, \<C>) \<Turnstile>\<^sub>\<rho> \<rho>` `\<rho> x\<^sub>s = Some (VClosure (Left x\<^sub>l') \<rho>\<^sub>l)`
+  have "(\<V>, \<C>) \<Turnstile>\<^sub>\<omega> (VClosure (Left x\<^sub>l') \<rho>\<^sub>l)" by (blast intro: may_be_static_eval_env.cases) then
+  have "(\<V>, \<C>) \<Turnstile>\<^sub>\<rho> \<rho>\<^sub>l" by (blast intro: may_be_static_eval_value.cases)
+
+  from `(\<V>, \<C>) \<Turnstile>\<^sub>\<rho> \<rho>\<^sub>l` `\<rho>\<^sub>l x\<^sub>l' = Some \<omega>\<^sub>l`
+  have "{|\<omega>\<^sub>l|} \<subseteq> \<V> x\<^sub>l'" "(\<V>, \<C>) \<Turnstile>\<^sub>\<omega> \<omega>\<^sub>l" by (blast intro: may_be_static_eval_env.cases)+
+
+  from `(\<V>, \<C>) \<Turnstile>\<^sub>\<rho> \<rho>` `\<rho> x\<^sub>s = Some (VClosure (Left x\<^sub>l') \<rho>\<^sub>l)`
+  have " | (VClosure (Left x\<^sub>l') \<rho>\<^sub>l) | \<in> \<V> x\<^sub>s" by (blast intro: may_be_static_eval_env.cases) then
+  have "^prim.Left x\<^sub>l' \<in> \<V> x\<^sub>s" by simp
+
+  from  `(\<V>, \<C>) \<Turnstile>\<^sub>e LET x = CASE x\<^sub>s LEFT x\<^sub>l |> e\<^sub>l RIGHT x\<^sub>r |> e\<^sub>r in e`
+  have "\<V> x\<^sub>l' \<subseteq> \<V> x\<^sub>l"
+  proof cases
+    case Let_Case
+    from `\<forall>x\<^sub>l'. ^prim.Left x\<^sub>l' \<in> \<V> x\<^sub>s \<longrightarrow> \<V> x\<^sub>l' \<subseteq> \<V> x\<^sub>l \<and> \<V> (\<lfloor>e\<^sub>l\<rfloor>) \<subseteq> \<V> x \<and> (\<V>, \<C>) \<Turnstile>\<^sub>e e\<^sub>l`
+    and `^prim.Left x\<^sub>l' \<in> \<V> x\<^sub>s`
+    show "\<V> x\<^sub>l' \<subseteq> \<V> x\<^sub>l" by simp
+  qed
+
+  from `{|\<omega>\<^sub>l|} \<subseteq> \<V> x\<^sub>l'` `\<V> x\<^sub>l' \<subseteq> \<V> x\<^sub>l` 
+  have "{|\<omega>\<^sub>l|} \<subseteq> \<V> x\<^sub>l" by blast
+
+  {
+    fix x' \<omega>'
+    assume "(\<rho>(x\<^sub>l \<mapsto> \<omega>\<^sub>l)) x' = Some \<omega>'" "x' \<noteq> x\<^sub>l" then
+    have "\<rho> x' = Some \<omega>'" by simp
+    with `(\<V>, \<C>) \<Turnstile>\<^sub>\<rho> \<rho>` 
+    have "{|\<omega>'|} \<subseteq> \<V> x' \<and> (\<V>, \<C>) \<Turnstile>\<^sub>\<omega> \<omega>'" by (simp add: may_be_static_eval_env.simps)
+   
+  }
+  with `{|\<omega>\<^sub>l|} \<subseteq> \<V> x\<^sub>l` `(\<V>, \<C>) \<Turnstile>\<^sub>\<omega> \<omega>\<^sub>l`
+  show "\<forall>x' \<omega>'. (\<rho>(x\<^sub>l \<mapsto> \<omega>\<^sub>l)) x' = Some \<omega>' \<longrightarrow> {|\<omega>'|} \<subseteq> \<V> x' \<and> (\<V>, \<C>) \<Turnstile>\<^sub>\<omega> \<omega>'" by auto
+qed
+
+
+lemma may_be_static_eval_state_to_stack_let_case_left: "
+  (\<V>, \<C>) \<Turnstile>\<^sub>\<sigma> \<langle>LET x = CASE x\<^sub>s LEFT x\<^sub>l |> e\<^sub>l RIGHT x\<^sub>r |> e\<^sub>r in e; \<rho>; \<kappa>\<rangle> \<Longrightarrow>
+  \<rho> x\<^sub>s = Some (VClosure (Left x\<^sub>l') \<rho>\<^sub>l) \<Longrightarrow> \<rho>\<^sub>l x\<^sub>l' = Some \<omega>\<^sub>l \<Longrightarrow> 
+  (\<V>, \<C>) \<Turnstile>\<^sub>\<kappa> \<V> (\<lfloor>e\<^sub>l\<rfloor>) \<Rrightarrow> \<langle>x,e,\<rho>\<rangle> # \<kappa>
+"
+proof
+
+  assume "(\<V>, \<C>) \<Turnstile>\<^sub>\<sigma> \<langle>LET x = CASE x\<^sub>s LEFT x\<^sub>l |> e\<^sub>l RIGHT x\<^sub>r |> e\<^sub>r in e; \<rho>; \<kappa>\<rangle>"
+  assume "\<rho> x\<^sub>s = Some (VClosure (Left x\<^sub>l') \<rho>\<^sub>l)" "\<rho>\<^sub>l x\<^sub>l' = Some \<omega>\<^sub>l"
+
+  from `(\<V>, \<C>) \<Turnstile>\<^sub>\<sigma> \<langle>LET x = CASE x\<^sub>s LEFT x\<^sub>l |> e\<^sub>l RIGHT x\<^sub>r |> e\<^sub>r in e;\<rho>;\<kappa>\<rangle>`
+  have "(\<V>, \<C>) \<Turnstile>\<^sub>e LET x = CASE x\<^sub>s LEFT x\<^sub>l |> e\<^sub>l RIGHT x\<^sub>r |> e\<^sub>r in e" "(\<V>, \<C>) \<Turnstile>\<^sub>\<rho> \<rho>" by (blast intro: may_be_static_eval_state.cases)+
+  
+  from `(\<V>, \<C>) \<Turnstile>\<^sub>\<rho> \<rho>` `\<rho> x\<^sub>s = Some (VClosure (Left x\<^sub>l') \<rho>\<^sub>l)`
+  have " | (VClosure (Left x\<^sub>l') \<rho>\<^sub>l) | \<in> \<V> x\<^sub>s" by (blast intro: may_be_static_eval_env.cases) then
+  have "^prim.Left x\<^sub>l' \<in> \<V> x\<^sub>s" by simp
+
+  from `(\<V>, \<C>) \<Turnstile>\<^sub>e LET x = CASE x\<^sub>s LEFT x\<^sub>l |> e\<^sub>l RIGHT x\<^sub>r |> e\<^sub>r in e`
+  show "\<V> (\<lfloor>e\<^sub>l\<rfloor>) \<subseteq> \<V> x" 
+  proof cases
+    case Let_Case
+    assume "\<forall>x\<^sub>l'. ^prim.Left x\<^sub>l' \<in> \<V> x\<^sub>s \<longrightarrow> \<V> x\<^sub>l' \<subseteq> \<V> x\<^sub>l \<and> \<V> (\<lfloor>e\<^sub>l\<rfloor>) \<subseteq> \<V> x \<and> (\<V>, \<C>) \<Turnstile>\<^sub>e e\<^sub>l"
+    with `^prim.Left x\<^sub>l' \<in> \<V> x\<^sub>s`
+    show "\<V> (\<lfloor>e\<^sub>l\<rfloor>) \<subseteq> \<V> x" by blast
+  qed
+
+  from `(\<V>, \<C>) \<Turnstile>\<^sub>\<sigma> \<langle>LET x = CASE x\<^sub>s LEFT x\<^sub>l |> e\<^sub>l RIGHT x\<^sub>r |> e\<^sub>r in e;\<rho>;\<kappa>\<rangle>`
+  show "(\<V>, \<C>) \<Turnstile>\<^sub>e e" by (blast intro: may_be_static_eval_state_to_exp_let)
+
+  from `(\<V>, \<C>) \<Turnstile>\<^sub>\<sigma> \<langle>LET x = CASE x\<^sub>s LEFT x\<^sub>l |> e\<^sub>l RIGHT x\<^sub>r |> e\<^sub>r in e;\<rho>;\<kappa>\<rangle>`
+  show "(\<V>, \<C>) \<Turnstile>\<^sub>\<rho> \<rho>" by (blast intro: may_be_static_eval_state.cases)
+
+  from `(\<V>, \<C>) \<Turnstile>\<^sub>\<sigma> \<langle>LET x = CASE x\<^sub>s LEFT x\<^sub>l |> e\<^sub>l RIGHT x\<^sub>r |> e\<^sub>r in e;\<rho>;\<kappa>\<rangle>`
+  show "(\<V>, \<C>) \<Turnstile>\<^sub>\<kappa> \<V> (\<lfloor>e\<rfloor>) \<Rrightarrow> \<kappa>" by (blast intro: may_be_static_eval_state_to_stack_let)
+  
+qed
+
+
+lemma may_be_static_eval_state_to_state_let_case_left: "
+  (\<V>, \<C>) \<Turnstile>\<^sub>\<sigma> \<langle>LET x = CASE x\<^sub>s LEFT x\<^sub>l |> e\<^sub>l RIGHT x\<^sub>r |> e\<^sub>r in e; \<rho>; \<kappa>\<rangle> \<Longrightarrow> 
+  \<rho> x\<^sub>s = Some (VClosure (Left x\<^sub>l') \<rho>\<^sub>l) \<Longrightarrow> 
+  \<rho>\<^sub>l x\<^sub>l' = Some \<omega>\<^sub>l \<Longrightarrow> 
+  (\<V>, \<C>) \<Turnstile>\<^sub>\<sigma> \<langle>e\<^sub>l; \<rho>(x\<^sub>l \<mapsto> \<omega>\<^sub>l); \<langle>x,e,\<rho>\<rangle> # \<kappa>\<rangle>
+"
+proof
+  assume "(\<V>, \<C>) \<Turnstile>\<^sub>\<sigma> \<langle>LET x = CASE x\<^sub>s LEFT x\<^sub>l |> e\<^sub>l RIGHT x\<^sub>r |> e\<^sub>r in e; \<rho>; \<kappa>\<rangle>" and "\<rho> x\<^sub>s = Some (VClosure (Left x\<^sub>l') \<rho>\<^sub>l)" then
+  show "(\<V>, \<C>) \<Turnstile>\<^sub>e e\<^sub>l" by (simp add: may_be_static_eval_state_to_exp_let_case_left)
+
+  assume "\<rho>\<^sub>l x\<^sub>l' = Some \<omega>\<^sub>l"
+  with `(\<V>, \<C>) \<Turnstile>\<^sub>\<sigma> \<langle>LET x = CASE x\<^sub>s LEFT x\<^sub>l |> e\<^sub>l RIGHT x\<^sub>r |> e\<^sub>r in e; \<rho>; \<kappa>\<rangle>` and `\<rho> x\<^sub>s = Some (VClosure (Left x\<^sub>l') \<rho>\<^sub>l)` 
+  show "(\<V>, \<C>) \<Turnstile>\<^sub>\<rho> \<rho>(x\<^sub>l \<mapsto> \<omega>\<^sub>l)" by (simp add: may_be_static_eval_state_to_env_let_case_left)
+
+  from `\<rho>\<^sub>l x\<^sub>l' = Some \<omega>\<^sub>l`  
+  and `(\<V>, \<C>) \<Turnstile>\<^sub>\<sigma> \<langle>LET x = CASE x\<^sub>s LEFT x\<^sub>l |> e\<^sub>l RIGHT x\<^sub>r |> e\<^sub>r in e; \<rho>; \<kappa>\<rangle>` 
+  and `\<rho> x\<^sub>s = Some (VClosure (Left x\<^sub>l') \<rho>\<^sub>l)` 
+  show "(\<V>, \<C>) \<Turnstile>\<^sub>\<kappa> \<V> (\<lfloor>e\<^sub>l\<rfloor>) \<Rrightarrow> \<langle>x,e,\<rho>\<rangle> # \<kappa>" by (simp add: may_be_static_eval_state_to_stack_let_case_left)
+qed
+
+
+lemma may_be_static_eval_state_to_env_let_case_right: "
+  (\<V>, \<C>) \<Turnstile>\<^sub>\<sigma> \<langle>LET x = CASE x\<^sub>s LEFT x\<^sub>l |> e\<^sub>l RIGHT x\<^sub>r |> e\<^sub>r in e; \<rho>; \<kappa>\<rangle> \<Longrightarrow> 
+  \<rho> x\<^sub>s = Some (VClosure (Right x\<^sub>r') \<rho>\<^sub>r) \<Longrightarrow> \<rho>\<^sub>r x\<^sub>r' = Some \<omega>\<^sub>r \<Longrightarrow> 
+  (\<V>, \<C>) \<Turnstile>\<^sub>\<rho> \<rho>(x\<^sub>r \<mapsto> \<omega>\<^sub>r)
+"
+
+proof
+  assume "\<rho> x\<^sub>s = Some (VClosure (Right x\<^sub>r') \<rho>\<^sub>r)" "\<rho>\<^sub>r x\<^sub>r' = Some \<omega>\<^sub>r"
+  assume "(\<V>, \<C>) \<Turnstile>\<^sub>\<sigma> \<langle>LET x = CASE x\<^sub>s LEFT x\<^sub>l |> e\<^sub>l RIGHT x\<^sub>r |> e\<^sub>r in e; \<rho>; \<kappa>\<rangle>" then 
+  have "(\<V>, \<C>) \<Turnstile>\<^sub>e LET x = CASE x\<^sub>s LEFT x\<^sub>l |> e\<^sub>l RIGHT x\<^sub>r |> e\<^sub>r in e" "(\<V>, \<C>) \<Turnstile>\<^sub>\<rho> \<rho>" by (simp add: may_be_static_eval_state.simps)+
+
+  from `(\<V>, \<C>) \<Turnstile>\<^sub>\<rho> \<rho>` `\<rho> x\<^sub>s = Some (VClosure (Right x\<^sub>r') \<rho>\<^sub>r)`
+  have "(\<V>, \<C>) \<Turnstile>\<^sub>\<omega> (VClosure (Right x\<^sub>r') \<rho>\<^sub>r)" by (blast intro: may_be_static_eval_env.cases) then
+  have "(\<V>, \<C>) \<Turnstile>\<^sub>\<rho> \<rho>\<^sub>r" by (blast intro: may_be_static_eval_value.cases)
+
+  from `(\<V>, \<C>) \<Turnstile>\<^sub>\<rho> \<rho>\<^sub>r` `\<rho>\<^sub>r x\<^sub>r' = Some \<omega>\<^sub>r`
+  have "{|\<omega>\<^sub>r|} \<subseteq> \<V> x\<^sub>r'" "(\<V>, \<C>) \<Turnstile>\<^sub>\<omega> \<omega>\<^sub>r" by (blast intro: may_be_static_eval_env.cases)+
+
+  from `(\<V>, \<C>) \<Turnstile>\<^sub>\<rho> \<rho>` `\<rho> x\<^sub>s = Some (VClosure (Right x\<^sub>r') \<rho>\<^sub>r)`
+  have " | (VClosure (Right x\<^sub>r') \<rho>\<^sub>r) | \<in> \<V> x\<^sub>s" by (blast intro: may_be_static_eval_env.cases) then
+  have "^prim.Right x\<^sub>r' \<in> \<V> x\<^sub>s" by simp
+
+  from  `(\<V>, \<C>) \<Turnstile>\<^sub>e LET x = CASE x\<^sub>s LEFT x\<^sub>l |> e\<^sub>l RIGHT x\<^sub>r |> e\<^sub>r in e`
+  have "\<V> x\<^sub>r' \<subseteq> \<V> x\<^sub>r"
+  proof cases
+    case Let_Case
+    from `\<forall>x\<^sub>r'. ^prim.Right x\<^sub>r' \<in> \<V> x\<^sub>s \<longrightarrow> \<V> x\<^sub>r' \<subseteq> \<V> x\<^sub>r \<and> \<V> (\<lfloor>e\<^sub>r\<rfloor>) \<subseteq> \<V> x \<and> (\<V>, \<C>) \<Turnstile>\<^sub>e e\<^sub>r`
+    and `^prim.Right x\<^sub>r' \<in> \<V> x\<^sub>s`
+    show "\<V> x\<^sub>r' \<subseteq> \<V> x\<^sub>r" by simp
+  qed
+
+  from `{|\<omega>\<^sub>r|} \<subseteq> \<V> x\<^sub>r'` `\<V> x\<^sub>r' \<subseteq> \<V> x\<^sub>r` 
+  have "{|\<omega>\<^sub>r|} \<subseteq> \<V> x\<^sub>r" by blast
+
+  {
+    fix x' \<omega>'
+    assume "(\<rho>(x\<^sub>r \<mapsto> \<omega>\<^sub>r)) x' = Some \<omega>'" "x' \<noteq> x\<^sub>r" then
+    have "\<rho> x' = Some \<omega>'" by simp
+    with `(\<V>, \<C>) \<Turnstile>\<^sub>\<rho> \<rho>` 
+    have "{|\<omega>'|} \<subseteq> \<V> x' \<and> (\<V>, \<C>) \<Turnstile>\<^sub>\<omega> \<omega>'" by (simp add: may_be_static_eval_env.simps)
+   
+  }
+  with `{|\<omega>\<^sub>r|} \<subseteq> \<V> x\<^sub>r` `(\<V>, \<C>) \<Turnstile>\<^sub>\<omega> \<omega>\<^sub>r`
+  show "\<forall>x' \<omega>'. (\<rho>(x\<^sub>r \<mapsto> \<omega>\<^sub>r)) x' = Some \<omega>' \<longrightarrow> {|\<omega>'|} \<subseteq> \<V> x' \<and> (\<V>, \<C>) \<Turnstile>\<^sub>\<omega> \<omega>'" by auto
+qed
+
+lemma may_be_static_eval_state_to_stack_let_case_right: "
+  (\<V>, \<C>) \<Turnstile>\<^sub>\<sigma>  \<langle>LET x = CASE x\<^sub>s LEFT x\<^sub>l |> e\<^sub>l RIGHT x\<^sub>r |> e\<^sub>r in e; \<rho>; \<kappa>\<rangle> \<Longrightarrow>
+  \<rho> x\<^sub>s = Some (VClosure (Right x\<^sub>r') \<rho>\<^sub>r) \<Longrightarrow> \<rho>\<^sub>r x\<^sub>r' = Some \<omega>\<^sub>r \<Longrightarrow> 
+  (\<V>, \<C>) \<Turnstile>\<^sub>\<kappa>  \<V> (\<lfloor>e\<^sub>r\<rfloor>) \<Rrightarrow> \<langle>x,e,\<rho>\<rangle> # \<kappa>
+"
+proof
+
+  assume "(\<V>, \<C>) \<Turnstile>\<^sub>\<sigma> \<langle>LET x = CASE x\<^sub>s LEFT x\<^sub>l |> e\<^sub>l RIGHT x\<^sub>r |> e\<^sub>r in e; \<rho>; \<kappa>\<rangle>"
+  assume "\<rho> x\<^sub>s = Some (VClosure (Right x\<^sub>r') \<rho>\<^sub>r)" "\<rho>\<^sub>r x\<^sub>r' = Some \<omega>\<^sub>r"
+
+  from `(\<V>, \<C>) \<Turnstile>\<^sub>\<sigma> \<langle>LET x = CASE x\<^sub>s LEFT x\<^sub>l |> e\<^sub>l RIGHT x\<^sub>r |> e\<^sub>r in e;\<rho>;\<kappa>\<rangle>`
+  have "(\<V>, \<C>) \<Turnstile>\<^sub>e LET x = CASE x\<^sub>s LEFT x\<^sub>l |> e\<^sub>l RIGHT x\<^sub>r |> e\<^sub>r in e" "(\<V>, \<C>) \<Turnstile>\<^sub>\<rho> \<rho>" by (blast intro: may_be_static_eval_state.cases)+
+  
+  from `(\<V>, \<C>) \<Turnstile>\<^sub>\<rho> \<rho>` `\<rho> x\<^sub>s = Some (VClosure (Right x\<^sub>r') \<rho>\<^sub>r)`
+  have " | (VClosure (Right x\<^sub>r') \<rho>\<^sub>r) | \<in> \<V> x\<^sub>s" by (blast intro: may_be_static_eval_env.cases) then
+  have "^prim.Right x\<^sub>r' \<in> \<V> x\<^sub>s" by simp
+
+  from `(\<V>, \<C>) \<Turnstile>\<^sub>e LET x = CASE x\<^sub>s LEFT x\<^sub>l |> e\<^sub>l RIGHT x\<^sub>r |> e\<^sub>r in e`
+  show "\<V> (\<lfloor>e\<^sub>r\<rfloor>) \<subseteq> \<V> x" 
+  proof cases
+    case Let_Case
+    assume "\<forall>x\<^sub>r'. ^prim.Right x\<^sub>r' \<in> \<V> x\<^sub>s \<longrightarrow> \<V> x\<^sub>r' \<subseteq> \<V> x\<^sub>r \<and> \<V> (\<lfloor>e\<^sub>r\<rfloor>) \<subseteq> \<V> x \<and> (\<V>, \<C>) \<Turnstile>\<^sub>e e\<^sub>r"
+    with `^prim.Right x\<^sub>r' \<in> \<V> x\<^sub>s`
+    show "\<V> (\<lfloor>e\<^sub>r\<rfloor>) \<subseteq> \<V> x" by blast
+  qed
+
+  from `(\<V>, \<C>) \<Turnstile>\<^sub>\<sigma> \<langle>LET x = CASE x\<^sub>s LEFT x\<^sub>l |> e\<^sub>l RIGHT x\<^sub>r |> e\<^sub>r in e;\<rho>;\<kappa>\<rangle>`
+  show "(\<V>, \<C>) \<Turnstile>\<^sub>e e" by (blast intro: may_be_static_eval_state_to_exp_let)
+
+  from `(\<V>, \<C>) \<Turnstile>\<^sub>\<sigma> \<langle>LET x = CASE x\<^sub>s LEFT x\<^sub>l |> e\<^sub>l RIGHT x\<^sub>r |> e\<^sub>r in e;\<rho>;\<kappa>\<rangle>`
+  show "(\<V>, \<C>) \<Turnstile>\<^sub>\<rho> \<rho>" by (blast intro: may_be_static_eval_state.cases)
+
+  from `(\<V>, \<C>) \<Turnstile>\<^sub>\<sigma> \<langle>LET x = CASE x\<^sub>s LEFT x\<^sub>l |> e\<^sub>l RIGHT x\<^sub>r |> e\<^sub>r in e;\<rho>;\<kappa>\<rangle>`
+  show "(\<V>, \<C>) \<Turnstile>\<^sub>\<kappa> \<V> (\<lfloor>e\<rfloor>) \<Rrightarrow> \<kappa>" by (blast intro: may_be_static_eval_state_to_stack_let)
+  
+qed
+
+lemma may_be_static_eval_state_to_state_let_case_right: "
+  (\<V>, \<C>) \<Turnstile>\<^sub>\<sigma> \<langle>LET x = CASE x\<^sub>s LEFT x\<^sub>l |> e\<^sub>l RIGHT x\<^sub>r |> e\<^sub>r in e; \<rho>; \<kappa>\<rangle> \<Longrightarrow> 
+  \<rho> x\<^sub>s = Some (VClosure (Right x\<^sub>r') \<rho>\<^sub>r) \<Longrightarrow> 
+  \<rho>\<^sub>r x\<^sub>r' = Some \<omega>\<^sub>r \<Longrightarrow> (\<V>, \<C>) \<Turnstile>\<^sub>\<sigma> \<langle>e\<^sub>r; \<rho>(x\<^sub>r \<mapsto> \<omega>\<^sub>r); \<langle>x,e,\<rho>\<rangle> # \<kappa>\<rangle>
+"
+proof
+  assume "(\<V>, \<C>) \<Turnstile>\<^sub>\<sigma> \<langle>LET x = CASE x\<^sub>s LEFT x\<^sub>l |> e\<^sub>l RIGHT x\<^sub>r |> e\<^sub>r in e; \<rho>; \<kappa>\<rangle>" and "\<rho> x\<^sub>s = Some (VClosure (Right x\<^sub>r') \<rho>\<^sub>r)" then
+  show "(\<V>, \<C>) \<Turnstile>\<^sub>e e\<^sub>r" by (simp add: may_be_static_eval_state_to_exp_let_case_right)
+
+  assume "\<rho>\<^sub>r x\<^sub>r' = Some \<omega>\<^sub>r"
+  with `(\<V>, \<C>) \<Turnstile>\<^sub>\<sigma> \<langle>LET x = CASE x\<^sub>s LEFT x\<^sub>l |> e\<^sub>l RIGHT x\<^sub>r |> e\<^sub>r in e; \<rho>; \<kappa>\<rangle>` and `\<rho> x\<^sub>s = Some (VClosure (Right x\<^sub>r') \<rho>\<^sub>r)` 
+  show "(\<V>, \<C>) \<Turnstile>\<^sub>\<rho> \<rho>(x\<^sub>r \<mapsto> \<omega>\<^sub>r)" by (simp add: may_be_static_eval_state_to_env_let_case_right)
+
+  from `\<rho>\<^sub>r x\<^sub>r' = Some \<omega>\<^sub>r`  
+  and `(\<V>, \<C>) \<Turnstile>\<^sub>\<sigma> \<langle>LET x = CASE x\<^sub>s LEFT x\<^sub>l |> e\<^sub>l RIGHT x\<^sub>r |> e\<^sub>r in e; \<rho>; \<kappa>\<rangle>` 
+  and `\<rho> x\<^sub>s = Some (VClosure (Right x\<^sub>r') \<rho>\<^sub>r)` 
+  show "(\<V>, \<C>) \<Turnstile>\<^sub>\<kappa> \<V> (\<lfloor>e\<^sub>r\<rfloor>) \<Rrightarrow> \<langle>x,e,\<rho>\<rangle> # \<kappa>" by (simp add: may_be_static_eval_state_to_stack_let_case_right)
+qed
+
+
+lemma may_be_static_eval_state_to_env_let_fst: "
+  (\<V>, \<C>) \<Turnstile>\<^sub>\<sigma> \<langle>LET x = FST x\<^sub>p in e; \<rho>; \<kappa>\<rangle> \<Longrightarrow> 
+  \<rho> x\<^sub>p = Some (VClosure (Pair x\<^sub>1 x\<^sub>2) \<rho>\<^sub>p) \<Longrightarrow> \<rho>\<^sub>p x\<^sub>1 = Some \<omega> \<Longrightarrow> 
+  (\<V>, \<C>) \<Turnstile>\<^sub>\<rho> \<rho>(x \<mapsto> \<omega>)
+"
+proof
+  assume "\<rho> x\<^sub>p = Some (VClosure (Pair x\<^sub>1 x\<^sub>2) \<rho>\<^sub>p)" and "\<rho>\<^sub>p x\<^sub>1 = Some \<omega>"
+  assume "(\<V>, \<C>) \<Turnstile>\<^sub>\<sigma> \<langle>LET x = FST x\<^sub>p in e; \<rho>; \<kappa>\<rangle>" then
+  have "(\<V>, \<C>) \<Turnstile>\<^sub>e LET x = FST x\<^sub>p in e" "(\<V>, \<C>) \<Turnstile>\<^sub>\<rho> \<rho>" by (simp add: may_be_static_eval_state.simps)+
+
+  thm may_be_static_eval_state.simps
+
+  from `(\<V>, \<C>) \<Turnstile>\<^sub>\<rho> \<rho>` `\<rho> x\<^sub>p = Some (VClosure (Pair x\<^sub>1 x\<^sub>2) \<rho>\<^sub>p)`
+  have "(\<V>, \<C>) \<Turnstile>\<^sub>\<omega> (VClosure (Pair x\<^sub>1 x\<^sub>2) \<rho>\<^sub>p)" by (blast intro: may_be_static_eval_env.cases) then
+  have "(\<V>, \<C>) \<Turnstile>\<^sub>\<rho> \<rho>\<^sub>p" by (blast intro: may_be_static_eval_value.cases)
+
+  from `(\<V>, \<C>) \<Turnstile>\<^sub>\<rho> \<rho>\<^sub>p` `\<rho>\<^sub>p x\<^sub>1 = Some \<omega>`
+  have "{|\<omega>|} \<subseteq> \<V> x\<^sub>1" "(\<V>, \<C>) \<Turnstile>\<^sub>\<omega> \<omega>" by (blast intro: may_be_static_eval_env.cases)+
+
+  from `(\<V>, \<C>) \<Turnstile>\<^sub>\<rho> \<rho>` `\<rho> x\<^sub>p = Some (VClosure (Pair x\<^sub>1 x\<^sub>2) \<rho>\<^sub>p)`
+  have " | (VClosure (Pair x\<^sub>1 x\<^sub>2) \<rho>\<^sub>p) | \<in> \<V> x\<^sub>p" by (blast intro: may_be_static_eval_env.cases) then
+  have "^prim.Pair x\<^sub>1 x\<^sub>2 \<in> \<V> x\<^sub>p" by simp
+
+  from  `(\<V>, \<C>) \<Turnstile>\<^sub>e LET x = FST x\<^sub>p in e`
+  have "\<V> x\<^sub>1 \<subseteq> \<V> x"
+  proof cases
+    case Let_Fst
+    from `\<forall>x\<^sub>1 x\<^sub>2. ^prim.Pair x\<^sub>1 x\<^sub>2 \<in> \<V> x\<^sub>p \<longrightarrow> \<V> x\<^sub>1 \<subseteq> \<V> x`
+    and `^prim.Pair x\<^sub>1 x\<^sub>2 \<in> \<V> x\<^sub>p`
+    show "\<V> x\<^sub>1 \<subseteq> \<V> x" by blast
+  qed
+
+  from `{|\<omega>|} \<subseteq> \<V> x\<^sub>1` `\<V> x\<^sub>1 \<subseteq> \<V> x` 
+  have "{|\<omega>|} \<subseteq> \<V> x" by blast
+
+  {
+    fix x' \<omega>'
+    assume "(\<rho>(x \<mapsto> \<omega>)) x' = Some \<omega>'" "x' \<noteq> x" then
+    have "\<rho> x' = Some \<omega>'" by simp
+    with `(\<V>, \<C>) \<Turnstile>\<^sub>\<rho> \<rho>` 
+    have "{|\<omega>'|} \<subseteq> \<V> x' \<and> (\<V>, \<C>) \<Turnstile>\<^sub>\<omega> \<omega>'" by (simp add: may_be_static_eval_env.simps)
+  }
+  with `{|\<omega>|} \<subseteq> \<V> x` `(\<V>, \<C>) \<Turnstile>\<^sub>\<omega> \<omega>`
+  show "\<forall>x' \<omega>'. (\<rho>(x \<mapsto> \<omega>)) x' = Some \<omega>' \<longrightarrow> {|\<omega>'|} \<subseteq> \<V> x' \<and> (\<V>, \<C>) \<Turnstile>\<^sub>\<omega> \<omega>'" by auto
+qed
+
+
+
+lemma may_be_static_eval_state_to_state_let_fst: "
+  (\<V>, \<C>) \<Turnstile>\<^sub>\<sigma> \<langle>LET x = FST x\<^sub>p in e; \<rho>; \<kappa>\<rangle> \<Longrightarrow>
+  \<rho> x\<^sub>p = Some (VClosure (Pair x\<^sub>1 x\<^sub>2) \<rho>\<^sub>p) \<Longrightarrow> \<rho>\<^sub>p x\<^sub>1 = Some \<omega> \<Longrightarrow> 
+  (\<V>, \<C>) \<Turnstile>\<^sub>\<sigma> \<langle>e; \<rho>(x \<mapsto> \<omega>); \<kappa>\<rangle>
+"
+proof
+  assume "(\<V>, \<C>) \<Turnstile>\<^sub>\<sigma> \<langle>LET x = FST x\<^sub>p in e; \<rho>; \<kappa>\<rangle>" then
+  show "(\<V>, \<C>) \<Turnstile>\<^sub>e e" by (simp add: may_be_static_eval_state_to_exp_let)
+
+  assume "\<rho> x\<^sub>p = Some (VClosure (Pair x\<^sub>1 x\<^sub>2) \<rho>\<^sub>p)" and "\<rho>\<^sub>p x\<^sub>1 = Some \<omega>"
+  with `(\<V>, \<C>) \<Turnstile>\<^sub>\<sigma> \<langle>LET x = FST x\<^sub>p in e; \<rho>; \<kappa>\<rangle>`
+  show "(\<V>, \<C>) \<Turnstile>\<^sub>\<rho> \<rho>(x \<mapsto> \<omega>)"  by (simp add: may_be_static_eval_state_to_env_let_fst)
+
+  from `\<rho> x\<^sub>p = Some (VClosure (Pair x\<^sub>1 x\<^sub>2) \<rho>\<^sub>p)` and `\<rho>\<^sub>p x\<^sub>1 = Some \<omega>`
+  and `(\<V>, \<C>) \<Turnstile>\<^sub>\<sigma> \<langle>LET x = FST x\<^sub>p in e; \<rho>; \<kappa>\<rangle>`
+  show "(\<V>, \<C>) \<Turnstile>\<^sub>\<kappa> \<V> (\<lfloor>e\<rfloor>) \<Rrightarrow> \<kappa>" by (simp add: may_be_static_eval_state_to_stack_let)
+qed
+
+
+lemma may_be_static_eval_state_to_env_let_snd: "
+  (\<V>, \<C>) \<Turnstile>\<^sub>\<sigma> \<langle>LET x = SND x\<^sub>p in e; \<rho>; \<kappa>\<rangle> \<Longrightarrow> \<rho> x\<^sub>p = Some (VClosure (Pair x\<^sub>1 x\<^sub>2) \<rho>\<^sub>p) \<Longrightarrow> \<rho>\<^sub>p x\<^sub>2 = Some \<omega> \<Longrightarrow> (\<V>, \<C>) \<Turnstile>\<^sub>\<rho> \<rho>(x \<mapsto> \<omega>)
+"
+proof
+  assume "\<rho> x\<^sub>p = Some (VClosure (Pair x\<^sub>1 x\<^sub>2) \<rho>\<^sub>p)" and "\<rho>\<^sub>p x\<^sub>2 = Some \<omega>"
+  assume "(\<V>, \<C>) \<Turnstile>\<^sub>\<sigma> \<langle>LET x = SND x\<^sub>p in e; \<rho>; \<kappa>\<rangle>" then
+  have "(\<V>, \<C>) \<Turnstile>\<^sub>e LET x = SND x\<^sub>p in e" "(\<V>, \<C>) \<Turnstile>\<^sub>\<rho> \<rho>" by (simp add: may_be_static_eval_state.simps)+
+
+  from `(\<V>, \<C>) \<Turnstile>\<^sub>\<rho> \<rho>` `\<rho> x\<^sub>p = Some (VClosure (Pair x\<^sub>1 x\<^sub>2) \<rho>\<^sub>p)`
+  have "(\<V>, \<C>) \<Turnstile>\<^sub>\<omega> (VClosure (Pair x\<^sub>1 x\<^sub>2) \<rho>\<^sub>p)" by (blast intro: may_be_static_eval_env.cases) then
+  have "(\<V>, \<C>) \<Turnstile>\<^sub>\<rho> \<rho>\<^sub>p" by (blast intro: may_be_static_eval_value.cases)
+
+  from `(\<V>, \<C>) \<Turnstile>\<^sub>\<rho> \<rho>\<^sub>p` `\<rho>\<^sub>p x\<^sub>2 = Some \<omega>`
+  have "{|\<omega>|} \<subseteq> \<V> x\<^sub>2" "(\<V>, \<C>) \<Turnstile>\<^sub>\<omega> \<omega>" by (blast intro: may_be_static_eval_env.cases)+
+
+  from `(\<V>, \<C>) \<Turnstile>\<^sub>\<rho> \<rho>` `\<rho> x\<^sub>p = Some (VClosure (Pair x\<^sub>1 x\<^sub>2) \<rho>\<^sub>p)`
+  have " | (VClosure (Pair x\<^sub>1 x\<^sub>2) \<rho>\<^sub>p) | \<in> \<V> x\<^sub>p" by (blast intro: may_be_static_eval_env.cases) then
+  have "^prim.Pair x\<^sub>1 x\<^sub>2 \<in> \<V> x\<^sub>p" by simp
+
+  from  `(\<V>, \<C>) \<Turnstile>\<^sub>e LET x = SND x\<^sub>p in e`
+  have "\<V> x\<^sub>2 \<subseteq> \<V> x"
+  proof cases
+    case Let_Snd
+    from `\<forall>x\<^sub>1 x\<^sub>2. ^prim.Pair x\<^sub>1 x\<^sub>2 \<in> \<V> x\<^sub>p \<longrightarrow> \<V> x\<^sub>2 \<subseteq> \<V> x`
+    and `^prim.Pair x\<^sub>1 x\<^sub>2 \<in> \<V> x\<^sub>p`
+    show "\<V> x\<^sub>2 \<subseteq> \<V> x" by blast
+  qed
+
+
+  from `{|\<omega>|} \<subseteq> \<V> x\<^sub>2` `\<V> x\<^sub>2 \<subseteq> \<V> x` 
+  have "{|\<omega>|} \<subseteq> \<V> x" by blast
+
+  {
+    fix x' \<omega>'
+    assume "(\<rho>(x \<mapsto> \<omega>)) x' = Some \<omega>'" "x' \<noteq> x" then
+    have "\<rho> x' = Some \<omega>'" by simp
+    with `(\<V>, \<C>) \<Turnstile>\<^sub>\<rho> \<rho>` 
+    have "{|\<omega>'|} \<subseteq> \<V> x' \<and> (\<V>, \<C>) \<Turnstile>\<^sub>\<omega> \<omega>'" by (simp add: may_be_static_eval_env.simps)
+  }
+  with \<open>{|\<omega>|} \<subseteq> \<V> x\<close> \<open>(\<V>, \<C>) \<Turnstile>\<^sub>\<omega> \<omega>\<close> 
+  show "\<forall>x' \<omega>'. (\<rho>(x \<mapsto> \<omega>)) x' = Some \<omega>' \<longrightarrow> {|\<omega>'|} \<subseteq> \<V> x' \<and> (\<V>, \<C>) \<Turnstile>\<^sub>\<omega> \<omega>'" by simp
+qed
+
+
+lemma may_be_static_eval_state_to_state_let_snd: "
+  (\<V>, \<C>) \<Turnstile>\<^sub>\<sigma> \<langle>LET x = SND x\<^sub>p in e; \<rho>; \<kappa>\<rangle> \<Longrightarrow>
+  \<rho> x\<^sub>p = Some (VClosure (Pair x\<^sub>1 x\<^sub>2) \<rho>\<^sub>p) \<Longrightarrow> \<rho>\<^sub>p x\<^sub>2 = Some \<omega> \<Longrightarrow> 
+  (\<V>, \<C>) \<Turnstile>\<^sub>\<sigma> \<langle>e; \<rho>(x \<mapsto> \<omega>); \<kappa>\<rangle>
+"
+proof
+  assume "(\<V>, \<C>) \<Turnstile>\<^sub>\<sigma> \<langle>LET x = SND x\<^sub>p in e; \<rho>; \<kappa>\<rangle>" then
+  show "(\<V>, \<C>) \<Turnstile>\<^sub>e e" by (simp add: may_be_static_eval_state_to_exp_let)
+
+  assume "\<rho> x\<^sub>p = Some (VClosure (Pair x\<^sub>1 x\<^sub>2) \<rho>\<^sub>p)" and "\<rho>\<^sub>p x\<^sub>2 = Some \<omega>"
+  with `(\<V>, \<C>) \<Turnstile>\<^sub>\<sigma> \<langle>LET x = SND x\<^sub>p in e; \<rho>; \<kappa>\<rangle>`
+  show "(\<V>, \<C>) \<Turnstile>\<^sub>\<rho> \<rho>(x \<mapsto> \<omega>)" by (simp add: may_be_static_eval_state_to_env_let_snd)
+
+  from `\<rho> x\<^sub>p = Some (VClosure (Pair x\<^sub>1 x\<^sub>2) \<rho>\<^sub>p)` and `\<rho>\<^sub>p x\<^sub>2 = Some \<omega>`
+  and `(\<V>, \<C>) \<Turnstile>\<^sub>\<sigma> \<langle>LET x = SND x\<^sub>p in e; \<rho>; \<kappa>\<rangle>`
+  show "(\<V>, \<C>) \<Turnstile>\<^sub>\<kappa> \<V> (\<lfloor>e\<rfloor>) \<Rrightarrow> \<kappa>" by (simp add: may_be_static_eval_state_to_stack_let)
+qed
+
+
+lemma may_be_static_eval_state_to_env_let_app: "
+  (\<V>, \<C>) \<Turnstile>\<^sub>\<sigma> \<langle>LET x = APP f x\<^sub>a in e; \<rho>; \<kappa>\<rangle> \<Longrightarrow> 
+  \<rho> f = Some (VClosure (Abs f\<^sub>l x\<^sub>l e\<^sub>l) \<rho>\<^sub>l) \<Longrightarrow> \<rho> x\<^sub>a = Some \<omega>\<^sub>a \<Longrightarrow> 
+  (\<V>, \<C>) \<Turnstile>\<^sub>\<rho> \<rho>\<^sub>l(f\<^sub>l \<mapsto> (VClosure (Abs f\<^sub>l x\<^sub>l e\<^sub>l) \<rho>\<^sub>l), x\<^sub>l \<mapsto> \<omega>\<^sub>a)
+"
+proof
+  assume "\<rho> f = Some (VClosure (Abs f\<^sub>l x\<^sub>l e\<^sub>l) \<rho>\<^sub>l)" "\<rho> x\<^sub>a = Some \<omega>\<^sub>a"
+  assume "(\<V>, \<C>) \<Turnstile>\<^sub>\<sigma> \<langle>LET x = APP f x\<^sub>a in e; \<rho>; \<kappa>\<rangle>" then
+  have "(\<V>, \<C>) \<Turnstile>\<^sub>e LET x = APP f x\<^sub>a in e" "(\<V>, \<C>) \<Turnstile>\<^sub>\<rho> \<rho>" by (simp add: may_be_static_eval_state.simps)+
+
+  from `(\<V>, \<C>) \<Turnstile>\<^sub>\<rho> \<rho>` and `\<rho> x\<^sub>a = Some \<omega>\<^sub>a`
+  have "{|\<omega>\<^sub>a|} \<subseteq> \<V> x\<^sub>a" "(\<V>, \<C>) \<Turnstile>\<^sub>\<omega> \<omega>\<^sub>a" by (blast intro: may_be_static_eval_env.cases)+
+
+  from `(\<V>, \<C>) \<Turnstile>\<^sub>\<rho> \<rho>` and `\<rho> f = Some (VClosure (Abs f\<^sub>l x\<^sub>l e\<^sub>l) \<rho>\<^sub>l)`
+  have "{|(VClosure (Abs f\<^sub>l x\<^sub>l e\<^sub>l) \<rho>\<^sub>l)|} \<subseteq> \<V> f" "(\<V>, \<C>) \<Turnstile>\<^sub>\<omega> (VClosure (Abs f\<^sub>l x\<^sub>l e\<^sub>l) \<rho>\<^sub>l)" by (blast intro: may_be_static_eval_env.cases)+
+
+  from `{|(VClosure (Abs f\<^sub>l x\<^sub>l e\<^sub>l) \<rho>\<^sub>l)|} \<subseteq> \<V> f`
+  have "^Abs f\<^sub>l x\<^sub>l e\<^sub>l \<in> \<V> f" by simp
+
+  from `(\<V>, \<C>) \<Turnstile>\<^sub>\<omega> (VClosure (Abs f\<^sub>l x\<^sub>l e\<^sub>l) \<rho>\<^sub>l)`
+  have "{|(VClosure (Abs f\<^sub>l x\<^sub>l e\<^sub>l) \<rho>\<^sub>l)|} \<subseteq> \<V> f\<^sub>l" "(\<V>, \<C>) \<Turnstile>\<^sub>\<rho> \<rho>\<^sub>l" by (rule may_be_static_eval_value.cases; auto)+
+
+
+  with `(\<V>, \<C>) \<Turnstile>\<^sub>e LET x = APP f x\<^sub>a in e`
+  have "\<V> x\<^sub>a \<subseteq> \<V> x\<^sub>l"
+  proof cases
+    case Let_App
+    assume "\<forall>f' x' e'. ^Abs f' x' e' \<in> \<V> f \<longrightarrow> \<V> x\<^sub>a \<subseteq> \<V> x' \<and> \<V> (\<lfloor>e'\<rfloor>) \<subseteq> \<V> x"
+    with `^Abs f\<^sub>l x\<^sub>l e\<^sub>l \<in> \<V> f`
+    show "\<V> x\<^sub>a \<subseteq> \<V> x\<^sub>l" by blast
+  qed
+
+  from `{|\<omega>\<^sub>a|} \<subseteq> \<V> x\<^sub>a` `\<V> x\<^sub>a \<subseteq> \<V> x\<^sub>l`
+  have "{|\<omega>\<^sub>a|} \<subseteq> \<V> x\<^sub>l" by blast
+
+
+  {
+    fix x' \<omega>'
+    assume "(\<rho>\<^sub>l(f\<^sub>l \<mapsto> (VClosure (Abs f\<^sub>l x\<^sub>l e\<^sub>l) \<rho>\<^sub>l), x\<^sub>l \<mapsto> \<omega>\<^sub>a)) x' = Some \<omega>'" "x' \<noteq> x\<^sub>l" "x' \<noteq> f\<^sub>l" then
+    have "\<rho>\<^sub>l x' = Some \<omega>'" by simp
+    with `(\<V>, \<C>) \<Turnstile>\<^sub>\<rho> \<rho>\<^sub>l` 
+    have "{|\<omega>'|} \<subseteq> \<V> x' \<and> (\<V>, \<C>) \<Turnstile>\<^sub>\<omega> \<omega>'" by (simp add: may_be_static_eval_env.simps)
+  }
+  with \<open>{|(VClosure (Abs f\<^sub>l x\<^sub>l e\<^sub>l) \<rho>\<^sub>l)|} \<subseteq> \<V> f\<^sub>l\<close> \<open>(\<V>, \<C>) \<Turnstile>\<^sub>\<omega> (VClosure (Abs f\<^sub>l x\<^sub>l e\<^sub>l) \<rho>\<^sub>l)\<close> \<open>(\<V>, \<C>) \<Turnstile>\<^sub>\<omega> \<omega>\<^sub>a\<close> \<open>{|\<omega>\<^sub>a|} \<subseteq> \<V> x\<^sub>l\<close>
+  show "\<forall>x \<omega>. (\<rho>\<^sub>l(f\<^sub>l \<mapsto> (VClosure (Abs f\<^sub>l x\<^sub>l e\<^sub>l) \<rho>\<^sub>l), x\<^sub>l \<mapsto> \<omega>\<^sub>a)) x = Some \<omega> \<longrightarrow> {|\<omega>|} \<subseteq> \<V> x \<and> (\<V>, \<C>) \<Turnstile>\<^sub>\<omega> \<omega>" by auto
+
+qed
+
+lemma may_be_static_eval_state_to_stack_let_app: "
+  (\<V>, \<C>) \<Turnstile>\<^sub>\<sigma> \<langle>LET x = APP f x\<^sub>a in e; \<rho>; \<kappa>\<rangle> \<Longrightarrow> 
+  \<rho> f = Some (VClosure (Abs f' x\<^sub>p e\<^sub>b) \<rho>') \<Longrightarrow> \<rho> x\<^sub>a = Some \<omega>\<^sub>a \<Longrightarrow> 
+  (\<V>, \<C>) \<Turnstile>\<^sub>\<kappa> \<V> (\<lfloor>e\<^sub>b\<rfloor>) \<Rrightarrow> \<langle>x,e,\<rho>\<rangle> # \<kappa>
+"
+proof
+  assume "\<rho> f = Some (VClosure (Abs f' x\<^sub>p e\<^sub>b) \<rho>')" and "\<rho> x\<^sub>a = Some \<omega>\<^sub>a"
+  assume "(\<V>, \<C>) \<Turnstile>\<^sub>\<sigma> \<langle>LET x = APP f x\<^sub>a in e; \<rho>; \<kappa>\<rangle>" then
+  have "(\<V>, \<C>) \<Turnstile>\<^sub>e LET x = APP f x\<^sub>a in e"  "(\<V>, \<C>) \<Turnstile>\<^sub>\<rho> \<rho>" by (blast intro: may_be_static_eval_state.cases)+
+
+  from `(\<V>, \<C>) \<Turnstile>\<^sub>\<rho> \<rho>` and `\<rho> f = Some (VClosure (Abs f' x\<^sub>p e\<^sub>b) \<rho>')`
+  have " {|(VClosure (Abs f' x\<^sub>p e\<^sub>b) \<rho>')|} \<subseteq> \<V> f" by (blast intro: may_be_static_eval_env.cases) then
+  have " ^Abs f' x\<^sub>p e\<^sub>b \<in> \<V> f" by simp
+
+  from `(\<V>, \<C>) \<Turnstile>\<^sub>e LET x = APP f x\<^sub>a in e`
+  show " \<V> (\<lfloor>e\<^sub>b\<rfloor>) \<subseteq> \<V> x"
+  proof cases
+    case Let_App
+    assume "\<forall>f' x' e'. ^Abs f' x' e' \<in> \<V> f \<longrightarrow> \<V> x\<^sub>a \<subseteq> \<V> x' \<and> \<V> (\<lfloor>e'\<rfloor>) \<subseteq> \<V> x"
+    with `^Abs f' x\<^sub>p e\<^sub>b \<in> \<V> f`
+    show " \<V> (\<lfloor>e\<^sub>b\<rfloor>) \<subseteq> \<V> x" by simp
+  qed
+
+  from `(\<V>, \<C>) \<Turnstile>\<^sub>\<sigma> \<langle>LET x = APP f x\<^sub>a in e; \<rho>; \<kappa>\<rangle>`
+  show "(\<V>, \<C>) \<Turnstile>\<^sub>e e" by (blast intro: may_be_static_eval_state_to_exp_let)
+
+  from `(\<V>, \<C>) \<Turnstile>\<^sub>\<sigma> \<langle>LET x = APP f x\<^sub>a in e; \<rho>; \<kappa>\<rangle>`
+  show "(\<V>, \<C>) \<Turnstile>\<^sub>\<rho> \<rho>" by (blast intro: may_be_static_eval_state.cases)
+
+  from `(\<V>, \<C>) \<Turnstile>\<^sub>\<sigma> \<langle>LET x = APP f x\<^sub>a in e; \<rho>; \<kappa>\<rangle>`
+  show "(\<V>, \<C>) \<Turnstile>\<^sub>\<kappa> \<V> (\<lfloor>e\<rfloor>) \<Rrightarrow> \<kappa>" by (blast intro: may_be_static_eval_state_to_stack_let)
+qed
+
+
+theorem may_be_static_eval_state_preserved_under_step : "
+  \<lbrakk>
+    (\<V>, \<C>) \<Turnstile>\<^sub>\<sigma> \<langle>LET x = b in e; \<rho>; \<kappa>\<rangle>; 
+    seq_step (b, \<rho>) \<omega>
+  \<rbrakk> \<Longrightarrow>
+  (\<V>, \<C>) \<Turnstile>\<^sub>\<sigma> \<langle>e;\<rho>(x \<mapsto> \<omega>);\<kappa>\<rangle>
+"
+proof -
+  assume 
+    H1: "(\<V>, \<C>) \<Turnstile>\<^sub>\<sigma> \<langle>LET x = b in e; \<rho>; \<kappa>\<rangle>" and
+    H2: "seq_step (b, \<rho>) \<omega>"
+    
+  from H2 show "(\<V>, \<C>) \<Turnstile>\<^sub>\<sigma> \<langle>e;\<rho>(x \<mapsto> \<omega>);\<kappa>\<rangle>"
+  proof cases
+    case Let_Unit
+    
+    assume
+      H3: "b = \<lparr>\<rparr>" and
+      H4: "\<omega> = VUnit"
+
+    from H1 H3 have "(\<V>, \<C>) \<Turnstile>\<^sub>\<sigma> \<langle>LET x = \<lparr>\<rparr> in e; \<rho>; \<kappa>\<rangle>" by simp
+
+    then have "(\<V>, \<C>) \<Turnstile>\<^sub>\<sigma> \<langle>e; \<rho> ++ [x \<mapsto> VUnit]; \<kappa>\<rangle>" by (simp add: may_be_static_eval_state_to_state_let_unit)
+    
+    with H4 show "(\<V>, \<C>) \<Turnstile>\<^sub>\<sigma> \<langle>e;\<rho>(x \<mapsto> \<omega>);\<kappa>\<rangle>" by simp
+  next
+    case (Let_Prim p)
+
+    assume
+      H3: "b = Prim p" and
+      H4: "\<omega> = VClosure p \<rho>"
+
+    from H1 H3 have "(\<V>, \<C>) \<Turnstile>\<^sub>\<sigma> \<langle>LET x = Prim p in e; \<rho>; \<kappa>\<rangle>" by simp
+
+    then have "(\<V>, \<C>) \<Turnstile>\<^sub>\<sigma> \<langle>e; \<rho> ++ [x \<mapsto> VClosure p \<rho>]; \<kappa>\<rangle>" by (simp add: may_be_static_eval_state_to_state_let_prim)
+    
+    with H4 show "(\<V>, \<C>) \<Turnstile>\<^sub>\<sigma> \<langle>e;\<rho>(x \<mapsto> \<omega>);\<kappa>\<rangle>" by simp
+  next
+    case (Let_Fst x\<^sub>p x\<^sub>1 x\<^sub>2 \<rho>\<^sub>p)
+
+    assume 
+      H3: "b = FST x\<^sub>p" and
+      H4: "\<rho> x\<^sub>p = Some (VClosure (prim.Pair x\<^sub>1 x\<^sub>2) \<rho>\<^sub>p)" and
+      H5: "\<rho>\<^sub>p x\<^sub>1 = Some \<omega>"
+
+    from H1 H3 have "(\<V>, \<C>) \<Turnstile>\<^sub>\<sigma> \<langle>LET x = FST x\<^sub>p in e; \<rho>; \<kappa>\<rangle>" by simp
+
+    with H4 H5 show "(\<V>, \<C>) \<Turnstile>\<^sub>\<sigma> \<langle>e; \<rho>(x \<mapsto> \<omega>); \<kappa>\<rangle>" by (simp add: may_be_static_eval_state_to_state_let_fst)
+  next
+    case (Let_Snd x\<^sub>p x\<^sub>1 x\<^sub>2 \<rho>\<^sub>p)
+
+    assume 
+      H3: "b = SND x\<^sub>p" and
+      H4: "\<rho> x\<^sub>p = Some (VClosure (prim.Pair x\<^sub>1 x\<^sub>2) \<rho>\<^sub>p)" and
+      H5: "\<rho>\<^sub>p x\<^sub>2 = Some \<omega>"
+
+    from H1 H3 have "(\<V>, \<C>) \<Turnstile>\<^sub>\<sigma> \<langle>LET x = SND x\<^sub>p in e; \<rho>; \<kappa>\<rangle>" by simp
+
+    with H4 H5 show "(\<V>, \<C>) \<Turnstile>\<^sub>\<sigma> \<langle>e; \<rho>(x \<mapsto> \<omega>); \<kappa>\<rangle>" by (simp add: may_be_static_eval_state_to_state_let_snd)
+  qed
+qed
+
+theorem may_be_static_eval_state_preserved_under_step_up : "
+  \<lbrakk>
+    (\<V>, \<C>) \<Turnstile>\<^sub>\<sigma> \<langle>LET x = b in e; \<rho>; \<kappa>\<rangle>;
+    seq_step_up (b, \<rho>) (e', \<rho>')
+  \<rbrakk> \<Longrightarrow>
+  (\<V>, \<C>) \<Turnstile>\<^sub>\<sigma> \<langle>e'; \<rho>'; \<langle>x,e,\<rho>\<rangle> # \<kappa>\<rangle>
+"
+proof -
+  assume 
+    H1: "(\<V>, \<C>) \<Turnstile>\<^sub>\<sigma> \<langle>LET x = b in e; \<rho>; \<kappa>\<rangle>" and
+    H2: "seq_step_up (b, \<rho>) (e', \<rho>')"
+
+  from H2 show "(\<V>, \<C>) \<Turnstile>\<^sub>\<sigma> \<langle>e'; \<rho>'; \<langle>x,e,\<rho>\<rangle> # \<kappa>\<rangle>" 
+  proof cases
+    case (Let_Case_Left x\<^sub>s x\<^sub>l' \<rho>\<^sub>l \<omega>\<^sub>l x\<^sub>l x\<^sub>r e\<^sub>r)
+
+    assume 
+      H3: "b = CASE x\<^sub>s LEFT x\<^sub>l |> e' RIGHT x\<^sub>r |> e\<^sub>r" and
+      H4: "\<rho>' = \<rho>(x\<^sub>l \<mapsto> \<omega>\<^sub>l)" and
+      H5: "\<rho> x\<^sub>s = Some (VClosure (prim.Left x\<^sub>l') \<rho>\<^sub>l)" and
+      H6: "\<rho>\<^sub>l x\<^sub>l' = Some \<omega>\<^sub>l"
+
+    from H1 H3 H4 H5 H6
+    show "(\<V>, \<C>) \<Turnstile>\<^sub>\<sigma> \<langle>e'; \<rho>'; \<langle>x,e,\<rho>\<rangle> # \<kappa>\<rangle>" by (simp add: may_be_static_eval_state_to_state_let_case_left)
+  next
+    case (Let_Case_Right x\<^sub>s x\<^sub>r' \<rho>\<^sub>r \<omega>\<^sub>r x\<^sub>l e\<^sub>l x\<^sub>r)
+
+    assume 
+      H3: "b = CASE x\<^sub>s LEFT x\<^sub>l |> e\<^sub>l RIGHT x\<^sub>r |> e'" and
+      H4: "\<rho>' = \<rho>(x\<^sub>r \<mapsto> \<omega>\<^sub>r)" and
+      H5: "\<rho> x\<^sub>s = Some (VClosure (prim.Right x\<^sub>r') \<rho>\<^sub>r)" and
+      H6: "\<rho>\<^sub>r x\<^sub>r' = Some \<omega>\<^sub>r"
+
+    from H1 H3 H4 H5 H6
+    show "(\<V>, \<C>) \<Turnstile>\<^sub>\<sigma> \<langle>e'; \<rho>'; \<langle>x,e,\<rho>\<rangle> # \<kappa>\<rangle>" by (simp add: may_be_static_eval_state_to_state_let_case_right)
+  next
+    case (Let_App f f\<^sub>l x\<^sub>l \<rho>\<^sub>l x\<^sub>a \<omega>\<^sub>l)
+    assume
+      H3: "b = APP f x\<^sub>a" and
+      H4: "\<rho>' = \<rho>\<^sub>l(f\<^sub>l \<mapsto> VClosure (Abs f\<^sub>l x\<^sub>l e') \<rho>\<^sub>l, x\<^sub>l \<mapsto> \<omega>\<^sub>l)" and
+      H5: "\<rho> f = Some (VClosure (Abs f\<^sub>l x\<^sub>l e') \<rho>\<^sub>l)" and
+      H6: "\<rho> x\<^sub>a = Some \<omega>\<^sub>l"
+
+    have H7: "(\<V>, \<C>) \<Turnstile>\<^sub>e e'" using H1 H3 H5 may_be_static_eval_state_to_exp_let_app by auto
+  
+    have "(\<V>, \<C>) \<Turnstile>\<^sub>\<rho> \<rho>\<^sub>l(f\<^sub>l \<mapsto> (VClosure (Abs f\<^sub>l x\<^sub>l e') \<rho>\<^sub>l), x\<^sub>l \<mapsto> \<omega>\<^sub>l)" using H1 H3 H5 H6 may_be_static_eval_state_to_env_let_app by auto
+
+    with H4 have H8: "(\<V>, \<C>) \<Turnstile>\<^sub>\<rho> \<rho>'" by simp
+  
+    have H9: "(\<V>, \<C>) \<Turnstile>\<^sub>\<kappa> \<V> (\<lfloor>e'\<rfloor>) \<Rrightarrow> \<langle>x,e,\<rho>\<rangle> # \<kappa>"  using H1 H3 H5 H6 may_be_static_eval_state_to_stack_let_app by auto
+  
+    from H7 H8 H9
+    show "(\<V>, \<C>) \<Turnstile>\<^sub>\<sigma> \<langle>e'; \<rho>'; \<langle>x,e,\<rho>\<rangle> # \<kappa>\<rangle>" by (simp add: may_be_static_eval_state.intros)
+  qed
+qed
+
+theorem may_be_static_eval_state_preserved_under_step_down : "
+  \<lbrakk>
+    (\<V>, \<C>) \<Turnstile>\<^sub>\<sigma> \<langle>RESULT x; \<rho>; \<langle>x\<^sub>\<kappa>, e\<^sub>\<kappa>, \<rho>\<^sub>\<kappa>\<rangle> # \<kappa>\<rangle>; 
+    \<rho> x = Some \<omega>
+  \<rbrakk> \<Longrightarrow>
+  (\<V>, \<C>) \<Turnstile>\<^sub>\<sigma> \<langle>e\<^sub>\<kappa>;\<rho>\<^sub>\<kappa> ++ [x\<^sub>\<kappa> \<mapsto> \<omega>];\<kappa>\<rangle>
+"
+proof -
+  assume 
+    H1: "(\<V>, \<C>) \<Turnstile>\<^sub>\<sigma> \<langle>RESULT x; \<rho>; \<langle>x\<^sub>\<kappa>, e\<^sub>\<kappa>, \<rho>\<^sub>\<kappa>\<rangle> # \<kappa>\<rangle>" and
+    H2: "\<rho> x = Some \<omega>"
+
+  from H1 H2
+  show "(\<V>, \<C>) \<Turnstile>\<^sub>\<sigma> \<langle>e\<^sub>\<kappa>;\<rho>\<^sub>\<kappa> ++ [x\<^sub>\<kappa> \<mapsto> \<omega>];\<kappa>\<rangle>" by (auto simp: may_be_static_eval_state_to_state_result)
+qed
+
+lemma may_be_static_eval_pool_to_exp_let: "
+  (\<V>, \<C>) \<Turnstile>\<^sub>\<E> \<E> \<Longrightarrow>
+  \<E> \<pi> = Some (\<langle>LET x = b in e; \<rho>; \<kappa>\<rangle>) \<Longrightarrow>
+  (\<V>, \<C>) \<Turnstile>\<^sub>e e
+"
+proof -
+ assume "(\<V>, \<C>) \<Turnstile>\<^sub>\<E> \<E>" and "\<E> \<pi> = Some (\<langle>LET x = b in e; \<rho>; \<kappa>\<rangle>)" then
+ have "(\<V>, \<C>) \<Turnstile>\<^sub>\<sigma> \<langle>LET x = b in e; \<rho>; \<kappa>\<rangle>" by (simp add: may_be_static_eval_pool.simps) then
+ show "(\<V>, \<C>) \<Turnstile>\<^sub>e e " by (blast intro: may_be_static_eval_state_to_exp_let)
+qed
+
+
+lemma may_be_static_eval_pool_let_sync_send_values_relate: "
+  (\<V>, \<C>) \<Turnstile>\<^sub>\<E> \<E> \<Longrightarrow>
+  \<E> \<pi>\<^sub>s = Some (\<langle>LET x\<^sub>s = SYNC x\<^sub>s\<^sub>e in e\<^sub>s; \<rho>\<^sub>s; \<kappa>\<^sub>s\<rangle>) \<Longrightarrow>
+  \<rho>\<^sub>s x\<^sub>s\<^sub>e = Some (VClosure (Send_Evt x\<^sub>s\<^sub>c x\<^sub>m) \<rho>\<^sub>s\<^sub>e) \<Longrightarrow>
+  \<rho>\<^sub>s\<^sub>e x\<^sub>s\<^sub>c = Some (VChan (Ch \<pi>\<^sub>c x\<^sub>c)) \<Longrightarrow>
+  {^\<lparr>\<rparr>} \<subseteq> \<V> x\<^sub>s \<and> \<V> x\<^sub>m \<subseteq> \<C> x\<^sub>c
+"
+proof -
+  assume "(\<V>, \<C>) \<Turnstile>\<^sub>\<E> \<E>"
+  and "\<E> \<pi>\<^sub>s = Some (\<langle>LET x\<^sub>s = SYNC x\<^sub>s\<^sub>e in e\<^sub>s; \<rho>\<^sub>s; \<kappa>\<^sub>s\<rangle>)"
+  and "\<rho>\<^sub>s x\<^sub>s\<^sub>e = Some (VClosure (Send_Evt x\<^sub>s\<^sub>c x\<^sub>m) \<rho>\<^sub>s\<^sub>e)"
+  and "\<rho>\<^sub>s\<^sub>e x\<^sub>s\<^sub>c = Some (VChan (Ch \<pi>\<^sub>c x\<^sub>c))"
+
+  from `(\<V>, \<C>) \<Turnstile>\<^sub>\<E> \<E>` and `\<E> \<pi>\<^sub>s = Some (\<langle>LET x\<^sub>s = SYNC x\<^sub>s\<^sub>e in e\<^sub>s; \<rho>\<^sub>s; \<kappa>\<^sub>s\<rangle>)`
+  have "(\<V>, \<C>) \<Turnstile>\<^sub>\<sigma> \<langle>LET x\<^sub>s = SYNC x\<^sub>s\<^sub>e in e\<^sub>s; \<rho>\<^sub>s; \<kappa>\<^sub>s\<rangle>" by (simp add: may_be_static_eval_pool.simps) then
+  have "(\<V>, \<C>) \<Turnstile>\<^sub>e LET x\<^sub>s = SYNC x\<^sub>s\<^sub>e in e\<^sub>s" "(\<V>, \<C>) \<Turnstile>\<^sub>\<rho> \<rho>\<^sub>s" by (simp add: may_be_static_eval_state.simps)+
+
+  from `(\<V>, \<C>) \<Turnstile>\<^sub>\<rho> \<rho>\<^sub>s` and `\<rho>\<^sub>s x\<^sub>s\<^sub>e = Some (VClosure (Send_Evt x\<^sub>s\<^sub>c x\<^sub>m) \<rho>\<^sub>s\<^sub>e)`
+  have "{|(VClosure (Send_Evt x\<^sub>s\<^sub>c x\<^sub>m) \<rho>\<^sub>s\<^sub>e)|} \<subseteq> \<V> x\<^sub>s\<^sub>e" and "(\<V>, \<C>) \<Turnstile>\<^sub>\<omega> (VClosure (Send_Evt x\<^sub>s\<^sub>c x\<^sub>m) \<rho>\<^sub>s\<^sub>e)" by (blast intro: may_be_static_eval_env.cases)+
+
+  from `{|(VClosure (Send_Evt x\<^sub>s\<^sub>c x\<^sub>m) \<rho>\<^sub>s\<^sub>e)|} \<subseteq> \<V> x\<^sub>s\<^sub>e`
+  have "^Send_Evt x\<^sub>s\<^sub>c x\<^sub>m \<in> \<V> x\<^sub>s\<^sub>e" by simp
+
+  from `(\<V>, \<C>) \<Turnstile>\<^sub>\<omega> (VClosure (Send_Evt x\<^sub>s\<^sub>c x\<^sub>m) \<rho>\<^sub>s\<^sub>e)`
+  have "(\<V>, \<C>) \<Turnstile>\<^sub>\<rho> \<rho>\<^sub>s\<^sub>e" by (blast intro: may_be_static_eval_value.cases)
+  with `\<rho>\<^sub>s\<^sub>e x\<^sub>s\<^sub>c = Some (VChan (Ch \<pi>\<^sub>c x\<^sub>c))`
+  have "{|(VChan (Ch \<pi>\<^sub>c x\<^sub>c))|} \<subseteq> \<V> x\<^sub>s\<^sub>c" by (blast intro: may_be_static_eval_env.cases) then
+  have "{^Chan x\<^sub>c} \<subseteq> \<V> x\<^sub>s\<^sub>c" by simp then
+  have "^Chan x\<^sub>c \<in> \<V> x\<^sub>s\<^sub>c" by auto
+  
+  from `(\<V>, \<C>) \<Turnstile>\<^sub>e LET x\<^sub>s = SYNC x\<^sub>s\<^sub>e in e\<^sub>s`
+  show "{^\<lparr>\<rparr>} \<subseteq> \<V> x\<^sub>s \<and> \<V> x\<^sub>m \<subseteq> \<C> x\<^sub>c"
+  proof cases
+    case Let_Sync
+    assume "\<forall>x\<^sub>s\<^sub>c x\<^sub>m x\<^sub>c. ^Send_Evt x\<^sub>s\<^sub>c x\<^sub>m \<in> \<V> x\<^sub>s\<^sub>e \<longrightarrow> ^Chan x\<^sub>c \<in> \<V> x\<^sub>s\<^sub>c \<longrightarrow> {^\<lparr>\<rparr>} \<subseteq> \<V> x\<^sub>s \<and> \<V> x\<^sub>m \<subseteq> \<C> x\<^sub>c"
+    with `^Send_Evt x\<^sub>s\<^sub>c x\<^sub>m \<in> \<V> x\<^sub>s\<^sub>e` and `^Chan x\<^sub>c \<in> \<V> x\<^sub>s\<^sub>c`
+    show "{^\<lparr>\<rparr>} \<subseteq> \<V> x\<^sub>s \<and> \<V> x\<^sub>m \<subseteq> \<C> x\<^sub>c" by blast
+  qed
+
+qed
+
+lemma may_be_static_eval_pool_let_sync_send_message_relate: "
+  (\<V>, \<C>) \<Turnstile>\<^sub>\<E> \<E> \<Longrightarrow>
+  \<E> \<pi>\<^sub>s = Some (\<langle>LET x\<^sub>s = SYNC x\<^sub>s\<^sub>e in e\<^sub>s; \<rho>\<^sub>s; \<kappa>\<^sub>s\<rangle>) \<Longrightarrow>
+  \<rho>\<^sub>s x\<^sub>s\<^sub>e = Some (VClosure (Send_Evt x\<^sub>s\<^sub>c x\<^sub>m) \<rho>\<^sub>s\<^sub>e) \<Longrightarrow>
+  \<rho>\<^sub>s\<^sub>e x\<^sub>m = Some \<omega>\<^sub>m \<Longrightarrow>
+  {|\<omega>\<^sub>m|} \<subseteq> \<V> x\<^sub>m \<and> (\<V>, \<C>) \<Turnstile>\<^sub>\<omega> \<omega>\<^sub>m
+"
+proof -
+  assume "(\<V>, \<C>) \<Turnstile>\<^sub>\<E> \<E>"
+  and "\<E> \<pi>\<^sub>s = Some (\<langle>LET x\<^sub>s = SYNC x\<^sub>s\<^sub>e in e\<^sub>s; \<rho>\<^sub>s; \<kappa>\<^sub>s\<rangle>)"
+  and "\<rho>\<^sub>s x\<^sub>s\<^sub>e = Some (VClosure (Send_Evt x\<^sub>s\<^sub>c x\<^sub>m) \<rho>\<^sub>s\<^sub>e)"
+  and "\<rho>\<^sub>s\<^sub>e x\<^sub>m = Some \<omega>\<^sub>m"
+
+  from `(\<V>, \<C>) \<Turnstile>\<^sub>\<E> \<E>` and `\<E> \<pi>\<^sub>s = Some (\<langle>LET x\<^sub>s = SYNC x\<^sub>s\<^sub>e in e\<^sub>s; \<rho>\<^sub>s; \<kappa>\<^sub>s\<rangle>)`
+  have "(\<V>, \<C>) \<Turnstile>\<^sub>\<sigma> \<langle>LET x\<^sub>s = SYNC x\<^sub>s\<^sub>e in e\<^sub>s; \<rho>\<^sub>s; \<kappa>\<^sub>s\<rangle>" by (simp add: may_be_static_eval_pool.simps) then
+  have "(\<V>, \<C>) \<Turnstile>\<^sub>\<rho> \<rho>\<^sub>s" by (simp add: may_be_static_eval_state.simps)
+  with `\<rho>\<^sub>s x\<^sub>s\<^sub>e = Some (VClosure (Send_Evt x\<^sub>s\<^sub>c x\<^sub>m) \<rho>\<^sub>s\<^sub>e)`
+  have "(\<V>, \<C>) \<Turnstile>\<^sub>\<omega> (VClosure (Send_Evt x\<^sub>s\<^sub>c x\<^sub>m) \<rho>\<^sub>s\<^sub>e)" by (blast intro: may_be_static_eval_env.cases) then
+  have "(\<V>, \<C>) \<Turnstile>\<^sub>\<rho> \<rho>\<^sub>s\<^sub>e" by (blast intro: may_be_static_eval_value.cases)
+  with `\<rho>\<^sub>s\<^sub>e x\<^sub>m = Some \<omega>\<^sub>m`
+  show "{|\<omega>\<^sub>m|} \<subseteq> \<V> x\<^sub>m \<and> (\<V>, \<C>) \<Turnstile>\<^sub>\<omega> \<omega>\<^sub>m" by (blast intro: may_be_static_eval_env.cases)
+qed
+
+lemma may_be_static_eval_pool_to_env_let_sync_send: "
+  (\<V>, \<C>) \<Turnstile>\<^sub>\<E> \<E> \<Longrightarrow>
+  \<E> \<pi>\<^sub>s = Some (\<langle>LET x\<^sub>s = SYNC x\<^sub>s\<^sub>e in e\<^sub>s; \<rho>\<^sub>s; \<kappa>\<^sub>s\<rangle>) \<Longrightarrow>
+  \<rho>\<^sub>s x\<^sub>s\<^sub>e = Some (VClosure (Send_Evt x\<^sub>s\<^sub>c x\<^sub>m) \<rho>\<^sub>s\<^sub>e) \<Longrightarrow>
+  \<rho>\<^sub>s\<^sub>e x\<^sub>s\<^sub>c = Some (VChan c) \<Longrightarrow>
+  (\<V>, \<C>) \<Turnstile>\<^sub>\<rho> \<rho>\<^sub>s(x\<^sub>s \<mapsto> VUnit)
+"
+proof
+  assume "\<rho>\<^sub>s\<^sub>e x\<^sub>s\<^sub>c = Some (VChan c)"
+  and  "(\<V>, \<C>) \<Turnstile>\<^sub>\<E> \<E>"
+  and "\<E> \<pi>\<^sub>s = Some (\<langle>LET x\<^sub>s = SYNC x\<^sub>s\<^sub>e in e\<^sub>s; \<rho>\<^sub>s; \<kappa>\<^sub>s\<rangle>)"
+  and "\<rho>\<^sub>s x\<^sub>s\<^sub>e = Some (VClosure (Send_Evt x\<^sub>s\<^sub>c x\<^sub>m) \<rho>\<^sub>s\<^sub>e)"
+
+  from `(\<V>, \<C>) \<Turnstile>\<^sub>\<E> \<E>` and `\<E> \<pi>\<^sub>s = Some (\<langle>LET x\<^sub>s = SYNC x\<^sub>s\<^sub>e in e\<^sub>s; \<rho>\<^sub>s; \<kappa>\<^sub>s\<rangle>)`
+  have "(\<V>, \<C>) \<Turnstile>\<^sub>\<sigma> \<langle>LET x\<^sub>s = SYNC x\<^sub>s\<^sub>e in e\<^sub>s; \<rho>\<^sub>s; \<kappa>\<^sub>s\<rangle>" by (simp add: may_be_static_eval_pool.simps) then
+  have "(\<V>, \<C>) \<Turnstile>\<^sub>\<rho> \<rho>\<^sub>s" by (simp add: may_be_static_eval_state.simps)+
+
+  have "{^\<lparr>\<rparr>} \<subseteq> \<V> x\<^sub>s"
+  proof (cases c)
+    case (Ch \<pi> x\<^sub>c)
+    assume "c = Ch \<pi> x\<^sub>c" 
+    with `\<rho>\<^sub>s\<^sub>e x\<^sub>s\<^sub>c = Some (VChan c)`
+    and  `(\<V>, \<C>) \<Turnstile>\<^sub>\<E> \<E>`
+    and `\<E> \<pi>\<^sub>s = Some (\<langle>LET x\<^sub>s = SYNC x\<^sub>s\<^sub>e in e\<^sub>s; \<rho>\<^sub>s; \<kappa>\<^sub>s\<rangle>)`
+    and `\<rho>\<^sub>s x\<^sub>s\<^sub>e = Some (VClosure (Send_Evt x\<^sub>s\<^sub>c x\<^sub>m) \<rho>\<^sub>s\<^sub>e)`
+    show "{^\<lparr>\<rparr>} \<subseteq> \<V> x\<^sub>s" using may_be_static_eval_pool_let_sync_send_values_relate by simp
+  qed
+  
+  have "(\<V>, \<C>) \<Turnstile>\<^sub>\<omega> VUnit" by (simp add: Unit)
+  {
+    fix x' \<omega>'
+    assume "(\<rho>\<^sub>s(x\<^sub>s \<mapsto> VUnit)) x' = Some \<omega>'" "x' \<noteq> x\<^sub>s" then
+    have "\<rho>\<^sub>s x' = Some \<omega>'" by simp
+    with `(\<V>, \<C>) \<Turnstile>\<^sub>\<rho> \<rho>\<^sub>s` 
+    have "{|\<omega>'|} \<subseteq> \<V> x' \<and> (\<V>, \<C>) \<Turnstile>\<^sub>\<omega> \<omega>'" by (simp add: may_be_static_eval_env.simps)
+  }
+  with \<open>{^\<lparr>\<rparr>} \<subseteq> \<V> x\<^sub>s\<close> \<open>(\<V>, \<C>) \<Turnstile>\<^sub>\<omega> VUnit\<close> 
+  show "\<forall>x \<omega>. (\<rho>\<^sub>s(x\<^sub>s \<mapsto> VUnit)) x = Some \<omega> \<longrightarrow> {|\<omega>|} \<subseteq> \<V> x \<and> (\<V>, \<C>) \<Turnstile>\<^sub>\<omega> \<omega>" by simp
+qed
+
+
+lemma may_be_static_eval_pool_let_sync_recv_values_relate: "
+  (\<V>, \<C>) \<Turnstile>\<^sub>\<E> \<E> \<Longrightarrow>
+  \<E> \<pi>\<^sub>r = Some (\<langle>LET x\<^sub>r = SYNC x\<^sub>r\<^sub>e in e\<^sub>r; \<rho>\<^sub>r; \<kappa>\<^sub>r\<rangle>) \<Longrightarrow>
+  \<rho>\<^sub>r x\<^sub>r\<^sub>e = Some (VClosure (Recv_Evt x\<^sub>r\<^sub>c) \<rho>\<^sub>r\<^sub>e) \<Longrightarrow>
+  \<rho>\<^sub>r\<^sub>e x\<^sub>r\<^sub>c = Some (VChan (Ch \<pi>\<^sub>c x\<^sub>c)) \<Longrightarrow>
+  \<C> x\<^sub>c \<subseteq> \<V> x\<^sub>r
+"
+proof -
+  assume "(\<V>, \<C>) \<Turnstile>\<^sub>\<E> \<E>"
+  and "\<E> \<pi>\<^sub>r = Some (\<langle>LET x\<^sub>r = SYNC x\<^sub>r\<^sub>e in e\<^sub>r; \<rho>\<^sub>r; \<kappa>\<^sub>r\<rangle>)"
+  and "\<rho>\<^sub>r x\<^sub>r\<^sub>e = Some (VClosure (Recv_Evt x\<^sub>r\<^sub>c) \<rho>\<^sub>r\<^sub>e)"
+  and "\<rho>\<^sub>r\<^sub>e x\<^sub>r\<^sub>c = Some (VChan (Ch \<pi>\<^sub>c x\<^sub>c))"
+
+  from `(\<V>, \<C>) \<Turnstile>\<^sub>\<E> \<E>` and `\<E> \<pi>\<^sub>r = Some (\<langle>LET x\<^sub>r = SYNC x\<^sub>r\<^sub>e in e\<^sub>r; \<rho>\<^sub>r; \<kappa>\<^sub>r\<rangle>)`
+  have "(\<V>, \<C>) \<Turnstile>\<^sub>\<sigma> \<langle>LET x\<^sub>r = SYNC x\<^sub>r\<^sub>e in e\<^sub>r; \<rho>\<^sub>r; \<kappa>\<^sub>r\<rangle>" by (simp add: may_be_static_eval_pool.simps) then
+  have "(\<V>, \<C>) \<Turnstile>\<^sub>e LET x\<^sub>r = SYNC x\<^sub>r\<^sub>e in e\<^sub>r" "(\<V>, \<C>) \<Turnstile>\<^sub>\<rho> \<rho>\<^sub>r" by (simp add: may_be_static_eval_state.simps)+
+
+  from `(\<V>, \<C>) \<Turnstile>\<^sub>\<rho> \<rho>\<^sub>r` and `\<rho>\<^sub>r x\<^sub>r\<^sub>e = Some (VClosure (Recv_Evt x\<^sub>r\<^sub>c) \<rho>\<^sub>r\<^sub>e)`
+  have "{|(VClosure (Recv_Evt x\<^sub>r\<^sub>c) \<rho>\<^sub>r\<^sub>e)|} \<subseteq> \<V> x\<^sub>r\<^sub>e" and "(\<V>, \<C>) \<Turnstile>\<^sub>\<omega> (VClosure (Recv_Evt x\<^sub>r\<^sub>c) \<rho>\<^sub>r\<^sub>e)" by (blast intro: may_be_static_eval_env.cases)+
+
+  from `{|(VClosure (Recv_Evt x\<^sub>r\<^sub>c) \<rho>\<^sub>r\<^sub>e)|} \<subseteq> \<V> x\<^sub>r\<^sub>e`
+  have "^Recv_Evt x\<^sub>r\<^sub>c \<in> \<V> x\<^sub>r\<^sub>e" by simp
+
+  from `(\<V>, \<C>) \<Turnstile>\<^sub>\<omega> (VClosure (Recv_Evt x\<^sub>r\<^sub>c) \<rho>\<^sub>r\<^sub>e)`
+  have "(\<V>, \<C>) \<Turnstile>\<^sub>\<rho> \<rho>\<^sub>r\<^sub>e" by (blast intro: may_be_static_eval_value.cases)
+  with `\<rho>\<^sub>r\<^sub>e x\<^sub>r\<^sub>c = Some (VChan (Ch \<pi>\<^sub>c x\<^sub>c))`
+  have "{|(VChan (Ch \<pi>\<^sub>c x\<^sub>c))|} \<subseteq> \<V> x\<^sub>r\<^sub>c" by (blast intro: may_be_static_eval_env.cases) then
+  have "{^Chan x\<^sub>c} \<subseteq> \<V> x\<^sub>r\<^sub>c" by simp then
+  have "^Chan x\<^sub>c \<in> \<V> x\<^sub>r\<^sub>c" by auto
+  
+  from `(\<V>, \<C>) \<Turnstile>\<^sub>e LET x\<^sub>r = SYNC x\<^sub>r\<^sub>e in e\<^sub>r`
+  show "\<C> x\<^sub>c \<subseteq> \<V> x\<^sub>r"
+  proof cases
+    case Let_Sync
+    assume "\<forall>x\<^sub>r\<^sub>c x\<^sub>c. ^Recv_Evt x\<^sub>r\<^sub>c \<in> \<V> x\<^sub>r\<^sub>e \<longrightarrow> ^Chan x\<^sub>c \<in> \<V> x\<^sub>r\<^sub>c \<longrightarrow> \<C> x\<^sub>c \<subseteq> \<V> x\<^sub>r"
+    with `^Recv_Evt x\<^sub>r\<^sub>c \<in> \<V> x\<^sub>r\<^sub>e` and `^Chan x\<^sub>c \<in> \<V> x\<^sub>r\<^sub>c`
+    show "\<C> x\<^sub>c \<subseteq> \<V> x\<^sub>r" by blast
+  qed
+qed
+
+
+lemma may_be_static_eval_pool_to_stack_let: "
+  (\<V>, \<C>) \<Turnstile>\<^sub>\<E> \<E> \<Longrightarrow>
+  \<E> \<pi> = Some (\<langle>LET x = b in e; \<rho>; \<kappa>\<rangle>) \<Longrightarrow>
+  (\<V>, \<C>) \<Turnstile>\<^sub>\<kappa> \<V> (\<lfloor>e\<rfloor>) \<Rrightarrow> \<kappa>
+"
+proof -
+  assume "(\<V>, \<C>) \<Turnstile>\<^sub>\<E> \<E>" and "\<E> \<pi> = Some (\<langle>LET x = b in e; \<rho>; \<kappa>\<rangle>)" then
+  have "(\<V>, \<C>) \<Turnstile>\<^sub>\<sigma> \<langle>LET x = b in e; \<rho>; \<kappa>\<rangle>" by (simp add: may_be_static_eval_pool.simps) then
+  show "(\<V>, \<C>) \<Turnstile>\<^sub>\<kappa> \<V> (\<lfloor>e\<rfloor>) \<Rrightarrow> \<kappa>" by (simp add: may_be_static_eval_state_to_stack_let)
+qed
+
+lemma may_be_static_eval_pool_to_env_let_sync_recv: "
+  (\<V>, \<C>) \<Turnstile>\<^sub>\<E> \<E> \<Longrightarrow>
+  \<E> \<pi>\<^sub>s = Some (\<langle>LET x\<^sub>s = SYNC x\<^sub>s\<^sub>e in e\<^sub>s; \<rho>\<^sub>s; \<kappa>\<^sub>s\<rangle>) \<Longrightarrow>
+  \<rho>\<^sub>s x\<^sub>s\<^sub>e = Some (VClosure (Send_Evt x\<^sub>s\<^sub>c x\<^sub>m) \<rho>\<^sub>s\<^sub>e) \<Longrightarrow>
+  \<rho>\<^sub>s\<^sub>e x\<^sub>s\<^sub>c = Some (VChan c) \<Longrightarrow>
+  \<rho>\<^sub>s\<^sub>e x\<^sub>m = Some \<omega>\<^sub>m \<Longrightarrow>
+  \<E> \<pi>\<^sub>r = Some (\<langle>LET x\<^sub>r = SYNC x\<^sub>r\<^sub>e in e\<^sub>r; \<rho>\<^sub>r; \<kappa>\<^sub>r\<rangle>) \<Longrightarrow> 
+  \<rho>\<^sub>r x\<^sub>r\<^sub>e = Some (VClosure (Recv_Evt x\<^sub>r\<^sub>c) \<rho>\<^sub>r\<^sub>e) \<Longrightarrow> 
+  \<rho>\<^sub>r\<^sub>e x\<^sub>r\<^sub>c = Some (VChan c) \<Longrightarrow> 
+  (\<V>, \<C>) \<Turnstile>\<^sub>\<rho> \<rho>\<^sub>r(x\<^sub>r \<mapsto> \<omega>\<^sub>m)
+"
+proof
+  assume "(\<V>, \<C>) \<Turnstile>\<^sub>\<E> \<E>"
+  and "\<E> \<pi>\<^sub>s = Some (\<langle>LET x\<^sub>s = SYNC x\<^sub>s\<^sub>e in e\<^sub>s; \<rho>\<^sub>s; \<kappa>\<^sub>s\<rangle>)"
+  and "\<rho>\<^sub>s x\<^sub>s\<^sub>e = Some (VClosure (Send_Evt x\<^sub>s\<^sub>c x\<^sub>m) \<rho>\<^sub>s\<^sub>e)"
+  and "\<rho>\<^sub>s\<^sub>e x\<^sub>m = Some \<omega>\<^sub>m" then
+  have "{|\<omega>\<^sub>m|} \<subseteq> \<V> x\<^sub>m" "(\<V>, \<C>) \<Turnstile>\<^sub>\<omega> \<omega>\<^sub>m" using may_be_static_eval_pool_let_sync_send_message_relate by auto
+
+  assume "\<rho>\<^sub>s\<^sub>e x\<^sub>s\<^sub>c = Some (VChan c)"
+  and "\<E> \<pi>\<^sub>r = Some (\<langle>LET x\<^sub>r = SYNC x\<^sub>r\<^sub>e in e\<^sub>r; \<rho>\<^sub>r; \<kappa>\<^sub>r\<rangle>)"
+  and "\<rho>\<^sub>r x\<^sub>r\<^sub>e = Some (VClosure (Recv_Evt x\<^sub>r\<^sub>c) \<rho>\<^sub>r\<^sub>e)"
+  and "\<rho>\<^sub>r\<^sub>e x\<^sub>r\<^sub>c = Some (VChan c)"
+
+  from `(\<V>, \<C>) \<Turnstile>\<^sub>\<E> \<E>` and `\<E> \<pi>\<^sub>r = Some (\<langle>LET x\<^sub>r = SYNC x\<^sub>r\<^sub>e in e\<^sub>r; \<rho>\<^sub>r; \<kappa>\<^sub>r\<rangle>)`
+  have "(\<V>, \<C>) \<Turnstile>\<^sub>\<sigma> \<langle>LET x\<^sub>r = SYNC x\<^sub>r\<^sub>e in e\<^sub>r; \<rho>\<^sub>r; \<kappa>\<^sub>r\<rangle>" by (simp add: may_be_static_eval_pool.simps) then
+  have "(\<V>, \<C>) \<Turnstile>\<^sub>\<rho> \<rho>\<^sub>r" by (simp add: may_be_static_eval_state.simps)+
+
+
+  have "\<V> x\<^sub>m \<subseteq> \<V> x\<^sub>r"
+  proof (cases c)
+    case (Ch \<pi>\<^sub>c x\<^sub>c)
+    assume "c = Ch \<pi>\<^sub>c x\<^sub>c" 
+
+    with `c = Ch \<pi>\<^sub>c x\<^sub>c`
+    and `\<rho>\<^sub>s\<^sub>e x\<^sub>s\<^sub>c = Some (VChan c)`
+    and `(\<V>, \<C>) \<Turnstile>\<^sub>\<E> \<E>`
+    and `\<rho>\<^sub>s x\<^sub>s\<^sub>e = Some (VClosure (Send_Evt x\<^sub>s\<^sub>c x\<^sub>m) \<rho>\<^sub>s\<^sub>e)`
+    and `\<E> \<pi>\<^sub>s = Some (\<langle>LET x\<^sub>s = SYNC x\<^sub>s\<^sub>e in e\<^sub>s; \<rho>\<^sub>s; \<kappa>\<^sub>s\<rangle>)`
+    and `\<rho>\<^sub>s\<^sub>e x\<^sub>m = Some \<omega>\<^sub>m`
+    have "\<V> x\<^sub>m \<subseteq> \<C> x\<^sub>c" using \<open>\<rho>\<^sub>s\<^sub>e x\<^sub>s\<^sub>c = Some (VChan c)\<close> may_be_static_eval_pool_let_sync_send_values_relate by blast
+
+    with `c = Ch \<pi>\<^sub>c x\<^sub>c`
+    and `\<rho>\<^sub>r\<^sub>e x\<^sub>r\<^sub>c = Some (VChan c)`
+    and `(\<V>, \<C>) \<Turnstile>\<^sub>\<E> \<E>`
+    and `\<E> \<pi>\<^sub>r = Some (\<langle>LET x\<^sub>r = SYNC x\<^sub>r\<^sub>e in e\<^sub>r; \<rho>\<^sub>r; \<kappa>\<^sub>r\<rangle>)`
+    and `\<rho>\<^sub>r x\<^sub>r\<^sub>e = Some (VClosure (Recv_Evt x\<^sub>r\<^sub>c) \<rho>\<^sub>r\<^sub>e)`
+    have "\<C> x\<^sub>c \<subseteq> \<V> x\<^sub>r" using  may_be_static_eval_pool_let_sync_recv_values_relate by auto
+
+    from `\<V> x\<^sub>m \<subseteq> \<C> x\<^sub>c` and `\<C> x\<^sub>c \<subseteq> \<V> x\<^sub>r`
+    show "\<V> x\<^sub>m \<subseteq> \<V> x\<^sub>r" by simp
+  qed
+
+  from `{|\<omega>\<^sub>m|} \<subseteq> \<V> x\<^sub>m` and `\<V> x\<^sub>m \<subseteq> \<V> x\<^sub>r`
+  have "{|\<omega>\<^sub>m|} \<subseteq> \<V> x\<^sub>r" by blast
+
+  from `(\<V>, \<C>) \<Turnstile>\<^sub>\<E> \<E>` and `\<E> \<pi>\<^sub>s = Some (\<langle>LET x\<^sub>s = SYNC x\<^sub>s\<^sub>e in e\<^sub>s; \<rho>\<^sub>s; \<kappa>\<^sub>s\<rangle>)`
+  have "(\<V>, \<C>) \<Turnstile>\<^sub>\<sigma> \<langle>LET x\<^sub>s = SYNC x\<^sub>s\<^sub>e in e\<^sub>s; \<rho>\<^sub>s; \<kappa>\<^sub>s\<rangle>" by (simp add: may_be_static_eval_pool.simps) then
+  have "(\<V>, \<C>) \<Turnstile>\<^sub>\<rho> \<rho>\<^sub>s" by (simp add: may_be_static_eval_state.simps)+
+  {
+    fix x' \<omega>'
+    assume "(\<rho>\<^sub>r(x\<^sub>r \<mapsto> \<omega>\<^sub>m)) x' = Some \<omega>'" "x' \<noteq> x\<^sub>r" then
+    have "\<rho>\<^sub>r x' = Some \<omega>'" by simp
+    with `(\<V>, \<C>) \<Turnstile>\<^sub>\<rho> \<rho>\<^sub>r` 
+    have "{|\<omega>'|} \<subseteq> \<V> x' \<and> (\<V>, \<C>) \<Turnstile>\<^sub>\<omega> \<omega>'" by (simp add: may_be_static_eval_env.simps)
+  }
+  with `{|\<omega>\<^sub>m|} \<subseteq> \<V> x\<^sub>r` and `(\<V>, \<C>) \<Turnstile>\<^sub>\<omega> \<omega>\<^sub>m`
+  show "\<forall>x \<omega>. (\<rho>\<^sub>r(x\<^sub>r \<mapsto> \<omega>\<^sub>m)) x = Some \<omega> \<longrightarrow> {|\<omega>|} \<subseteq> \<V> x \<and> (\<V>, \<C>) \<Turnstile>\<^sub>\<omega> \<omega>" by auto
+qed
+
+
+lemma may_be_static_eval_preserved_under_sync: "
+  (\<V>, \<C>) \<Turnstile>\<^sub>\<E> \<E> \<Longrightarrow>
+  \<E> \<pi>\<^sub>s = Some (\<langle>LET x\<^sub>s = SYNC x\<^sub>s\<^sub>e in e\<^sub>s; \<rho>\<^sub>s; \<kappa>\<^sub>s\<rangle>) \<Longrightarrow>
+  \<rho>\<^sub>s x\<^sub>s\<^sub>e = Some (VClosure (Send_Evt x\<^sub>s\<^sub>c x\<^sub>m) \<rho>\<^sub>s\<^sub>e) \<Longrightarrow>
+  \<rho>\<^sub>s\<^sub>e x\<^sub>s\<^sub>c = Some (VChan c) \<Longrightarrow>
+  \<rho>\<^sub>s\<^sub>e x\<^sub>m = Some \<omega>\<^sub>m \<Longrightarrow>
+  \<E> \<pi>\<^sub>r = Some (\<langle>LET x\<^sub>r = SYNC x\<^sub>r\<^sub>e in e\<^sub>r; \<rho>\<^sub>r; \<kappa>\<^sub>r\<rangle>) \<Longrightarrow>
+  \<rho>\<^sub>r x\<^sub>r\<^sub>e = Some (VClosure (Recv_Evt x\<^sub>r\<^sub>c) \<rho>\<^sub>r\<^sub>e) \<Longrightarrow>
+  \<rho>\<^sub>r\<^sub>e x\<^sub>r\<^sub>c = Some (VChan c) \<Longrightarrow> 
+  (\<V>, \<C>) \<Turnstile>\<^sub>\<E> \<E>(\<pi>\<^sub>s ;;(LNext x\<^sub>s) \<mapsto> \<langle>e\<^sub>s; \<rho>\<^sub>s(x\<^sub>s \<mapsto> VUnit); \<kappa>\<^sub>s\<rangle>, \<pi>\<^sub>r ;;(LNext x\<^sub>r) \<mapsto> \<langle>e\<^sub>r; \<rho>\<^sub>r(x\<^sub>r \<mapsto> \<omega>\<^sub>m); \<kappa>\<^sub>r\<rangle>)
+"
+proof
+  assume "(\<V>, \<C>) \<Turnstile>\<^sub>\<E> \<E>"
+  and "\<E> \<pi>\<^sub>s = Some (\<langle>LET x\<^sub>s = SYNC x\<^sub>s\<^sub>e in e\<^sub>s;\<rho>\<^sub>s;\<kappa>\<^sub>s\<rangle>)"
+  and "\<rho>\<^sub>s x\<^sub>s\<^sub>e = Some (VClosure (Send_Evt x\<^sub>s\<^sub>c x\<^sub>m) \<rho>\<^sub>s\<^sub>e)"
+  and "\<rho>\<^sub>s\<^sub>e x\<^sub>s\<^sub>c = Some (VChan c)"
+  and "\<rho>\<^sub>s\<^sub>e x\<^sub>m = Some \<omega>\<^sub>m"
+  and "\<E> \<pi>\<^sub>r = Some (\<langle>LET x\<^sub>r = SYNC x\<^sub>r\<^sub>e in e\<^sub>r;\<rho>\<^sub>r;\<kappa>\<^sub>r\<rangle>)"
+  and "\<rho>\<^sub>r x\<^sub>r\<^sub>e = Some (VClosure (Recv_Evt x\<^sub>r\<^sub>c) \<rho>\<^sub>r\<^sub>e)"
+  and "\<rho>\<^sub>r\<^sub>e x\<^sub>r\<^sub>c = Some (VChan c)"
+
+
+  from \<open>(\<V>, \<C>) \<Turnstile>\<^sub>\<E> \<E>\<close> and \<open>\<E> \<pi>\<^sub>s = Some (\<langle>LET x\<^sub>s = SYNC x\<^sub>s\<^sub>e in e\<^sub>s;\<rho>\<^sub>s;\<kappa>\<^sub>s\<rangle>)\<close> 
+  have "(\<V>, \<C>) \<Turnstile>\<^sub>e e\<^sub>s" by (blast intro: may_be_static_eval_pool_to_exp_let)
+
+  from \<open>(\<V>, \<C>) \<Turnstile>\<^sub>\<E> \<E>\<close> \<open>\<E> \<pi>\<^sub>s = Some (\<langle>LET x\<^sub>s = SYNC x\<^sub>s\<^sub>e in e\<^sub>s;\<rho>\<^sub>s;\<kappa>\<^sub>s\<rangle>)\<close> 
+  and \<open>\<rho>\<^sub>s x\<^sub>s\<^sub>e = Some (VClosure (Send_Evt x\<^sub>s\<^sub>c x\<^sub>m) \<rho>\<^sub>s\<^sub>e)\<close> \<open>\<rho>\<^sub>s\<^sub>e x\<^sub>s\<^sub>c = Some (VChan c)\<close> 
+  have "(\<V>, \<C>) \<Turnstile>\<^sub>\<rho> \<rho>\<^sub>s(x\<^sub>s \<mapsto> VUnit)" by (blast intro: may_be_static_eval_pool_to_env_let_sync_send)
+
+  from \<open>(\<V>, \<C>) \<Turnstile>\<^sub>\<E> \<E>\<close> and \<open>\<E> \<pi>\<^sub>s = Some (\<langle>LET x\<^sub>s = SYNC x\<^sub>s\<^sub>e in e\<^sub>s;\<rho>\<^sub>s;\<kappa>\<^sub>s\<rangle>)\<close>
+  have  "(\<V>, \<C>) \<Turnstile>\<^sub>\<kappa> \<V> (\<lfloor>e\<^sub>s\<rfloor>) \<Rrightarrow> \<kappa>\<^sub>s" by (blast intro: may_be_static_eval_pool_to_stack_let)
+
+  from `(\<V>, \<C>) \<Turnstile>\<^sub>e e\<^sub>s` and `(\<V>, \<C>) \<Turnstile>\<^sub>\<rho> \<rho>\<^sub>s(x\<^sub>s \<mapsto> VUnit)` and `(\<V>, \<C>) \<Turnstile>\<^sub>\<kappa> \<V> (\<lfloor>e\<^sub>s\<rfloor>) \<Rrightarrow> \<kappa>\<^sub>s`
+  have "(\<V>, \<C>) \<Turnstile>\<^sub>\<sigma> \<langle>e\<^sub>s;\<rho>\<^sub>s(x\<^sub>s \<mapsto> VUnit);\<kappa>\<^sub>s\<rangle>" by (blast intro: may_be_static_eval_state.intros)
+
+  from \<open>(\<V>, \<C>) \<Turnstile>\<^sub>\<E> \<E>\<close> and \<open>\<E> \<pi>\<^sub>r = Some (\<langle>LET x\<^sub>r = SYNC x\<^sub>r\<^sub>e in e\<^sub>r;\<rho>\<^sub>r;\<kappa>\<^sub>r\<rangle>)\<close> 
+  have "(\<V>, \<C>) \<Turnstile>\<^sub>e e\<^sub>r" by (blast intro: may_be_static_eval_pool_to_exp_let)
+
+  from \<open>(\<V>, \<C>) \<Turnstile>\<^sub>\<E> \<E>\<close> 
+  and \<open>\<E> \<pi>\<^sub>s = Some (\<langle>LET x\<^sub>s = SYNC x\<^sub>s\<^sub>e in e\<^sub>s;\<rho>\<^sub>s;\<kappa>\<^sub>s\<rangle>)\<close> 
+  and \<open>\<rho>\<^sub>s x\<^sub>s\<^sub>e = Some (VClosure (Send_Evt x\<^sub>s\<^sub>c x\<^sub>m) \<rho>\<^sub>s\<^sub>e)\<close> 
+  and \<open>\<rho>\<^sub>s\<^sub>e x\<^sub>m = Some \<omega>\<^sub>m\<close> \<open>\<rho>\<^sub>s\<^sub>e x\<^sub>s\<^sub>c = Some (VChan c)\<close>
+  and \<open>\<E> \<pi>\<^sub>r = Some (\<langle>LET x\<^sub>r = SYNC x\<^sub>r\<^sub>e in e\<^sub>r;\<rho>\<^sub>r;\<kappa>\<^sub>r\<rangle>)\<close> 
+  and \<open>\<rho>\<^sub>r x\<^sub>r\<^sub>e = Some (VClosure (Recv_Evt x\<^sub>r\<^sub>c) \<rho>\<^sub>r\<^sub>e)\<close> \<open>\<rho>\<^sub>r\<^sub>e x\<^sub>r\<^sub>c = Some (VChan c)\<close> 
+  have "(\<V>, \<C>) \<Turnstile>\<^sub>\<rho> \<rho>\<^sub>r(x\<^sub>r \<mapsto> \<omega>\<^sub>m)" by (blast intro: may_be_static_eval_pool_to_env_let_sync_recv)
+
+  from \<open>(\<V>, \<C>) \<Turnstile>\<^sub>\<E> \<E>\<close> and \<open>\<E> \<pi>\<^sub>r = Some (\<langle>LET x\<^sub>r = SYNC x\<^sub>r\<^sub>e in e\<^sub>r;\<rho>\<^sub>r;\<kappa>\<^sub>r\<rangle>)\<close>
+  have  "(\<V>, \<C>) \<Turnstile>\<^sub>\<kappa> \<V> (\<lfloor>e\<^sub>r\<rfloor>) \<Rrightarrow> \<kappa>\<^sub>r" by (blast intro: may_be_static_eval_pool_to_stack_let)
+
+  from `(\<V>, \<C>) \<Turnstile>\<^sub>e e\<^sub>r` and `(\<V>, \<C>) \<Turnstile>\<^sub>\<rho> \<rho>\<^sub>r(x\<^sub>r \<mapsto> \<omega>\<^sub>m)` and `(\<V>, \<C>) \<Turnstile>\<^sub>\<kappa> \<V> (\<lfloor>e\<^sub>r\<rfloor>) \<Rrightarrow> \<kappa>\<^sub>r`
+  have "(\<V>, \<C>) \<Turnstile>\<^sub>\<sigma> \<langle>e\<^sub>r;\<rho>\<^sub>r(x\<^sub>r \<mapsto> \<omega>\<^sub>m);\<kappa>\<^sub>r\<rangle>" by (blast intro: may_be_static_eval_state.intros)
+
+  {
+    fix \<pi> \<sigma>
+    assume  "\<pi> \<noteq> \<pi>\<^sub>s ;;(LNext x\<^sub>s)" and "\<pi> \<noteq> \<pi>\<^sub>r ;; (LNext x\<^sub>r)"
+    and "(\<E>(\<pi>\<^sub>s ;;(LNext x\<^sub>s) \<mapsto> \<langle>e\<^sub>s;\<rho>\<^sub>s(x\<^sub>s \<mapsto> VUnit);\<kappa>\<^sub>s\<rangle>, \<pi>\<^sub>r ;; (LNext x\<^sub>r) \<mapsto> \<langle>e\<^sub>r;\<rho>\<^sub>r(x\<^sub>r \<mapsto> \<omega>\<^sub>m);\<kappa>\<^sub>r\<rangle>)) \<pi> = Some \<sigma>" then
+    have "\<E> \<pi> = Some \<sigma>" by simp
+    with \<open>(\<V>, \<C>) \<Turnstile>\<^sub>\<E> \<E>\<close>
+    have "(\<V>, \<C>) \<Turnstile>\<^sub>\<sigma> \<sigma>" by (blast intro: may_be_static_eval_pool.cases)
+  } with `(\<V>, \<C>) \<Turnstile>\<^sub>\<sigma> \<langle>e\<^sub>r;\<rho>\<^sub>r (x\<^sub>r \<mapsto> \<omega>\<^sub>m);\<kappa>\<^sub>r\<rangle>` `(\<V>, \<C>) \<Turnstile>\<^sub>\<sigma> \<langle>e\<^sub>s;\<rho>\<^sub>s (x\<^sub>s \<mapsto> VUnit);\<kappa>\<^sub>s\<rangle>`
+  show "\<forall>\<pi> \<sigma>. (\<E>(\<pi>\<^sub>s ;; (LNext x\<^sub>s) \<mapsto> \<langle>e\<^sub>s;\<rho>\<^sub>s(x\<^sub>s \<mapsto> VUnit);\<kappa>\<^sub>s\<rangle>, \<pi>\<^sub>r ;;(LNext x\<^sub>r) \<mapsto> \<langle>e\<^sub>r;\<rho>\<^sub>r(x\<^sub>r \<mapsto> \<omega>\<^sub>m);\<kappa>\<^sub>r\<rangle>)) \<pi> = Some \<sigma> \<longrightarrow> (\<V>, \<C>) \<Turnstile>\<^sub>\<sigma> \<sigma>" by simp
+
+qed
+
+
+lemma may_be_static_eval_pool_to_env_let_chan: "
+  (\<V>, \<C>) \<Turnstile>\<^sub>\<E> \<E> \<Longrightarrow>
+  \<E> \<pi> = Some (\<langle>LET x = CHAN \<lparr>\<rparr> in e; \<rho>; \<kappa>\<rangle>) \<Longrightarrow> 
+  (\<V>, \<C>) \<Turnstile>\<^sub>\<rho> \<rho>(x \<mapsto> (VChan (Ch \<pi> x)))
+"
+proof
+  assume "(\<V>, \<C>) \<Turnstile>\<^sub>\<E> \<E>" and "\<E> \<pi> = Some (\<langle>LET x = CHAN \<lparr>\<rparr> in e; \<rho>; \<kappa>\<rangle>)" then
+  have "(\<V>, \<C>) \<Turnstile>\<^sub>\<sigma> \<langle>LET x = CHAN \<lparr>\<rparr> in e; \<rho>; \<kappa>\<rangle>" by (blast intro: may_be_static_eval_pool.cases) then
+  have "(\<V>, \<C>) \<Turnstile>\<^sub>e LET x = CHAN \<lparr>\<rparr> in e" by (blast intro: may_be_static_eval_state.cases) then
+  have "{^Chan x} \<subseteq> \<V> x"  by (blast intro: may_be_static_eval.cases)
+  have "(\<V>, \<C>) \<Turnstile>\<^sub>\<omega> (VChan (Ch \<pi> x))" by (simp add: Chan)
+
+  from `(\<V>, \<C>) \<Turnstile>\<^sub>\<sigma> \<langle>LET x = CHAN \<lparr>\<rparr> in e; \<rho>; \<kappa>\<rangle>` 
+  have "(\<V>, \<C>) \<Turnstile>\<^sub>\<rho> \<rho>" by (simp add: may_be_static_eval_state.simps)+
+  {
+    fix x' \<omega>'
+    assume "(\<rho>(x \<mapsto> (VChan (Ch \<pi> x)))) x' = Some \<omega>'" and "x \<noteq> x'"then
+    have "\<rho> x' = Some \<omega>'" by simp with `(\<V>, \<C>) \<Turnstile>\<^sub>\<rho> \<rho>`
+    have "{|\<omega>'|} \<subseteq> \<V> x' \<and> (\<V>, \<C>) \<Turnstile>\<^sub>\<omega> \<omega>'" by (simp add: may_be_static_eval_env.simps)
+  } with `{^Chan x} \<subseteq> \<V> x` and `(\<V>, \<C>) \<Turnstile>\<^sub>\<omega> (VChan (Ch \<pi> x))`
+  show "\<forall>x' \<omega>'. (\<rho>(x \<mapsto> (VChan (Ch \<pi> x)))) x' = Some \<omega>' \<longrightarrow> {|\<omega>'|} \<subseteq> \<V> x' \<and> (\<V>, \<C>) \<Turnstile>\<^sub>\<omega> \<omega>'" by simp
+qed
+
+
+lemma may_be_static_eval_preserved_under_chan: "
+  (\<V>, \<C>) \<Turnstile>\<^sub>\<E> \<E> \<Longrightarrow>
+  \<E> \<pi> = Some (\<langle>LET x = CHAN \<lparr>\<rparr> in e; \<rho>; \<kappa>\<rangle>) \<Longrightarrow> 
+  (\<V>, \<C>) \<Turnstile>\<^sub>\<E> \<E>(\<pi> ;;(LNext x) \<mapsto> \<langle>e; \<rho>(x \<mapsto> (VChan (Ch \<pi> x))); \<kappa>\<rangle>)
+"
+proof
+  assume "(\<V>, \<C>) \<Turnstile>\<^sub>\<E> \<E>" and "\<E> \<pi> = Some (\<langle>LET x = CHAN \<lparr>\<rparr> in e; \<rho>; \<kappa>\<rangle>)" then
+  have "(\<V>, \<C>) \<Turnstile>\<^sub>e e" by (blast intro: may_be_static_eval_pool_to_exp_let)
+
+  from `(\<V>, \<C>) \<Turnstile>\<^sub>\<E> \<E>` and `\<E> \<pi> = Some (\<langle>LET x = CHAN \<lparr>\<rparr> in e; \<rho>; \<kappa>\<rangle>)`
+  have "(\<V>, \<C>) \<Turnstile>\<^sub>\<rho> \<rho>(x \<mapsto> (VChan (Ch \<pi> x)))" by (blast intro: may_be_static_eval_pool_to_env_let_chan )
+
+  from `(\<V>, \<C>) \<Turnstile>\<^sub>\<E> \<E>` and `\<E> \<pi> = Some (\<langle>LET x = CHAN \<lparr>\<rparr> in e; \<rho>; \<kappa>\<rangle>)`
+  have "(\<V>, \<C>) \<Turnstile>\<^sub>\<kappa> \<V> (\<lfloor>e\<rfloor>) \<Rrightarrow> \<kappa>" by (blast intro: may_be_static_eval_pool_to_stack_let)
+
+  from `(\<V>, \<C>) \<Turnstile>\<^sub>e e` and `(\<V>, \<C>) \<Turnstile>\<^sub>\<rho> \<rho>(x \<mapsto> (VChan (Ch \<pi> x)))` and `(\<V>, \<C>) \<Turnstile>\<^sub>\<kappa> \<V> (\<lfloor>e\<rfloor>) \<Rrightarrow> \<kappa>`
+  have "(\<V>, \<C>) \<Turnstile>\<^sub>\<sigma> \<langle>e;\<rho>(x \<mapsto> (VChan (Ch \<pi> x)));\<kappa>\<rangle>" by (blast intro: may_be_static_eval_state.intros)
+  {
+    fix \<pi>' \<sigma>'
+    assume "(\<E>(\<pi> ;;(LNext x) \<mapsto> \<langle>e;\<rho>(x \<mapsto> (VChan (Ch \<pi> x)));\<kappa>\<rangle>)) \<pi>' = Some \<sigma>'" 
+    and "\<pi>' \<noteq> \<pi> ;;(LNext x)" then
+    have "\<E> \<pi>' = Some \<sigma>'" by simp with `(\<V>, \<C>) \<Turnstile>\<^sub>\<E> \<E>`
+    have "(\<V>, \<C>) \<Turnstile>\<^sub>\<sigma> \<sigma>'" by (simp add: may_be_static_eval_pool.simps)
+  } with `(\<V>, \<C>) \<Turnstile>\<^sub>\<sigma> \<langle>e;\<rho>(x \<mapsto> (VChan (Ch \<pi> x)));\<kappa>\<rangle>`
+  show "\<forall>\<pi>' \<sigma>'. (\<E>(\<pi> ;;(LNext x) \<mapsto> \<langle>e;\<rho>(x \<mapsto> (VChan (Ch \<pi> x)));\<kappa>\<rangle>)) \<pi>' = Some \<sigma>' \<longrightarrow> (\<V>, \<C>) \<Turnstile>\<^sub>\<sigma> \<sigma>'" by simp
+qed
+
+
+lemma may_be_static_eval_pool_to_env_let_spawn: "
+  (\<V>, \<C>) \<Turnstile>\<^sub>\<E> \<E> \<Longrightarrow>
+  \<E> \<pi> = Some (\<langle>LET x = SPAWN e\<^sub>c in e; \<rho>; \<kappa>\<rangle>) \<Longrightarrow> 
+  (\<V>, \<C>) \<Turnstile>\<^sub>\<rho> \<rho>(x \<mapsto> VUnit)"
+proof
+
+  assume "(\<V>, \<C>) \<Turnstile>\<^sub>\<E> \<E>" and "\<E> \<pi> = Some (\<langle>LET x = SPAWN e\<^sub>c in e; \<rho>; \<kappa>\<rangle>)" then
+  have "(\<V>, \<C>) \<Turnstile>\<^sub>\<sigma> \<langle>LET x = SPAWN e\<^sub>c in e; \<rho>; \<kappa>\<rangle>" by (simp add: may_be_static_eval_pool.simps) then
+  have "(\<V>, \<C>) \<Turnstile>\<^sub>e LET x = SPAWN e\<^sub>c in e" by (blast intro: may_be_static_eval_state.cases) then
+  have "{^\<lparr>\<rparr>} \<subseteq> \<V> x"  by (blast intro: may_be_static_eval.cases) then
+  have "(\<V>, \<C>) \<Turnstile>\<^sub>\<omega> VUnit" by (simp add: Unit)
+
+  from `(\<V>, \<C>) \<Turnstile>\<^sub>\<sigma> \<langle>LET x = SPAWN e\<^sub>c in e; \<rho>; \<kappa>\<rangle>` 
+  have "(\<V>, \<C>) \<Turnstile>\<^sub>\<rho> \<rho>" by (simp add: may_be_static_eval_state.simps)
+
+  {
+    fix x' \<omega>'
+    assume "(\<rho>(x \<mapsto> VUnit)) x' = Some \<omega>'" and "x \<noteq> x'" then
+    have "\<rho> x' = Some \<omega>'" by simp with `(\<V>, \<C>) \<Turnstile>\<^sub>\<rho> \<rho>`
+    have "{|\<omega>'|} \<subseteq> \<V> x' \<and> (\<V>, \<C>) \<Turnstile>\<^sub>\<omega> \<omega>'" by (blast intro: may_be_static_eval_env.cases)
+  } with `{^\<lparr>\<rparr>} \<subseteq> \<V> x` and `(\<V>, \<C>) \<Turnstile>\<^sub>\<omega> VUnit`
+  show "\<forall>x' \<omega>'. (\<rho>(x \<mapsto> VUnit)) x' = Some \<omega>' \<longrightarrow> {|\<omega>'|} \<subseteq> \<V> x' \<and> (\<V>, \<C>) \<Turnstile>\<^sub>\<omega> \<omega>'" by simp
+qed
+
+lemma may_be_static_eval_preserved_under_spawn: "
+  (\<V>, \<C>) \<Turnstile>\<^sub>\<E> \<E> \<Longrightarrow>
+  \<E> \<pi> = Some (\<langle>LET x = SPAWN e\<^sub>c in e; \<rho>; \<kappa>\<rangle>) \<Longrightarrow> 
+  (\<V>, \<C>) \<Turnstile>\<^sub>\<E> \<E>(\<pi> ;;(LNext x) \<mapsto> \<langle>e; \<rho>(x \<mapsto> VUnit); \<kappa>\<rangle>, \<pi>;;(LSpawn x) \<mapsto> \<langle>e\<^sub>c; \<rho>; []\<rangle>)
+"
+proof
+
+  assume "(\<V>, \<C>) \<Turnstile>\<^sub>\<E> \<E>" and "\<E> \<pi> = Some (\<langle>LET x = SPAWN e\<^sub>c in e; \<rho>; \<kappa>\<rangle>)"
+
+  from `(\<V>, \<C>) \<Turnstile>\<^sub>\<E> \<E>` and `\<E> \<pi> = Some (\<langle>LET x = SPAWN e\<^sub>c in e; \<rho>; \<kappa>\<rangle>)`
+  have "(\<V>, \<C>) \<Turnstile>\<^sub>e e" by (blast intro: may_be_static_eval_pool_to_exp_let)
+
+  from `(\<V>, \<C>) \<Turnstile>\<^sub>\<E> \<E>` and `\<E> \<pi> = Some (\<langle>LET x = SPAWN e\<^sub>c in e; \<rho>; \<kappa>\<rangle>)`
+  have "(\<V>, \<C>) \<Turnstile>\<^sub>\<rho> \<rho>(x \<mapsto> VUnit)" by (blast intro: may_be_static_eval_pool_to_env_let_spawn)
+
+  from `(\<V>, \<C>) \<Turnstile>\<^sub>\<E> \<E>` and `\<E> \<pi> = Some (\<langle>LET x = SPAWN e\<^sub>c in e; \<rho>; \<kappa>\<rangle>)`
+  have "(\<V>, \<C>) \<Turnstile>\<^sub>\<kappa> \<V> (\<lfloor>e\<rfloor>) \<Rrightarrow> \<kappa>" by (blast intro: may_be_static_eval_pool_to_stack_let)
+
+  from \<open>(\<V>, \<C>) \<Turnstile>\<^sub>\<kappa> \<V> (\<lfloor>e\<rfloor>) \<Rrightarrow> \<kappa>\<close> \<open>(\<V>, \<C>) \<Turnstile>\<^sub>\<rho> \<rho>(x \<mapsto> VUnit)\<close> \<open>(\<V>, \<C>) \<Turnstile>\<^sub>e e\<close>
+  have "(\<V>, \<C>) \<Turnstile>\<^sub>\<sigma> \<langle>e;\<rho>(x \<mapsto> VUnit);\<kappa>\<rangle>" by (simp add: may_be_static_eval_state.intros)
+
+  from `(\<V>, \<C>) \<Turnstile>\<^sub>\<E> \<E>` and `\<E> \<pi> = Some (\<langle>LET x = SPAWN e\<^sub>c in e; \<rho>; \<kappa>\<rangle>)`
+  have "(\<V>, \<C>) \<Turnstile>\<^sub>\<sigma> \<langle>LET x = SPAWN e\<^sub>c in e; \<rho>; \<kappa>\<rangle>" by (simp add: may_be_static_eval_pool.simps) then
+  have "(\<V>, \<C>) \<Turnstile>\<^sub>e LET x = SPAWN e\<^sub>c in e" and "(\<V>, \<C>) \<Turnstile>\<^sub>\<rho> \<rho>" by (simp add: may_be_static_eval_state.simps)+
+  
+  from `(\<V>, \<C>) \<Turnstile>\<^sub>e LET x = SPAWN e\<^sub>c in e`
+  have "(\<V>, \<C>) \<Turnstile>\<^sub>e e\<^sub>c" by (blast intro: may_be_static_eval.cases)
+
+  have "(\<V>, \<C>) \<Turnstile>\<^sub>\<kappa> \<V> (\<lfloor>e\<^sub>c\<rfloor>) \<Rrightarrow> []" by (simp add: may_be_static_eval_stack.Empty)
+  from \<open>(\<V>, \<C>) \<Turnstile>\<^sub>\<kappa> \<V> (\<lfloor>e\<^sub>c\<rfloor>) \<Rrightarrow> []\<close> \<open>(\<V>, \<C>) \<Turnstile>\<^sub>\<rho> \<rho>\<close> \<open>(\<V>, \<C>) \<Turnstile>\<^sub>e e\<^sub>c\<close> 
+  have "(\<V>, \<C>) \<Turnstile>\<^sub>\<sigma> \<langle>e\<^sub>c;\<rho>;[]\<rangle>" by (simp add: may_be_static_eval_state.intros)
+
+  {
+    fix \<pi>' \<sigma>'
+    assume "(\<E>(\<pi> ;;(LNext x) \<mapsto> \<langle>e;\<rho>(x \<mapsto> VUnit);\<kappa>\<rangle>, \<pi> ;; (LSpawn x) \<mapsto> \<langle>e\<^sub>c;\<rho>;[]\<rangle>)) \<pi>' = Some \<sigma>'"
+    and "\<pi>' \<noteq> \<pi> ;; (LNext x)" and " \<pi>' \<noteq> \<pi> ;; (LSpawn x)" then
+    have "\<E> \<pi>' = Some \<sigma>'" by simp with `(\<V>, \<C>) \<Turnstile>\<^sub>\<E> \<E>`
+    have "(\<V>, \<C>) \<Turnstile>\<^sub>\<sigma> \<sigma>'" by (blast intro: may_be_static_eval_pool.cases)
+  } with `(\<V>, \<C>) \<Turnstile>\<^sub>\<sigma> \<langle>e;\<rho>(x \<mapsto> VUnit);\<kappa>\<rangle>` and `(\<V>, \<C>) \<Turnstile>\<^sub>\<sigma> \<langle>e\<^sub>c;\<rho>;[]\<rangle>`
+  show "\<forall>\<pi>' \<sigma>'. (\<E>(\<pi> ;; (LNext x) \<mapsto> \<langle>e;\<rho>(x \<mapsto> VUnit);\<kappa>\<rangle>, \<pi> ;; (LSpawn x) \<mapsto> \<langle>e\<^sub>c;\<rho>;[]\<rangle>)) \<pi>' = Some \<sigma>' \<longrightarrow> (\<V>, \<C>) \<Turnstile>\<^sub>\<sigma> \<sigma>'" by simp
+qed
+
+
+theorem may_be_static_eval_preserved_under_concur_step : "
+  \<lbrakk>
+    (\<V>, \<C>) \<Turnstile>\<^sub>\<E> \<E>; 
+    (\<E>, H) \<rightarrow> (\<E>', H')
+  \<rbrakk> \<Longrightarrow>
+  (\<V>, \<C>) \<Turnstile>\<^sub>\<E> \<E>'
+"
+proof -
+  assume 
+    H1: "(\<V>, \<C>) \<Turnstile>\<^sub>\<E> \<E>" and
+    H2: "(\<E>, H) \<rightarrow> (\<E>', H')"
+
+  from H2 show "(\<V>, \<C>) \<Turnstile>\<^sub>\<E> \<E>'"
+  proof cases
+    case (Seq_Step_Down \<pi> x \<rho> x\<^sub>\<kappa> e\<^sub>\<kappa> \<rho>\<^sub>\<kappa> \<kappa> \<omega>)
+
+    assume 
+      H3: "\<E>' = \<E> ++ [\<pi> ;; LReturn x\<^sub>\<kappa> \<mapsto> \<langle>e\<^sub>\<kappa>;\<rho>\<^sub>\<kappa> ++ [x\<^sub>\<kappa> \<mapsto> \<omega>];\<kappa>\<rangle>]" and
+      H4: "leaf \<E> \<pi>" and 
+      H5: "\<E> \<pi> = Some (\<langle>RESULT x;\<rho>;\<langle>x\<^sub>\<kappa>,e\<^sub>\<kappa>,\<rho>\<^sub>\<kappa>\<rangle> # \<kappa>\<rangle>)" and 
+      H6: "\<rho> x = Some \<omega>"
+
+
+    from H1 H5 H6
+    have "(\<V>, \<C>) \<Turnstile>\<^sub>\<E> \<E>(\<pi> ;; LReturn x\<^sub>\<kappa> \<mapsto> \<langle>e\<^sub>\<kappa>;\<rho>\<^sub>\<kappa> ++ [x\<^sub>\<kappa> \<mapsto> \<omega>];\<kappa>\<rangle>)" using may_be_static_eval_pool.simps may_be_static_eval_state_to_state_result by fastforce
+
+    with H3 show "(\<V>, \<C>) \<Turnstile>\<^sub>\<E> \<E>'" by simp
+  next
+    case (Seq_Step \<pi> x b e \<rho> \<kappa> \<omega>)
+    assume 
+      H3: "\<E>' = \<E> ++ [\<pi> ;; (LNext x) \<mapsto> \<langle>e;\<rho>(x \<mapsto> \<omega>);\<kappa>\<rangle>]" and
+      H4: "leaf \<E> \<pi>" and 
+      H5: "\<E> \<pi> = Some (\<langle>LET x = b in e;\<rho>;\<kappa>\<rangle>)" and 
+      H6: "seq_step (b, \<rho>) \<omega>"
+
+    from H1 H5 have H7:"(\<V>, \<C>) \<Turnstile>\<^sub>\<sigma> \<langle>LET x = b in e;\<rho>;\<kappa>\<rangle>" by (auto simp: may_be_static_eval_pool.simps)
+
+    with H6 have H8: "(\<V>, \<C>) \<Turnstile>\<^sub>\<sigma> \<langle>e;\<rho>(x \<mapsto> \<omega>);\<kappa>\<rangle>" by (auto simp: may_be_static_eval_state_preserved_under_step)
+
+    with H1 have "(\<V>, \<C>) \<Turnstile>\<^sub>\<E> \<E>(\<pi> ;; (LNext x) \<mapsto> \<langle>e;\<rho>(x \<mapsto> \<omega>);\<kappa>\<rangle>)" by (auto simp: may_be_static_eval_pool.simps)
+
+    with H3 show "(\<V>, \<C>) \<Turnstile>\<^sub>\<E> \<E>'" by simp
+  next
+    case (Seq_Step_Up \<pi> x b e \<rho> \<kappa> e' \<rho>')
+    assume "\<E>' = \<E> ++ [\<pi> ;; (LCall x) \<mapsto> \<langle>e';\<rho>';\<langle>x,e,\<rho>\<rangle> # \<kappa>\<rangle>]"
+    assume "leaf \<E> \<pi>" and "\<E> \<pi> = Some (\<langle>LET x = b in e;\<rho>;\<kappa>\<rangle>)"
+    and "seq_step_up (b, \<rho>) (e', \<rho>')"
+    with \<open>(\<V>, \<C>) \<Turnstile>\<^sub>\<E> \<E>\<close>
+    have "(\<V>, \<C>) \<Turnstile>\<^sub>\<E> \<E>(\<pi> ;; (LCall) x \<mapsto> \<langle>e';\<rho>';\<langle>x,e,\<rho>\<rangle> # \<kappa>\<rangle>)"
+      using may_be_static_eval_pool.simps may_be_static_eval_state_preserved_under_step_up by fastforce
+    with \<open>\<E>' = \<E> ++ [\<pi> ;; (LCall x) \<mapsto> \<langle>e';\<rho>';\<langle>x,e,\<rho>\<rangle> # \<kappa>\<rangle>]\<close>
+    show "(\<V>, \<C>) \<Turnstile>\<^sub>\<E> \<E>'" by simp
+  next
+    case (Let_Chan \<pi> x e \<rho> \<kappa>)
+    assume "\<E>' = \<E> ++ [\<pi> ;; (LNext x) \<mapsto> \<langle>e;\<rho> ++ [x \<mapsto> (VChan (Ch \<pi> x))];\<kappa>\<rangle>]"
+    assume "leaf \<E> \<pi>" and "\<E> \<pi> = Some (\<langle>LET x = CHAN \<lparr>\<rparr> in e;\<rho>;\<kappa>\<rangle>)"
+    with \<open>(\<V>, \<C>) \<Turnstile>\<^sub>\<E> \<E>\<close>
+    have "(\<V>, \<C>) \<Turnstile>\<^sub>\<E> \<E>(\<pi> ;; (LNext x) \<mapsto> \<langle>e;\<rho> ++ [x \<mapsto> (VChan (Ch \<pi> x))];\<kappa>\<rangle>)" by (simp add: may_be_static_eval_preserved_under_chan)
+    with \<open>\<E>' = \<E> ++ [\<pi> ;; (LNext x) \<mapsto> \<langle>e;\<rho> ++ [x \<mapsto> (VChan (Ch \<pi> x))];\<kappa>\<rangle>]\<close>
+    show "(\<V>, \<C>) \<Turnstile>\<^sub>\<E> \<E>'" by simp
+  next
+    case (Let_Spawn \<pi> x e\<^sub>c e \<rho> \<kappa>)
+    assume "\<E>' = \<E> ++ [\<pi> ;; (LNext x) \<mapsto> \<langle>e;\<rho> ++ [x \<mapsto> VUnit];\<kappa>\<rangle>, \<pi> ;; (LSpawn x) \<mapsto> \<langle>e\<^sub>c;\<rho>;[]\<rangle>]"
+    assume "leaf \<E> \<pi>" and "\<E> \<pi> = Some (\<langle>LET x = SPAWN e\<^sub>c in e;\<rho>;\<kappa>\<rangle>)"
+    with \<open>(\<V>, \<C>) \<Turnstile>\<^sub>\<E> \<E>\<close>
+    have "(\<V>, \<C>) \<Turnstile>\<^sub>\<E> \<E>(\<pi> ;; (LNext x) \<mapsto> \<langle>e;\<rho> ++ [x \<mapsto> VUnit];\<kappa>\<rangle>, \<pi> ;; (LSpawn x) \<mapsto> \<langle>e\<^sub>c;\<rho>;[]\<rangle>)" by (simp add: may_be_static_eval_preserved_under_spawn)
+    with \<open>\<E>' = \<E> ++ [\<pi> ;; (LNext x) \<mapsto> \<langle>e;\<rho> ++ [x \<mapsto> VUnit];\<kappa>\<rangle>, \<pi> ;; (LSpawn x) \<mapsto> \<langle>e\<^sub>c;\<rho>;[]\<rangle>]\<close>
+    show "(\<V>, \<C>) \<Turnstile>\<^sub>\<E> \<E>'" by simp
+  next
+    case (Let_Sync \<pi>\<^sub>s x\<^sub>s x\<^sub>s\<^sub>e e\<^sub>s \<rho>\<^sub>s \<kappa>\<^sub>s x\<^sub>s\<^sub>c x\<^sub>m \<rho>\<^sub>s\<^sub>e \<pi>\<^sub>r x\<^sub>r x\<^sub>r\<^sub>e e\<^sub>r \<rho>\<^sub>r \<kappa>\<^sub>r x\<^sub>r\<^sub>c \<rho>\<^sub>r\<^sub>e c \<omega>\<^sub>m)
+    assume "\<E>' = \<E> ++ [\<pi>\<^sub>s ;; (LNext x\<^sub>s) \<mapsto> \<langle>e\<^sub>s;\<rho>\<^sub>s ++ [x\<^sub>s \<mapsto> VUnit];\<kappa>\<^sub>s\<rangle>, \<pi>\<^sub>r ;; (LNext x\<^sub>r) \<mapsto> \<langle>e\<^sub>r;\<rho>\<^sub>r ++ [x\<^sub>r \<mapsto> \<omega>\<^sub>m];\<kappa>\<^sub>r\<rangle>]"
+
+    assume "leaf \<E> \<pi>\<^sub>s"
+    and "\<E> \<pi>\<^sub>s = Some (\<langle>LET x\<^sub>s = SYNC x\<^sub>s\<^sub>e in e\<^sub>s;\<rho>\<^sub>s;\<kappa>\<^sub>s\<rangle>)"
+    and "\<rho>\<^sub>s x\<^sub>s\<^sub>e = Some (VClosure (Send_Evt x\<^sub>s\<^sub>c x\<^sub>m) \<rho>\<^sub>s\<^sub>e)"
+    and "leaf \<E> \<pi>\<^sub>r"
+    and "\<E> \<pi>\<^sub>r = Some (\<langle>LET x\<^sub>r = SYNC x\<^sub>r\<^sub>e in e\<^sub>r;\<rho>\<^sub>r;\<kappa>\<^sub>r\<rangle>)"
+    and "\<rho>\<^sub>r x\<^sub>r\<^sub>e = Some (VClosure (Recv_Evt x\<^sub>r\<^sub>c) \<rho>\<^sub>r\<^sub>e)"
+    and "\<rho>\<^sub>s\<^sub>e x\<^sub>s\<^sub>c = Some (VChan c)"
+    and "\<rho>\<^sub>r\<^sub>e x\<^sub>r\<^sub>c = Some (VChan c)"
+    and "\<rho>\<^sub>s\<^sub>e x\<^sub>m = Some \<omega>\<^sub>m"
+    with \<open>(\<V>, \<C>) \<Turnstile>\<^sub>\<E> \<E>\<close>
+    have "(\<V>, \<C>) \<Turnstile>\<^sub>\<E> \<E>(\<pi>\<^sub>s ;; (LNext x\<^sub>s) \<mapsto> \<langle>e\<^sub>s;\<rho>\<^sub>s ++ [x\<^sub>s \<mapsto> VUnit];\<kappa>\<^sub>s\<rangle>, \<pi>\<^sub>r ;; (LNext x\<^sub>r) \<mapsto> \<langle>e\<^sub>r;\<rho>\<^sub>r ++ [x\<^sub>r \<mapsto> \<omega>\<^sub>m];\<kappa>\<^sub>r\<rangle>)" by (simp add: may_be_static_eval_preserved_under_sync)
+    with \<open>\<E>' = \<E> ++ [\<pi>\<^sub>s ;; (LNext x\<^sub>s) \<mapsto> \<langle>e\<^sub>s;\<rho>\<^sub>s ++ [x\<^sub>s \<mapsto> VUnit];\<kappa>\<^sub>s\<rangle>, \<pi>\<^sub>r ;; (LNext x\<^sub>r) \<mapsto> \<langle>e\<^sub>r;\<rho>\<^sub>r ++ [x\<^sub>r \<mapsto> \<omega>\<^sub>m];\<kappa>\<^sub>r\<rangle>]\<close>
+    show "(\<V>, \<C>) \<Turnstile>\<^sub>\<E> \<E>'" by simp
+  qed
+qed
+
+
+theorem may_be_static_eval_preserved_under_concur_step_star : "
+  \<lbrakk>
+    (\<V>, \<C>) \<Turnstile>\<^sub>\<E> \<E>;  
+    (\<E>, H) \<rightarrow>* (\<E>', H')
+  \<rbrakk> \<Longrightarrow>
+  (\<V>, \<C>) \<Turnstile>\<^sub>\<E> \<E>'
+"
+proof -
+  assume 
+    H1: "(\<V>, \<C>) \<Turnstile>\<^sub>\<E> \<E>" and 
+    H2: "(\<E>, H) \<rightarrow>* (\<E>', H')" 
+
+  obtain X X' where H3: "X = (\<E>, H)" and H4: "X' = (\<E>', H')" by simp
+  
+  from H2 H3 H4 have H5: "X \<rightarrow>* X'" by simp
+ 
+  from H5 have 
+    H6: "\<forall> \<E> H \<E>' H' . X = (\<E>, H) \<longrightarrow> X' = (\<E>', H') \<longrightarrow> (\<V>, \<C>) \<Turnstile>\<^sub>\<E> \<E> \<longrightarrow> (\<V>, \<C>) \<Turnstile>\<^sub>\<E> \<E>'"
+  proof (induction rule: star.induct)
+    case (refl X0)
+    show ?case by simp
+  next
+    case (step X Xm X')
+
+    {
+      fix \<E> H \<E>' H' 
+      assume 
+        L1H1: "X = (\<E>, H)" and 
+        L1H2: "X' = (\<E>', H')" and 
+        L1H3: "(\<V>, \<C>) \<Turnstile>\<^sub>\<E> \<E>"
+
+      from L1H1 L1H2 L1H3 
+      have "(\<V>, \<C>) \<Turnstile>\<^sub>\<E> \<E>'"
+      by (metis eq_fst_iff may_be_static_eval_preserved_under_concur_step step.IH step.hyps(1))
+    }
+    
+    then show ?case by blast
+  qed 
+
+  from H1 H3 H4 H6
+  show "(\<V>, \<C>) \<Turnstile>\<^sub>\<E> \<E>'" by simp
+qed
+
+theorem may_be_static_eval_env_to_precise : "
+  \<rho> x = Some \<omega> \<Longrightarrow>
+  (\<V>, \<C>) \<Turnstile>\<^sub>\<rho> \<rho> \<Longrightarrow>
+  {|\<omega>|} \<subseteq> \<V> x
+"
+proof -
+  assume "\<rho> x = Some \<omega>" and "(\<V>, \<C>) \<Turnstile>\<^sub>\<rho> \<rho>" then
+  show "{|\<omega>|} \<subseteq> \<V> x" by (simp add: may_be_static_eval_env.simps)
+qed
+
+theorem may_be_static_eval_pool_to_precise : "
+  \<rho> x = Some \<omega> \<Longrightarrow>
+  \<E> \<pi> = Some (\<langle>e; \<rho>; \<kappa>\<rangle>) \<Longrightarrow>
+  (\<V>, \<C>) \<Turnstile>\<^sub>\<E> \<E> \<Longrightarrow>
+  {|\<omega>|} \<subseteq> \<V> x
+"
+proof -
+  assume "\<rho> x = Some \<omega>"
+
+  assume "(\<V>, \<C>) \<Turnstile>\<^sub>\<E> \<E>" and "\<E> \<pi> = Some (\<langle>e; \<rho>; \<kappa>\<rangle>)" then
+
+  have "(\<V>, \<C>) \<Turnstile>\<^sub>\<sigma> \<langle>e; \<rho>; \<kappa>\<rangle>" by (simp add: may_be_static_eval_pool.simps) then
+
+  have "(\<V>, \<C>) \<Turnstile>\<^sub>\<rho> \<rho>" by (simp add: may_be_static_eval_state.simps) 
+  with `\<rho> x = Some \<omega>`
+
+  show "{|\<omega>|} \<subseteq> \<V> x" by (simp add: may_be_static_eval_env.simps)
+qed
+
+theorem values_not_bound_pool_sound : "
+  \<rho>' x = Some \<omega> \<Longrightarrow>
+  (\<V>, \<C>) \<Turnstile>\<^sub>\<E> \<E> \<Longrightarrow> 
+  (\<E>, H) \<rightarrow>* (\<E>', H') \<Longrightarrow>
+  \<E>' \<pi> = Some (\<langle>e'; \<rho>'; \<kappa>'\<rangle>) \<Longrightarrow>
+  {|\<omega>|} \<subseteq> \<V> x
+"
+proof -
+  assume 
+    H1: "\<rho>' x = Some \<omega>" and
+    H2: "(\<V>, \<C>) \<Turnstile>\<^sub>\<E> \<E>" and 
+    H3: "(\<E>, H) \<rightarrow>* (\<E>', H')" and 
+    H4: "\<E>' \<pi> = Some (\<langle>e'; \<rho>'; \<kappa>'\<rangle>)"
+
+  from H2 H3
+  have H5: "(\<V>, \<C>) \<Turnstile>\<^sub>\<E> \<E>'" by (blast intro: may_be_static_eval_preserved_under_concur_step_star)
+
+  from H1 H4 H5
+  show "{|\<omega>|} \<subseteq> \<V> x" using may_be_static_eval_pool_to_precise by auto
+qed
+
+
+lemma may_be_static_eval_to_pool: "
+  \<lbrakk>
+    (\<V>, \<C>) \<Turnstile>\<^sub>e e
+  \<rbrakk> \<Longrightarrow>
+  (\<V>, \<C>) \<Turnstile>\<^sub>\<E> [[] \<mapsto> \<langle>e; empty; []\<rangle>]
+"
+proof -
+  assume "(\<V>, \<C>) \<Turnstile>\<^sub>e e"
+
+  have "(\<V>, \<C>) \<Turnstile>\<^sub>\<rho> empty" by (simp add: may_be_static_eval_value_may_be_static_eval_env.Intro)
+  have "(\<V>, \<C>) \<Turnstile>\<^sub>\<kappa> \<V> (\<lfloor>e\<rfloor>) \<Rrightarrow> []" by (simp add: may_be_static_eval_stack.Empty)
+
+  from `(\<V>, \<C>) \<Turnstile>\<^sub>e e` and `(\<V>, \<C>) \<Turnstile>\<^sub>\<rho> empty` and `(\<V>, \<C>) \<Turnstile>\<^sub>\<kappa> \<V> (\<lfloor>e\<rfloor>) \<Rrightarrow> []`
+  have "(\<V>, \<C>) \<Turnstile>\<^sub>\<sigma> \<langle>e; empty; []\<rangle>" by (simp add: may_be_static_eval_state.intros)
+
+  have "[[] \<mapsto> \<langle>e; empty; []\<rangle>] [] = Some (\<langle>e; empty; []\<rangle>)" by simp
+  with `(\<V>, \<C>) \<Turnstile>\<^sub>\<sigma> \<langle>e; empty; []\<rangle>`
+  show "(\<V>, \<C>) \<Turnstile>\<^sub>\<E> [[] \<mapsto> \<langle>e; empty; []\<rangle>]" by (simp add: may_be_static_eval_pool.intros)
+qed
+
+
+theorem values_not_bound_sound : "
+  \<rho>' x = Some \<omega> \<Longrightarrow>
+  (\<V>, \<C>) \<Turnstile>\<^sub>e e \<Longrightarrow>
+  ([[] \<mapsto> \<langle>e; empty; []\<rangle>], H) \<rightarrow>* (\<E>', H') \<Longrightarrow>
+  \<E>' \<pi> = Some (\<langle>e'; \<rho>'; \<kappa>'\<rangle>) \<Longrightarrow>
+  {|\<omega>|} \<subseteq> \<V> x
+"
+proof -
+  assume 
+    H1: "\<rho>' x = Some \<omega>" and
+    H2: "(\<V>, \<C>) \<Turnstile>\<^sub>e e" and 
+    H3: "([[] \<mapsto> \<langle>e; empty; []\<rangle>], H) \<rightarrow>* (\<E>', H')" and 
+    H4: "\<E>' \<pi> = Some (\<langle>e'; \<rho>'; \<kappa>'\<rangle>)"
+
+  from H2 have 
+    H5: "(\<V>, \<C>) \<Turnstile>\<^sub>\<E> [[] \<mapsto> \<langle>e; empty; []\<rangle>]" by (simp add: may_be_static_eval_to_pool)
+
+  from H1 H3 H4 H5
+  show " {|\<omega>|} \<subseteq> \<V> x" using values_not_bound_pool_sound by blast
+qed
+
+
+datatype node_label = NLet var | NResult var
+
+fun nodeLabel :: "exp \<Rightarrow> node_label" where
+  "nodeLabel (LET x = b in e) = NLet x" |
+  "nodeLabel (RESULT y) = NResult y"
+
+type_synonym node_set = "node_label set"
+
+type_synonym node_map = "node_label \<Rightarrow> var set"
+
+datatype edge_label = ENext | ESpawn | ECall | EReturn
+
+type_synonym flow_label = "(node_label \<times> edge_label \<times> node_label)"
+
+type_synonym flow_set = "flow_label set"
+
+type_synonym step_label = "(node_label \<times> edge_label)"
+
+type_synonym static_path = "step_label list"
+
+
+inductive is_super_exp :: "exp \<Rightarrow> exp \<Rightarrow> bool"  where
+  Refl : "
+    is_super_exp e e
+  " | 
+  Let_Spawn_Child: "
+    is_super_exp e\<^sub>c e \<Longrightarrow>
+    is_super_exp (LET x = SPAWN e\<^sub>c in e\<^sub>n) e
+  " |
+  Let_Case_Left: "
+    is_super_exp e\<^sub>l e \<Longrightarrow>
+    is_super_exp (LET x = CASE x\<^sub>s LEFT x\<^sub>l |> e\<^sub>l RIGHT x\<^sub>r |> e\<^sub>r in e\<^sub>n) e
+  " |
+  Let_Case_Right: "
+    is_super_exp e\<^sub>r e \<Longrightarrow>
+    is_super_exp (LET x = CASE x\<^sub>s LEFT x\<^sub>l |> e\<^sub>l RIGHT x\<^sub>r |> e\<^sub>r in e\<^sub>n) e
+  " |
+  Let_Abs_Body: "
+    is_super_exp e\<^sub>b e \<Longrightarrow>
+    is_super_exp (LET x = FN f x\<^sub>p . e\<^sub>b in e\<^sub>n) e
+  " | 
+  Let: "
+    is_super_exp e\<^sub>n e \<Longrightarrow>
+    is_super_exp (LET x = b in e\<^sub>n) e
+  "
+
+inductive is_super_exp_left :: "exp \<Rightarrow> exp \<Rightarrow> bool"  where
+  Refl : "
+    is_super_exp_left e0 e0
+  " | 
+  Let_Spawn_Child: "
+    is_super_exp_left e0 (LET x = SPAWN e\<^sub>c in e\<^sub>n)\<Longrightarrow>
+    is_super_exp_left e0 e\<^sub>c
+  " |
+  Let_Case_Left: "
+    is_super_exp_left e0 (LET x = CASE x\<^sub>s LEFT x\<^sub>l |> e\<^sub>l RIGHT x\<^sub>r |> e\<^sub>r in e\<^sub>n) \<Longrightarrow>
+    is_super_exp_left e0 e\<^sub>l
+  " |
+  Let_Case_Right: "
+    is_super_exp_left e0 (LET x = CASE x\<^sub>s LEFT x\<^sub>l |> e\<^sub>l RIGHT x\<^sub>r |> e\<^sub>r in e\<^sub>n) \<Longrightarrow>
+    is_super_exp_left e0 e\<^sub>r
+  " |
+  Let_Abs_Body: "
+    is_super_exp_left e0 (LET x = FN f x\<^sub>p . e\<^sub>b in e\<^sub>n) \<Longrightarrow>
+    is_super_exp_left e0 e\<^sub>b
+  " | 
+  Let: "
+    is_super_exp_left e0 (LET x = b in e\<^sub>n) \<Longrightarrow>
+    is_super_exp_left e0 e\<^sub>n
+  "
+
+
+lemma is_super_exp_trans: "
+  is_super_exp e\<^sub>z e\<^sub>y \<Longrightarrow> is_super_exp e\<^sub>y e\<^sub>x \<Longrightarrow> is_super_exp e\<^sub>z e\<^sub>x
+"
+proof -
+  assume "is_super_exp e\<^sub>y e\<^sub>x "
+  assume "is_super_exp e\<^sub>z e\<^sub>y" then
+  have "(\<forall> e\<^sub>x . is_super_exp e\<^sub>y e\<^sub>x \<longrightarrow> is_super_exp e\<^sub>z e\<^sub>x)"
+  proof (induction rule: is_super_exp.induct)
+    case (Refl e)
+    show "\<forall>e\<^sub>x. is_super_exp e e\<^sub>x \<longrightarrow> is_super_exp e e\<^sub>x" by simp
+  next
+    case (Let e\<^sub>n e x b)
+    assume "is_super_exp e\<^sub>n e" "\<forall>e\<^sub>x. is_super_exp e e\<^sub>x \<longrightarrow> is_super_exp e\<^sub>n e\<^sub>x"
+
+    have "\<forall>e\<^sub>x. is_super_exp e\<^sub>n e\<^sub>x \<longrightarrow> is_super_exp (LET x = b in e\<^sub>n) e\<^sub>x" by (simp add: is_super_exp.Let) 
+    with `\<forall>e\<^sub>x. is_super_exp e e\<^sub>x \<longrightarrow> is_super_exp e\<^sub>n e\<^sub>x`
+    show "\<forall>e\<^sub>x. is_super_exp e e\<^sub>x \<longrightarrow> is_super_exp (LET x = b in e\<^sub>n) e\<^sub>x" by blast
+  next
+    case (Let_Spawn_Child e\<^sub>c e x e\<^sub>n)
+    assume "is_super_exp e\<^sub>c e" "\<forall>e\<^sub>x. is_super_exp e e\<^sub>x \<longrightarrow> is_super_exp e\<^sub>c e\<^sub>x"
+
+    have "\<forall>e\<^sub>x. is_super_exp e\<^sub>c e\<^sub>x \<longrightarrow> is_super_exp (LET x = SPAWN e\<^sub>c in e\<^sub>n) e\<^sub>x" by (simp add: is_super_exp.Let_Spawn_Child)
+    with `\<forall>e\<^sub>x. is_super_exp e e\<^sub>x \<longrightarrow> is_super_exp e\<^sub>c e\<^sub>x`
+    show "\<forall>e\<^sub>x. is_super_exp e e\<^sub>x \<longrightarrow> is_super_exp (LET x = SPAWN e\<^sub>c in e\<^sub>n) e\<^sub>x"by blast
+  next
+    case (Let_Case_Left e\<^sub>l e x x\<^sub>s x\<^sub>l x\<^sub>r e\<^sub>r e\<^sub>n)
+    assume "is_super_exp e\<^sub>l e" "\<forall>e\<^sub>x. is_super_exp e e\<^sub>x \<longrightarrow> is_super_exp e\<^sub>l e\<^sub>x"
+
+    have "\<forall>e\<^sub>x. is_super_exp e\<^sub>l e\<^sub>x \<longrightarrow> is_super_exp (LET x = CASE x\<^sub>s LEFT x\<^sub>l |> e\<^sub>l RIGHT x\<^sub>r |> e\<^sub>r in e\<^sub>n) e\<^sub>x" by (simp add: is_super_exp.Let_Case_Left)
+    with `\<forall>e\<^sub>x. is_super_exp e e\<^sub>x \<longrightarrow> is_super_exp e\<^sub>l e\<^sub>x`
+    show "\<forall>e\<^sub>x. is_super_exp e e\<^sub>x \<longrightarrow> is_super_exp (LET x = CASE x\<^sub>s LEFT x\<^sub>l |> e\<^sub>l RIGHT x\<^sub>r |> e\<^sub>r in e\<^sub>n) e\<^sub>x" by blast
+  next
+    case (Let_Case_Right e\<^sub>r e x x\<^sub>s x\<^sub>l e\<^sub>l x\<^sub>r e\<^sub>n)
+    assume "is_super_exp e\<^sub>r e" "\<forall>e\<^sub>x. is_super_exp e e\<^sub>x \<longrightarrow> is_super_exp e\<^sub>r e\<^sub>x"
+
+    have "\<forall>e\<^sub>x. is_super_exp e\<^sub>r e\<^sub>x \<longrightarrow> is_super_exp (LET x = CASE x\<^sub>s LEFT x\<^sub>l |> e\<^sub>l RIGHT x\<^sub>r |> e\<^sub>r in e\<^sub>n) e\<^sub>x" by (simp add: is_super_exp.Let_Case_Right)
+    with `\<forall>e\<^sub>x. is_super_exp e e\<^sub>x \<longrightarrow> is_super_exp e\<^sub>r e\<^sub>x`
+    show "\<forall>e\<^sub>x. is_super_exp e e\<^sub>x \<longrightarrow> is_super_exp (LET x = CASE x\<^sub>s LEFT x\<^sub>l |> e\<^sub>l RIGHT x\<^sub>r |> e\<^sub>r in e\<^sub>n) e\<^sub>x" by blast
+  next
+    case (Let_Abs_Body e\<^sub>b e x f x\<^sub>p e\<^sub>n)
+    assume "is_super_exp e\<^sub>b e" "\<forall>e\<^sub>x. is_super_exp e e\<^sub>x \<longrightarrow> is_super_exp e\<^sub>b e\<^sub>x"
+
+    have "\<forall>e\<^sub>x. is_super_exp e\<^sub>b e\<^sub>x \<longrightarrow> is_super_exp (LET x = FN f x\<^sub>p . e\<^sub>b in e\<^sub>n) e\<^sub>x" by (simp add: is_super_exp.Let_Abs_Body)
+    with `\<forall>e\<^sub>x. is_super_exp e e\<^sub>x \<longrightarrow> is_super_exp e\<^sub>b e\<^sub>x`
+    show "\<forall>e\<^sub>x. is_super_exp e e\<^sub>x \<longrightarrow> is_super_exp (LET x = FN f x\<^sub>p . e\<^sub>b in e\<^sub>n) e\<^sub>x" by blast
+  qed 
+  with `is_super_exp e\<^sub>y e\<^sub>x`
+  show "is_super_exp e\<^sub>z e\<^sub>x" by blast
+qed
+
+lemma is_super_exp1: "
+  is_super_exp (LET x = b in e\<^sub>n) e\<^sub>n
+"
+by (simp add: is_super_exp.Let is_super_exp.Refl)
+
+lemma is_super_exp_left_implies_is_super_exp: "
+  is_super_exp_left e e' \<Longrightarrow> is_super_exp e e'
+"
+proof -
+  assume "is_super_exp_left e e'"
+  
+  then show "is_super_exp e e'"
+  proof induction
+    case (Refl e0)
+    show 
+      "is_super_exp e0 e0" by (simp add: is_super_exp.Refl)
+  next
+    case (Let_Spawn_Child e0 x e\<^sub>c e\<^sub>n)
+    from Let_Spawn_Child.IH show 
+      "is_super_exp e0 e\<^sub>c"
+    using is_super_exp.Let_Spawn_Child is_super_exp.Refl is_super_exp_trans by blast
+  next
+    case (Let_Case_Left e0 x x\<^sub>s x\<^sub>l e\<^sub>l x\<^sub>r e\<^sub>r e\<^sub>n)
+    from Let_Case_Left.IH show
+      "is_super_exp e0 e\<^sub>l"
+    using is_super_exp.Let_Case_Left is_super_exp.Refl is_super_exp_trans by blast
+  next
+    case (Let_Case_Right e0 x x\<^sub>s x\<^sub>l e\<^sub>l x\<^sub>r e\<^sub>r e\<^sub>n)
+    from Let_Case_Right.IH show 
+      "is_super_exp e0 e\<^sub>r"
+    using is_super_exp.Let_Case_Right is_super_exp.Refl is_super_exp_trans by blast
+  next
+    case (Let_Abs_Body e0 x f x\<^sub>p e\<^sub>b e\<^sub>n)
+    from Let_Abs_Body.IH show 
+      "is_super_exp e0 e\<^sub>b"
+    using is_super_exp.Let_Abs_Body is_super_exp.Refl is_super_exp_trans by blast
+  next
+    case (Let e0 x b e\<^sub>n)
+    from Let.IH show
+      "is_super_exp e0 e\<^sub>n"
+    using is_super_exp1 is_super_exp_trans by blast
+  qed
+qed
+
+
+inductive is_super_exp_over_prim :: "exp \<Rightarrow> prim \<Rightarrow> bool" where
+  Send_Evt: "
+    is_super_exp_over_prim e0 (Send_Evt xC xM)
+  " |
+  Recv_Evt: "
+    is_super_exp_over_prim e0 (Recv_Evt xC)
+  " |
+  Pair: "
+    is_super_exp_over_prim e0 (Pair x1 x2)
+  " |
+  Left: "
+    is_super_exp_over_prim e0 (Left x)
+  " |
+  Right: "
+    is_super_exp_over_prim e0 (Right x)
+  " |
+  Abs: "
+    is_super_exp_left e0 e\<^sub>b \<Longrightarrow>
+    is_super_exp_over_prim e0 (Abs f\<^sub>p x\<^sub>p e\<^sub>b)
+  " 
+
+inductive 
+  is_super_exp_over_env :: "exp \<Rightarrow> val_env \<Rightarrow> bool" and
+  is_super_exp_over_val :: "exp \<Rightarrow> val \<Rightarrow> bool"
+where
+  VUnit: "
+    is_super_exp_over_val e0 VUnit
+  " |
+  VChan: "
+    is_super_exp_over_val e0 (VChan c)
+  " |
+  VClosure: "
+    is_super_exp_over_prim e0 p \<Longrightarrow>
+    is_super_exp_over_env e0 \<rho>' \<Longrightarrow>
+    is_super_exp_over_val e0 (VClosure p \<rho>')
+  " |
+
+  Intro: "
+    \<forall> x \<omega> . \<rho> x = Some \<omega> \<longrightarrow> is_super_exp_over_val e0 \<omega> \<Longrightarrow>
+    is_super_exp_over_env e0 \<rho>
+  "
+
+inductive is_super_exp_over_stack :: "exp \<Rightarrow> cont list \<Rightarrow> bool" where
+  Empty: "
+    is_super_exp_over_stack e0 []
+  " |
+  Nonempty: "
+    is_super_exp_left e0 e\<^sub>\<kappa> \<Longrightarrow>
+    is_super_exp_over_env e0 \<rho>\<^sub>\<kappa> \<Longrightarrow>
+    is_super_exp_over_stack e0 \<kappa> \<Longrightarrow>
+    is_super_exp_over_stack e0 (\<langle>x\<^sub>\<kappa>,e\<^sub>\<kappa>,\<rho>\<^sub>\<kappa>\<rangle> # \<kappa>)
+  "
+
+inductive is_super_exp_over_state :: "exp \<Rightarrow> state \<Rightarrow> bool" where
+  Intro: "
+    is_super_exp_left e0 e \<Longrightarrow>
+    is_super_exp_over_env e0 \<rho> \<Longrightarrow>
+    is_super_exp_over_stack e0 \<kappa> \<Longrightarrow>
+    is_super_exp_over_state e0 (\<langle>e;\<rho>;\<kappa>\<rangle>)
+  "
+
+lemma is_super_exp_over_state_preserved: "
+  (E, H) \<rightarrow> (E', H') \<Longrightarrow>
+  \<forall>\<pi> \<sigma>. E \<pi> = Some \<sigma> \<longrightarrow> is_super_exp_over_state e\<^sub>0 \<sigma> \<Longrightarrow>
+  E' \<pi>' = Some \<sigma>' \<Longrightarrow>
+  is_super_exp_over_state e\<^sub>0 \<sigma>'
+"
+proof -
+  assume 
+    H1: "\<forall>\<pi> \<sigma>. E \<pi> = Some \<sigma> \<longrightarrow> is_super_exp_over_state e\<^sub>0 \<sigma>" and
+    H2: "E' \<pi>' = Some \<sigma>'" and
+    H3: "(E, H) \<rightarrow> (E', H')"
+
+  from H3 show "is_super_exp_over_state e\<^sub>0 \<sigma>'"
+  proof cases
+    case (Seq_Step_Down \<pi> x \<rho> x\<^sub>\<kappa> e\<^sub>\<kappa> \<rho>\<^sub>\<kappa> \<kappa> \<omega>)
+
+    from H1 local.Seq_Step_Down(4)
+    have L1H1: "is_super_exp_over_state e\<^sub>0 (\<langle>RESULT x;\<rho>;\<langle>x\<^sub>\<kappa>,e\<^sub>\<kappa>,\<rho>\<^sub>\<kappa>\<rangle> # \<kappa>\<rangle>)" by blast
+
+    then have 
+      L1H2: "is_super_exp_over_env e\<^sub>0 \<rho>" and 
+      L1H3: "is_super_exp_over_stack e\<^sub>0 (\<langle>x\<^sub>\<kappa>,e\<^sub>\<kappa>,\<rho>\<^sub>\<kappa>\<rangle> # \<kappa>)" by (blast dest: is_super_exp_over_state.cases)+
+
+    then have 
+      L1H4: "is_super_exp_left e\<^sub>0 e\<^sub>\<kappa>" and 
+      L1H5: "is_super_exp_over_env e\<^sub>0 \<rho>\<^sub>\<kappa>" and 
+      L1H6: "is_super_exp_over_stack e\<^sub>0 \<kappa>" by (blast dest: is_super_exp_over_stack.cases)+
+
+    from L1H2 L1H5 local.Seq_Step_Down(5) have L1H7: "is_super_exp_over_env e\<^sub>0 (\<rho>\<^sub>\<kappa>(x\<^sub>\<kappa> \<mapsto> \<omega>))"
+      by (smt is_super_exp_over_env.cases is_super_exp_over_env_is_super_exp_over_val.Intro map_upd_Some_unfold)
+
+    with L1H4 L1H6 L1H7 have L1H8: "is_super_exp_over_state e\<^sub>0 (\<langle>e\<^sub>\<kappa>;\<rho>\<^sub>\<kappa>(x\<^sub>\<kappa> \<mapsto> \<omega>);\<kappa>\<rangle>)"
+      by (simp add: is_super_exp_over_state.intros)
+
+    with H1 H2 local.Seq_Step_Down(1) show "is_super_exp_over_state e\<^sub>0 \<sigma>'"
+      by (metis map_add_empty map_add_upd map_upd_Some_unfold)
+  next
+    case (Seq_Step \<pi> x b el \<rho>l \<kappa>l \<omega>)
+
+    from H1 local.Seq_Step(4) 
+    have L1H1: "is_super_exp_over_state e\<^sub>0 (\<langle>LET x = b in el;\<rho>l;\<kappa>l\<rangle>)" by blast
+
+    then have 
+      L1H2: "is_super_exp_left e\<^sub>0 (LET x = b in el)" and
+      L1H3: "is_super_exp_over_env e\<^sub>0 \<rho>l" and
+      L1H4: "is_super_exp_over_stack e\<^sub>0 \<kappa>l" by (blast dest: is_super_exp_over_state.cases)+
+
+    from L1H2 have L1H5: "is_super_exp_left e\<^sub>0 el" by (blast dest: is_super_exp_left.Let)
+
+    from local.Seq_Step(5) have 
+      "is_super_exp_over_val e\<^sub>0 \<omega>"
+    proof cases
+      case Let_Unit
+      then show "is_super_exp_over_val e\<^sub>0 \<omega>" by (simp add: VUnit)
+    next
+      case (Let_Prim p)
+
+      have L2H1: "is_super_exp_over_prim e\<^sub>0 p"
+      proof (cases p)
+        case (Send_Evt x11 x12)
+        then show "is_super_exp_over_prim e\<^sub>0 p" by (simp add: is_super_exp_over_prim.Send_Evt)
+      next
+        case (Recv_Evt x2)
+        then show "is_super_exp_over_prim e\<^sub>0 p" by (simp add: is_super_exp_over_prim.Recv_Evt)
+      next
+        case (Pair x31 x32)
+        then show "is_super_exp_over_prim e\<^sub>0 p" by (simp add: is_super_exp_over_prim.Pair)
+      next
+        case (Left x4)
+        then show "is_super_exp_over_prim e\<^sub>0 p" by (simp add: is_super_exp_over_prim.Left)
+      next
+        case (Right x5)
+        then show "is_super_exp_over_prim e\<^sub>0 p" by (simp add: is_super_exp_over_prim.Right)
+      next
+        case (Abs x61 x62 x63)
+
+        with L1H2 local.Let_Prim(1) local.Abs
+        show "is_super_exp_over_prim e\<^sub>0 p" by (smt is_super_exp_left.Let_Abs_Body is_super_exp_over_prim.Abs )
+      qed
+
+      have L2H3: "is_super_exp_over_env e\<^sub>0 \<rho>l" by (simp add: L1H3)
+
+      with L2H1 have "is_super_exp_over_val e\<^sub>0 (VClosure p \<rho>l)" by (simp add: VClosure)
+
+      with local.Let_Prim(2) show "is_super_exp_over_val e\<^sub>0 \<omega>" by simp
+    next
+      case (Let_Fst x\<^sub>p x\<^sub>1 x\<^sub>2 \<rho>\<^sub>p)
+      then show "is_super_exp_over_val e\<^sub>0 \<omega>"
+        by (metis L1H3 is_super_exp_over_env.cases is_super_exp_over_val.cases val.distinct(3) val.distinct(5) val.inject(2))
+    next
+      case (Let_Snd x\<^sub>p x\<^sub>1 x\<^sub>2 \<rho>\<^sub>p)
+      then show "is_super_exp_over_val e\<^sub>0 \<omega>"
+        by (metis L1H3 is_super_exp_over_env.cases is_super_exp_over_val.cases val.distinct(3) val.distinct(5) val.inject(2))
+    qed
+    
+    with L1H3 have L1H6: "is_super_exp_over_env e\<^sub>0 (\<rho>l(x \<mapsto> \<omega>))"
+      by (smt is_super_exp_over_env.cases is_super_exp_over_env_is_super_exp_over_val.Intro map_upd_Some_unfold)
+
+    with L1H4 L1H5 have L1H7: "is_super_exp_over_state e\<^sub>0 (\<langle>el;\<rho>l(x \<mapsto> \<omega>);\<kappa>l\<rangle>)" by (simp add: is_super_exp_over_state.intros)
+   
+    with H1 H2 local.Seq_Step(1) show "is_super_exp_over_state e\<^sub>0 \<sigma>'"
+      by (metis map_add_empty map_add_upd map_upd_Some_unfold)
+  next
+    case (Seq_Step_Up \<pi> x b el \<rho>l \<kappa>l el' \<rho>l')
+
+    from H1 local.Seq_Step_Up(4) have 
+      L1H1: "is_super_exp_over_state e\<^sub>0 (\<langle>LET x = b in el;\<rho>l;\<kappa>l\<rangle>)" by blast
+
+    then have 
+      L1H2: "is_super_exp_left e\<^sub>0 (LET x = b in el)" and
+      L1H3: "is_super_exp_over_env e\<^sub>0 \<rho>l" and
+      L1H4: "is_super_exp_over_stack e\<^sub>0 \<kappa>l" by (blast dest: is_super_exp_over_state.cases)+
+
+    from L1H2 have 
+      L1H5: "is_super_exp_left e\<^sub>0 el" by (blast dest: is_super_exp_left.Let)
+
+    from L1H3 L1H4 L1H5 have 
+      L1H6: "is_super_exp_over_stack e\<^sub>0 (\<langle>x,el,\<rho>l\<rangle> # \<kappa>l)" 
+        by (simp add: is_super_exp_over_stack.Nonempty)
+
+    from local.Seq_Step_Up(5)
+    have 
+      L1H7: "is_super_exp_left e\<^sub>0 el' \<and> is_super_exp_over_env e\<^sub>0 \<rho>l'"
+    proof cases
+      case (Let_Case_Left x\<^sub>s x\<^sub>l' \<rho>\<^sub>l \<omega>\<^sub>l x\<^sub>l x\<^sub>r e\<^sub>r)
+
+      from L1H2 local.Let_Case_Left(1) have 
+        L2H1: "is_super_exp_left e\<^sub>0 el'" by (blast dest: is_super_exp_left.Let_Case_Left)
+
+      from L1H3 local.Let_Case_Left(3) have 
+        "is_super_exp_over_val e\<^sub>0 (VClosure (prim.Left x\<^sub>l') \<rho>\<^sub>l)"
+        by (blast dest: is_super_exp_over_env.cases)
+
+      then have "is_super_exp_over_env e\<^sub>0 \<rho>\<^sub>l" by (blast dest: is_super_exp_over_val.cases)
+
+      with local.Let_Case_Left(4) have "is_super_exp_over_val e\<^sub>0 \<omega>\<^sub>l" by (blast dest: is_super_exp_over_env.cases)
+
+      with L1H3 have "is_super_exp_over_env e\<^sub>0 (\<rho>l(x\<^sub>l \<mapsto> \<omega>\<^sub>l))"
+        by (smt is_super_exp_over_env.cases is_super_exp_over_env_is_super_exp_over_val.Intro map_upd_Some_unfold)
+
+      with local.Let_Case_Left(2) have 
+        L2H2: "is_super_exp_over_env e\<^sub>0 \<rho>l'" by simp
+
+      with L2H1 show "is_super_exp_left e\<^sub>0 el' \<and> is_super_exp_over_env e\<^sub>0 \<rho>l'" by simp
+    next
+      case (Let_Case_Right x\<^sub>s x\<^sub>r' \<rho>\<^sub>r \<omega>\<^sub>r x\<^sub>l e\<^sub>l x\<^sub>r)
+
+      from L1H2 local.Let_Case_Right(1) have 
+        L2H1: "is_super_exp_left e\<^sub>0 el'"
+          by (blast dest: is_super_exp_left.Let_Case_Right)
+
+      from L1H3 local.Let_Case_Right(3)
+      have "is_super_exp_over_val e\<^sub>0 (VClosure (prim.Right x\<^sub>r') \<rho>\<^sub>r)"
+        by (blast dest: is_super_exp_over_env.cases)
+
+      then have "is_super_exp_over_env e\<^sub>0 \<rho>\<^sub>r" by (blast dest: is_super_exp_over_val.cases)
+
+      with L1H3 local.Let_Case_Right(2) local.Let_Case_Right(4) have 
+        L2H2: "is_super_exp_over_env e\<^sub>0 \<rho>l'"
+          by (auto simp: is_super_exp_over_env.simps)
+
+      with L2H1 show "is_super_exp_left e\<^sub>0 el' \<and> is_super_exp_over_env e\<^sub>0 \<rho>l'" by simp
+    next
+      case (Let_App f f\<^sub>l x\<^sub>l \<rho>\<^sub>l x\<^sub>a \<omega>\<^sub>a)
+
+      from L1H3 local.Let_App(3) have
+        L2H1: "is_super_exp_over_val e\<^sub>0 (VClosure (Abs f\<^sub>l x\<^sub>l el') \<rho>\<^sub>l)" by (blast dest: is_super_exp_over_env.cases)
+
+      then have 
+        "is_super_exp_over_prim e\<^sub>0 (Abs f\<^sub>l x\<^sub>l el')" by (blast dest: is_super_exp_over_val.cases)
+
+      then have L2H2: "is_super_exp_left e\<^sub>0 el'" by (blast dest: is_super_exp_over_prim.cases)
+
+      from L2H1 have L2H3: "is_super_exp_over_env e\<^sub>0 \<rho>\<^sub>l" by (blast dest: is_super_exp_over_val.cases)
+
+      with L1H3 local.Let_App(4) have
+        L2H1: "is_super_exp_over_val e\<^sub>0 \<omega>\<^sub>a" by (blast dest: is_super_exp_over_env.cases)
+
+      with L1H3 L2H3 local.Let_App(2) local.Let_App(3) have 
+        L2H4: "is_super_exp_over_env e\<^sub>0 \<rho>l'" by (auto simp: is_super_exp_over_env.simps)
+
+       with L2H2 show "is_super_exp_left e\<^sub>0 el' \<and> is_super_exp_over_env e\<^sub>0 \<rho>l'" by simp
+    qed
+
+    with L1H6 have "is_super_exp_over_state e\<^sub>0 (\<langle>el';\<rho>l';\<langle>x,el,\<rho>l\<rangle> # \<kappa>l\<rangle>)" by (simp add: is_super_exp_over_state.intros)
+
+    with H1 H2 local.Seq_Step_Up(1) show 
+      "is_super_exp_over_state e\<^sub>0 \<sigma>'" by (metis fun_upd_other fun_upd_same map_add_empty map_add_upd option.sel)
+  next
+    case (Let_Chan \<pi> x e \<rho> \<kappa>)
+
+    from H1 local.Let_Chan(4) have 
+      "is_super_exp_over_state e\<^sub>0 (\<langle>LET x = CHAN \<lparr>\<rparr> in e;\<rho>;\<kappa>\<rangle>)" by simp
+
+    then have
+      L1H1: "is_super_exp_left e\<^sub>0 (LET x = CHAN \<lparr>\<rparr> in e)" and
+      L1H2: "is_super_exp_over_env e\<^sub>0 \<rho>" and
+      L1H3: "is_super_exp_over_stack e\<^sub>0 \<kappa>" using is_super_exp_over_state.cases by blast+
+
+    from L1H1 have
+      L1H4: "is_super_exp_left e\<^sub>0 e" using is_super_exp_left.Let by blast
+
+    from L1H2 have
+      L1H5: "is_super_exp_over_env e\<^sub>0 (\<rho>(x \<mapsto> VChan (Ch \<pi> x)))" using VChan is_super_exp_over_env.simps by auto
+
+    from L1H4 L1H5 L1H3 have
+      "is_super_exp_over_state e\<^sub>0 (\<langle>e;\<rho> ++ [x \<mapsto> VChan (Ch \<pi> x)];\<kappa>\<rangle>)" using is_super_exp_over_state.intros by simp
+
+    with H1 H2 local.Let_Chan(1) show
+      "is_super_exp_over_state e\<^sub>0 \<sigma>'" by (metis fun_upd_other fun_upd_same map_add_empty map_add_upd option.sel)
+  next
+    case (Let_Spawn \<pi> x e\<^sub>c e \<rho> \<kappa>)
+
+    from H1 local.Let_Spawn(4) have
+      "is_super_exp_over_state e\<^sub>0 (\<langle>LET x = SPAWN e\<^sub>c in e;\<rho>;\<kappa>\<rangle>)" by blast
+
+    then have
+      L1H1: "is_super_exp_left e\<^sub>0 (LET x = SPAWN e\<^sub>c in e)" and
+      L1H2: "is_super_exp_over_env e\<^sub>0 \<rho>" and
+      L1H3: "is_super_exp_over_stack e\<^sub>0 \<kappa>" using is_super_exp_over_state.cases by blast+
+
+    from L1H1 have
+      L1H4: "is_super_exp_left e\<^sub>0 e\<^sub>c" using is_super_exp_left.Let_Spawn_Child by blast
+
+    from L1H1 have
+      L1H5: "is_super_exp_left e\<^sub>0 e" using is_super_exp_left.Let by blast
+
+    from L1H2 L1H4 have
+      L1H6: "is_super_exp_over_state e\<^sub>0 (\<langle>e\<^sub>c;\<rho>;[]\<rangle>)" by (simp add: is_super_exp_over_stack.Empty is_super_exp_over_state.intros)
+
+    have
+      L1H7: "is_super_exp_over_val e\<^sub>0 VUnit" by (simp add: VUnit)
+
+    from L1H2 L1H3 L1H5 L1H7 have
+      L1H8: "is_super_exp_over_state e\<^sub>0 (\<langle>e;\<rho>(x \<mapsto> VUnit);\<kappa>\<rangle>)" by (simp add:is_super_exp_over_env.simps is_super_exp_over_state.intros)
+   
+    from H1 H2 L1H6 L1H8 local.Let_Spawn(1) show
+      "is_super_exp_over_state e\<^sub>0 \<sigma>'" by (smt fun_upd_apply map_add_empty map_add_upd option.sel)
+
+  next
+    case (Let_Sync \<pi>\<^sub>s x\<^sub>s x\<^sub>s\<^sub>e e\<^sub>s \<rho>\<^sub>s \<kappa>\<^sub>s x\<^sub>s\<^sub>c x\<^sub>m \<rho>\<^sub>s\<^sub>e \<pi>\<^sub>r x\<^sub>r x\<^sub>r\<^sub>e e\<^sub>r \<rho>\<^sub>r \<kappa>\<^sub>r x\<^sub>r\<^sub>c \<rho>\<^sub>r\<^sub>e c \<omega>\<^sub>m)
+
+    from H1 local.Let_Sync(7) have 
+      "is_super_exp_over_state e\<^sub>0 (\<langle>LET x\<^sub>r = SYNC x\<^sub>r\<^sub>e in e\<^sub>r;\<rho>\<^sub>r;\<kappa>\<^sub>r\<rangle>)" by blast
+
+    then have 
+      L1H1: "is_super_exp_left e\<^sub>0 (LET x\<^sub>r = SYNC x\<^sub>r\<^sub>e in e\<^sub>r)" and
+      L1H2: "is_super_exp_over_env e\<^sub>0 \<rho>\<^sub>r" and
+      L1H3: "is_super_exp_over_stack e\<^sub>0 \<kappa>\<^sub>r" using is_super_exp_over_state.cases by blast+
+
+    have 
+      L1H4: "is_super_exp_left e\<^sub>0 e\<^sub>r"
+      using L1H1 is_super_exp_left.Let by blast
+
+    from H1 local.Let_Sync(4) have 
+      "is_super_exp_over_state e\<^sub>0 (\<langle>LET x\<^sub>s = SYNC x\<^sub>s\<^sub>e in e\<^sub>s;\<rho>\<^sub>s;\<kappa>\<^sub>s\<rangle>)" by blast
+
+    then have 
+      L1H5: "is_super_exp_left e\<^sub>0 (LET x\<^sub>s = SYNC x\<^sub>s\<^sub>e in e\<^sub>s)" and
+      L1H6: "is_super_exp_over_env e\<^sub>0 \<rho>\<^sub>s" and
+      L1H7: "is_super_exp_over_stack e\<^sub>0 \<kappa>\<^sub>s" using is_super_exp_over_state.cases by blast+
+
+    from L1H6 local.Let_Sync(5) have 
+      L1H8: "is_super_exp_over_val e\<^sub>0 (VClosure (Send_Evt x\<^sub>s\<^sub>c x\<^sub>m) \<rho>\<^sub>s\<^sub>e)" using is_super_exp_over_env.cases by auto
+
+    then have 
+      L1H9: "is_super_exp_over_env e\<^sub>0 \<rho>\<^sub>s\<^sub>e"  using is_super_exp_over_val.cases by blast
+
+    from L1H9 local.Let_Sync(11) have 
+      L1H10: "is_super_exp_over_val e\<^sub>0 \<omega>\<^sub>m" using is_super_exp_over_env.cases by auto
+
+    from L1H5 have 
+      L1H11: "is_super_exp_left e\<^sub>0 e\<^sub>s" using is_super_exp_left.Let by blast
+
+    have 
+      L1H12: "is_super_exp_over_val e\<^sub>0 VUnit" by (simp add: VUnit)
+
+    from L1H2 L1H3 L1H4 L1H10 L1H12 have 
+      L1H13: "is_super_exp_over_state e\<^sub>0 (\<langle>e\<^sub>r;\<rho>\<^sub>r(x\<^sub>r \<mapsto> \<omega>\<^sub>m);\<kappa>\<^sub>r\<rangle>)" by (simp add: is_super_exp_over_env.simps is_super_exp_over_state.intros)
+
+    from L1H6 L1H7 L1H11 L1H12 have 
+      L1H14: "is_super_exp_over_state e\<^sub>0 (\<langle>e\<^sub>s;\<rho>\<^sub>s(x\<^sub>s \<mapsto> VUnit);\<kappa>\<^sub>s\<rangle>)" by (simp add: is_super_exp_over_env.simps is_super_exp_over_state.intros)
+
+    from H1 H2 L1H13 L1H14 local.Let_Sync(1) show 
+      "is_super_exp_over_state e\<^sub>0 \<sigma>'" by (smt fun_upd_apply map_add_empty map_add_upd option.sel)
+
+  qed
+qed
+
+lemma isnt_exp_sound_generalized: "
+  (\<E>0, H0) \<rightarrow>* (\<E>', H') \<Longrightarrow>
+  \<E>0 = [[] \<mapsto> \<langle>e\<^sub>0;Map.empty;[]\<rangle>] \<Longrightarrow>
+  \<E>' \<pi>' = Some \<sigma>' \<Longrightarrow>
+  is_super_exp_over_state e\<^sub>0 \<sigma>'
+"
+proof -
+  assume 
+    H1: "\<E>0 = [[] \<mapsto> \<langle>e\<^sub>0;Map.empty;[]\<rangle>]" and 
+    H2: "\<E>' \<pi>' = Some \<sigma>'" and
+    H3: "(\<E>0, H0) \<rightarrow>* (\<E>', H')"
+
+  obtain X0 X' where
+    H4: "X0 = (\<E>0, H0)" and 
+    H5: "X' = (\<E>', H')" by simp
+
+  from H3 H4 H5 have 
+    H6: "star_left (op \<rightarrow>) X0 X'" by (simp add: star_implies_star_left)
+
+  then have 
+    H7: "
+      \<forall> \<E>0 H0 \<E>' H' \<pi>' \<sigma>' .
+      X0 = (\<E>0, H0) \<longrightarrow> X' = (\<E>', H') \<longrightarrow>
+      \<E>0 = [[] \<mapsto> \<langle>e\<^sub>0;Map.empty;[]\<rangle>] \<longrightarrow>
+      \<E>' \<pi>' = Some \<sigma>' \<longrightarrow>
+      is_super_exp_over_state e\<^sub>0 \<sigma>'
+    " 
+  proof (induction)
+    case (refl z)
+
+    {
+      fix \<E>0 H0 \<E>' H' \<pi>' \<sigma>'
+      assume 
+        L1H0: "z = (\<E>0, H0)" "z = (\<E>', H')" and
+        L1H1: "\<E>0 = [[] \<mapsto> \<langle>e\<^sub>0;Map.empty;[]\<rangle>]" and
+        L1H2:  "\<E>0 \<pi>' = Some \<sigma>'"
+  
+      have 
+        L1H3: "is_super_exp_left e\<^sub>0 e\<^sub>0" by (simp add: is_super_exp_left.Refl)
+      have 
+        L1H4: "is_super_exp_over_env e\<^sub>0 Map.empty" by (simp add: is_super_exp_over_env_is_super_exp_over_val.Intro)
+      have 
+        L1H5: "is_super_exp_over_stack e\<^sub>0 []" by (simp add: is_super_exp_over_stack.Empty)
+
+      from L1H3 L1H4 L1H5 have 
+        L1H6: "is_super_exp_over_state e\<^sub>0 (\<langle>e\<^sub>0;Map.empty;[]\<rangle>)" by (simp add: is_super_exp_over_state.intros)
+
+     from L1H1 L1H2 L1H6 have
+        "is_super_exp_over_state e\<^sub>0 \<sigma>'" by (metis fun_upd_apply option.distinct(1) option.sel)
+    }
+
+    then show ?case by blast
+  next
+    case (step x y z)
+    {
+      fix \<E>0 H0 \<E>' H' \<pi>' \<sigma>'
+      assume 
+        L1H0: "x = (\<E>0, H0)" "z = (\<E>', H')" and 
+        L2H1: "\<E>0 = [[] \<mapsto> \<langle>e\<^sub>0;Map.empty;[]\<rangle>]" and
+        L2H2: "\<E>' \<pi>' = Some \<sigma>'"
+
+
+      obtain \<E> H where L2H3: "y = (\<E>, H)" by (meson surj_pair)
+      from L1H0(1) L2H1 L2H3 step.IH have 
+        L2H4: "\<forall>\<pi> \<sigma>. \<E> \<pi> = Some \<sigma> \<longrightarrow> is_super_exp_over_state e\<^sub>0 \<sigma>" by blast
+
+      from L1H0(2) L2H2 L2H3 L2H4 step.hyps(2) have 
+        "is_super_exp_over_state e\<^sub>0 \<sigma>'" using is_super_exp_over_state_preserved by blast
+
+    } 
+
+    then show ?case by blast
+  qed
+
+  from H1 H2 H4 H5 H7 show 
+    "is_super_exp_over_state e\<^sub>0 \<sigma>'" by blast
+qed
+
+lemma isnt_exp_sound: "
+  ([[] \<mapsto> \<langle>e\<^sub>0;Map.empty;[]\<rangle>], {}) \<rightarrow>* (\<E>', H') \<Longrightarrow>
+  \<E>' \<pi>' = Some (\<langle>e';\<rho>';\<kappa>'\<rangle>) \<Longrightarrow>
+  is_super_exp e\<^sub>0 e'
+" 
+using is_super_exp_left_implies_is_super_exp is_super_exp_over_state.simps isnt_exp_sound_generalized by fastforce
+
+
+
 end
